<?xml version="1.0"?>


<!DOCTYPE rdf:RDF [
    <!ENTITY owl "http://www.w3.org/2002/07/owl#" >
    <!ENTITY xsd "http://www.w3.org/2001/XMLSchema#" >
    <!ENTITY teddy "http://biomodels.net/teddy/TEDDY#" >
    <!ENTITY skos "http://www.w3.org/2004/02/skos/core#" >
    <!ENTITY ro "http://www.obofoundry.org/ro/ro.owl#" >
    <!ENTITY rdfs "http://www.w3.org/2000/01/rdf-schema#" >
    <!ENTITY rdf "http://www.w3.org/1999/02/22-rdf-syntax-ns#" >
    <!ENTITY protege "http://protege.stanford.edu/plugins/owl/protege#" >
]>


<rdf:RDF xmlns="http://biomodels.net/teddy/TEDDY#"
     xml:base="http://biomodels.net/teddy/TEDDY"
     xmlns:rdfs="http://www.w3.org/2000/01/rdf-schema#"
     xmlns:ro="http://www.obofoundry.org/ro/ro.owl#"
     xmlns:protege="http://protege.stanford.edu/plugins/owl/protege#"
     xmlns:owl="http://www.w3.org/2002/07/owl#"
     xmlns:xsd="http://www.w3.org/2001/XMLSchema#"
     xmlns:rdf="http://www.w3.org/1999/02/22-rdf-syntax-ns#"
     xmlns:skos="http://www.w3.org/2004/02/skos/core#"
     xmlns:teddy="http://biomodels.net/teddy/TEDDY#">
    <owl:Ontology rdf:about="http://biomodels.net/teddy/TEDDY#">
        <rdfs:label xml:lang="en">TErminology for the Description of DYnamics (TEDDY)</rdfs:label>
        <rdfs:seeAlso rdf:datatype="&xsd;anyURI">http://biomodels.net/teddy</rdfs:seeAlso>
        <owl:priorVersion rdf:datatype="&xsd;anyURI">http://teddyontology.svn.sourceforge.net/svnroot/teddyontology/teddy/tags/rel-2011-08-30/teddy.owl</owl:priorVersion>
        <owl:versionInfo rdf:datatype="&xsd;anyURI">rel-2014-04-24</owl:versionInfo>
        <rdfs:comment xml:lang="en">The TErminology for the Description of DYnamics (TEDDY) project aims to provide an ontology for dynamical behaviours, observable dynamical phenomena, and control elements of bio-models and biological systems in Systems Biology and Synthetic Biology.</rdfs:comment>
        <protege:defaultLanguage>en</protege:defaultLanguage>
    </owl:Ontology>
    


    <!-- 
    ///////////////////////////////////////////////////////////////////////////////////////
    //
    // Annotation properties
    //
    ///////////////////////////////////////////////////////////////////////////////////////
     -->

    


    <!-- http://www.w3.org/2004/02/skos/core#altLabel -->

    <owl:AnnotationProperty rdf:about="&skos;altLabel"/>
    


    <!-- http://www.w3.org/2004/02/skos/core#definition -->

    <owl:AnnotationProperty rdf:about="&skos;definition"/>
    


    <!-- http://www.w3.org/2004/02/skos/core#prefLabel -->

    <owl:AnnotationProperty rdf:about="&skos;prefLabel"/>
    


    <!-- 
    ///////////////////////////////////////////////////////////////////////////////////////
    //
    // Object Properties
    //
    ///////////////////////////////////////////////////////////////////////////////////////
     -->

    


    <!-- http://biomodels.net/teddy/TEDDY#TEDDY_0000174 -->

    <owl:ObjectProperty rdf:about="&teddy;TEDDY_0000174">
        <rdfs:label xml:lang="en">dependsOn</rdfs:label>
        <owl:deprecated xml:lang="en">Relates temporal behaviours [https://identifiers.org/biomodels.teddy/TEDDY_0000083] to functional motifs [https://identifiers.org/biomodels.teddy/TEDDY_0000003] they depend on.</owl:deprecated>
        <rdfs:range rdf:resource="&teddy;TEDDY_0000003"/>
        <rdfs:domain rdf:resource="&teddy;TEDDY_0000083"/>
    </owl:ObjectProperty>
    


    <!-- http://biomodels.net/teddy/TEDDY#TEDDY_0000176 -->

    <owl:ObjectProperty rdf:about="&teddy;TEDDY_0000176">
        <rdfs:label xml:lang="en">hasFeature</rdfs:label>
        <rdfs:comment xml:lang="en">Links a dynamic system to the way one or several temporal behaviours [https://identifiers.org/biomodels.teddy/TEDDY_0000083] are modified or related upon interaction with information external to the system considered. </rdfs:comment>
        <rdfs:range rdf:resource="&teddy;TEDDY_0000132"/>
    </owl:ObjectProperty>
    


    <!-- http://biomodels.net/teddy/TEDDY#TR_0004 -->

    <owl:ObjectProperty rdf:about="&teddy;TR_0004">
        <rdfs:label xml:lang="en">hasCharacteristic</rdfs:label>
        <skos:definition xml:lang="en">Used to describe properties by means of behaviour characteristic [https://identifiers.org/biomodels.teddy/TEDDY_0000002].</skos:definition>
        <rdfs:range rdf:resource="&teddy;TEDDY_0000002"/>
    </owl:ObjectProperty>
    


    <!-- http://biomodels.net/teddy/TEDDY#TR_0006 -->

    <owl:ObjectProperty rdf:about="&teddy;TR_0006">
        <rdfs:label xml:lang="en">hasSubPart</rdfs:label>
        <owl:deprecated rdf:datatype="&xsd;boolean">true</owl:deprecated>
        <rdfs:subPropertyOf rdf:resource="&ro;has_part"/>
    </owl:ObjectProperty>
    


    <!-- http://biomodels.net/teddy/TEDDY#TR_0008 -->

    <owl:ObjectProperty rdf:about="&teddy;TR_0008">
        <rdfs:label xml:lang="en">hasSuperPart</rdfs:label>
        <owl:deprecated rdf:datatype="&xsd;boolean">true</owl:deprecated>
        <rdfs:subPropertyOf rdf:resource="&ro;has_part"/>
    </owl:ObjectProperty>
    


    <!-- http://biomodels.net/teddy/TEDDY#TR_0010 -->

    <owl:ObjectProperty rdf:about="&teddy;TR_0010">
        <rdfs:label xml:lang="en">hasOnPart</rdfs:label>
        <owl:deprecated rdf:datatype="&xsd;boolean">true</owl:deprecated>
        <rdfs:subPropertyOf rdf:resource="&ro;has_part"/>
    </owl:ObjectProperty>
    


    <!-- http://biomodels.net/teddy/TEDDY#TR_0012 -->

    <owl:ObjectProperty rdf:about="&teddy;TR_0012">
        <rdf:type rdf:resource="&owl;IrreflexiveProperty"/>
        <rdf:type rdf:resource="&owl;SymmetricProperty"/>
        <rdfs:label xml:lang="en">adjacentTo</rdfs:label>
        <skos:definition xml:lang="en">Two temporal behaviours [https://identifiers.org/biomodels.teddy/TEDDY_0000083] are adjacentTo each other if and only if they are in phase space proximity.</skos:definition>
        <rdfs:domain rdf:resource="&teddy;TEDDY_0000083"/>
        <rdfs:range rdf:resource="&teddy;TEDDY_0000083"/>
    </owl:ObjectProperty>
    


    <!-- http://biomodels.net/teddy/TEDDY#TR_0013 -->

    <owl:ObjectProperty rdf:about="&teddy;TR_0013">
        <rdfs:label xml:lang="en">convergeTo</rdfs:label>
        <skos:definition xml:lang="en">A temporal behaviour [https://identifiers.org/biomodels.teddy/TEDDY_0000083] convergeTo another temporal behaviour [https://identifiers.org/biomodels.teddy/TEDDY_0000083] if and only if it reaches the other behaviour [https://identifiers.org/biomodels.teddy/TEDDY_0000083] as time goes to either positive or negative infinity.</skos:definition>
        <rdfs:range rdf:resource="&teddy;TEDDY_0000083"/>
        <rdfs:domain rdf:resource="&teddy;TEDDY_0000083"/>
    </owl:ObjectProperty>
    


    <!-- http://biomodels.net/teddy/TEDDY#TR_0015 -->

    <owl:ObjectProperty rdf:about="&teddy;TR_0015">
        <rdf:type rdf:resource="&owl;FunctionalProperty"/>
        <rdf:type rdf:resource="&owl;SymmetricProperty"/>
        <rdfs:label xml:lang="en">reverseOf</rdfs:label>
        <skos:definition xml:lang="en">reverseOf links two temporal behaviours [https://identifiers.org/biomodels.teddy/TEDDY_0000083] whose phase diagrams can be obtained from each other by reversing the directions of all the phase paths.</skos:definition>
        <rdfs:domain rdf:resource="&teddy;TEDDY_0000083"/>
        <rdfs:range rdf:resource="&teddy;TEDDY_0000083"/>
    </owl:ObjectProperty>
    


    <!-- http://biomodels.net/teddy/TEDDY#TR_0016 -->

    <owl:ObjectProperty rdf:about="&teddy;TR_0016">
        <rdfs:label xml:lang="en">transforms</rdfs:label>
        <owl:deprecated rdf:datatype="&xsd;boolean">true</owl:deprecated>
        <rdfs:domain rdf:resource="&teddy;TEDDY_0000053"/>
        <rdfs:range rdf:resource="&teddy;TEDDY_0000083"/>
    </owl:ObjectProperty>
    


    <!-- http://biomodels.net/teddy/TEDDY#TR_0017 -->

    <owl:ObjectProperty rdf:about="&teddy;TR_0017">
        <rdfs:label xml:lang="en">below</rdfs:label>
        <skos:definition xml:lang="en">Links a bifurcation [https://identifiers.org/biomodels.teddy/TEDDY_0000053] to a &apos;temporal behaviour&apos; [https://identifiers.org/biomodels.teddy/TEDDY_0000083] which exists below the critical value of the bifurcation parameter.</skos:definition>
        <rdfs:subPropertyOf rdf:resource="&teddy;TR_0016"/>
    </owl:ObjectProperty>
    


    <!-- http://biomodels.net/teddy/TEDDY#TR_0018 -->

    <owl:ObjectProperty rdf:about="&teddy;TR_0018">
        <rdfs:label xml:lang="en">above</rdfs:label>
        <skos:definition xml:lang="en">Links a bifurcation [https://identifiers.org/biomodels.teddy/TEDDY_0000053] to a &apos;temporal behaviour&apos; [https://identifiers.org/biomodels.teddy/TEDDY_0000083] which exists above the critical value of the bifurcation parameter.</skos:definition>
        <rdfs:subPropertyOf rdf:resource="&teddy;TR_0016"/>
    </owl:ObjectProperty>
    


    <!-- http://www.obofoundry.org/ro/ro.owl#has_part -->

    <owl:ObjectProperty rdf:about="&ro;has_part">
        <rdf:type rdf:resource="&owl;ReflexiveProperty"/>
        <rdfs:label xml:lang="en">hasPart</rdfs:label>
        <skos:definition rdf:datatype="&xsd;anyURI">Inverse of partOf [obo:part_of].</skos:definition>
        <owl:inverseOf rdf:resource="&ro;part_of"/>
    </owl:ObjectProperty>
    


    <!-- http://www.obofoundry.org/ro/ro.owl#part_of -->

    <owl:ObjectProperty rdf:about="&ro;part_of">
        <rdf:type rdf:resource="&owl;ReflexiveProperty"/>
        <rdfs:label xml:lang="en">partOf</rdfs:label>
        <rdfs:seeAlso rdf:datatype="&xsd;anyURI">http://obofoundry.org/ro/#OBO_REL:part_of</rdfs:seeAlso>
        <rdfs:comment>For continuants: C part_of C* if and only if: given any c that instantiates C at a time t, there is some c* such that c* instantiates C* at time t, and c part_of c* at t. 
For processes: P part_of P* if and only if: given any p that instantiates P at a time t, there is some p* such that p* instantiates P* at time t, and p part_of p* at t. (Here part_of is the instance-level part-relation.)</rdfs:comment>
    </owl:ObjectProperty>
    


    <!-- 
    ///////////////////////////////////////////////////////////////////////////////////////
    //
    // Data properties
    //
    ///////////////////////////////////////////////////////////////////////////////////////
     -->

    


    <!-- http://biomodels.net/teddy/TEDDY#TR_0009 -->

    <owl:DatatypeProperty rdf:about="&teddy;TR_0009">
        <rdf:type rdf:resource="&owl;FunctionalProperty"/>
        <rdfs:label xml:lang="en">hasValue</rdfs:label>
        <skos:definition xml:lang="en">Links a &apos;behaviour characteristic&apos; [https://identifiers.org/biomodels.teddy/TEDDY_0000002] to the type of its value.</skos:definition>
        <rdfs:domain rdf:resource="&teddy;TEDDY_0000002"/>
    </owl:DatatypeProperty>
    


    <!-- 
    ///////////////////////////////////////////////////////////////////////////////////////
    //
    // Classes
    //
    ///////////////////////////////////////////////////////////////////////////////////////
     -->

    


    <!-- http://biomodels.net/teddy/TEDDY#TEDDY_0000000 -->

    <owl:Class rdf:about="&teddy;TEDDY_0000000">
        <rdfs:label xml:lang="en">TEDDY entity</rdfs:label>
        <skos:definition xml:lang="en">A Thing related to the dynamics of bio-models and biological systems. Terms belonging to TEDDY Entities are used in descriptions of dynamical behaviours, observable dynamical phenomena, and control elements in Systems Biology and Synthetic Biology.</skos:definition>
    </owl:Class>
    


    <!-- http://biomodels.net/teddy/TEDDY#TEDDY_0000001 -->

    <owl:Class rdf:about="&teddy;TEDDY_0000001">
        <rdfs:label xml:lang="en">curve ((obsolete))</rdfs:label>
        <rdfs:subClassOf rdf:resource="&teddy;TEDDY_obsolete"/>
        <owl:deprecated rdf:datatype="&xsd;boolean">true</owl:deprecated>
        <skos:definition xml:lang="en">Obsolete: equivalent to TEDDY_0000083 &apos;Temporal Behaviour&apos;.</skos:definition>
    </owl:Class>
    


    <!-- http://biomodels.net/teddy/TEDDY#TEDDY_0000002 -->

    <owl:Class rdf:about="&teddy;TEDDY_0000002">
        <rdfs:label xml:lang="en">behaviour characteristic</rdfs:label>
        <rdfs:subClassOf rdf:resource="&teddy;TEDDY_0000000"/>
        <skos:definition xml:lang="en">Behaviour characteristic is a property that characterizes temporal behaviors [https://identifiers.org/biomodels.teddy/TEDDY_0000083].</skos:definition>
    </owl:Class>
    


    <!-- http://biomodels.net/teddy/TEDDY#TEDDY_0000003 -->

    <owl:Class rdf:about="&teddy;TEDDY_0000003">
        <rdfs:label xml:lang="en">functional motif</rdfs:label>
        <rdfs:subClassOf rdf:resource="&teddy;TEDDY_0000000"/>
        <rdfs:seeAlso rdf:datatype="&xsd;anyURI">https://identifiers.org/doi/10.1371/journal.pbio.0020369</rdfs:seeAlso>
        <skos:definition xml:lang="en">A connected graph or network consisting of M vertices and a set of edges having a particular functional significance, forming a subgraph of a larger network.</skos:definition>
    </owl:Class>
    <owl:Axiom>
        <owl:annotatedTarget rdf:datatype="&xsd;anyURI">https://identifiers.org/doi/10.1371/journal.pbio.0020369</owl:annotatedTarget>
        <rdfs:comment xml:lang="en">Sporns O, Kötter R (2004) Motifs in Brain Networks, PLoS Biology, 2(11):e369.</rdfs:comment>
        <owl:annotatedSource rdf:resource="&teddy;TEDDY_0000003"/>
        <owl:annotatedProperty rdf:resource="&rdfs;seeAlso"/>
    </owl:Axiom>
    


    <!-- http://biomodels.net/teddy/TEDDY#TEDDY_0000004 -->

    <owl:Class rdf:about="&teddy;TEDDY_0000004">
        <rdfs:label xml:lang="en">monotonicity</rdfs:label>
        <rdfs:subClassOf rdf:resource="&teddy;TEDDY_0000144"/>
        <rdfs:seeAlso rdf:datatype="&xsd;anyURI">http://mathworld.wolfram.com/MonotonicFunction.html</rdfs:seeAlso>
        <skos:definition xml:lang="en">A curve is `monotonic` if successive states are ordered either entirely non-decreasing or entirely non-increasing.</skos:definition>
        <skos:altLabel xml:lang="en">monotone</skos:altLabel>
        <skos:altLabel xml:lang="en">monotonic</skos:altLabel>
    </owl:Class>
    <owl:Axiom>
        <owl:annotatedTarget rdf:datatype="&xsd;anyURI">http://mathworld.wolfram.com/MonotonicFunction.html</owl:annotatedTarget>
        <rdfs:comment xml:lang="en">Weisstein, Eric W. Monotonic Function. From MathWorld--A Wolfram Web Resource.</rdfs:comment>
        <owl:annotatedSource rdf:resource="&teddy;TEDDY_0000004"/>
        <owl:annotatedProperty rdf:resource="&rdfs;seeAlso"/>
    </owl:Axiom>
    


    <!-- http://biomodels.net/teddy/TEDDY#TEDDY_0000005 -->

    <owl:Class rdf:about="&teddy;TEDDY_0000005">
        <rdfs:label xml:lang="en">non-monotonic</rdfs:label>
        <owl:equivalentClass>
            <owl:Class>
                <owl:intersectionOf rdf:parseType="Collection">
                    <rdf:Description rdf:about="&teddy;TEDDY_0000144"/>
                    <owl:Class>
                        <owl:complementOf rdf:resource="&teddy;TEDDY_0000004"/>
                    </owl:Class>
                </owl:intersectionOf>
            </owl:Class>
        </owl:equivalentClass>
        <rdfs:subClassOf rdf:resource="&teddy;TEDDY_0000144"/>
        <rdfs:seeAlso rdf:datatype="&xsd;anyURI">http://mathworld.wolfram.com/MonotonicFunction.html</rdfs:seeAlso>
        <skos:definition xml:lang="en">A curve is non-monotonic if it has both increasing ordered successive states and decreasing orderd succesive states.</skos:definition>
    </owl:Class>
    <owl:Axiom>
        <owl:annotatedTarget rdf:datatype="&xsd;anyURI">http://mathworld.wolfram.com/MonotonicFunction.html</owl:annotatedTarget>
        <rdfs:comment xml:lang="en">Weisstein, Eric W. Monotonic Function. From MathWorld--A Wolfram Web Resource.</rdfs:comment>
        <owl:annotatedSource rdf:resource="&teddy;TEDDY_0000005"/>
        <owl:annotatedProperty rdf:resource="&rdfs;seeAlso"/>
    </owl:Axiom>
    


    <!-- http://biomodels.net/teddy/TEDDY#TEDDY_0000006 -->

    <owl:Class rdf:about="&teddy;TEDDY_0000006">
        <rdfs:label xml:lang="en">oscillation</rdfs:label>
        <rdfs:subClassOf rdf:resource="&teddy;TEDDY_0000005"/>
        <owl:disjointWith rdf:resource="&teddy;TEDDY_0000010"/>
        <rdfs:seeAlso rdf:datatype="&xsd;anyURI">http://mathworld.wolfram.com/Oscillation.html</rdfs:seeAlso>
        <skos:definition xml:lang="en">The variation of a function which exhibits slope changes, also called the saltus of a function. A series may also oscillate, causing it not to converge.</skos:definition>
    </owl:Class>
    <owl:Axiom>
        <owl:annotatedTarget rdf:datatype="&xsd;anyURI">http://mathworld.wolfram.com/Oscillation.html</owl:annotatedTarget>
        <rdfs:comment xml:lang="en">Weisstein, Eric W. Oscillation. From MathWorld--A Wolfram Web Resource.</rdfs:comment>
        <owl:annotatedSource rdf:resource="&teddy;TEDDY_0000006"/>
        <owl:annotatedProperty rdf:resource="&rdfs;seeAlso"/>
    </owl:Axiom>
    


    <!-- http://biomodels.net/teddy/TEDDY#TEDDY_0000007 -->

    <owl:Class rdf:about="&teddy;TEDDY_0000007">
        <rdfs:label xml:lang="en">strict monotonicity</rdfs:label>
        <rdfs:subClassOf rdf:resource="&teddy;TEDDY_0000004"/>
        <rdfs:seeAlso rdf:datatype="&xsd;anyURI">http://eom.springer.de/M/m064830.htm</rdfs:seeAlso>
        <skos:definition xml:lang="en">A curve is strictly monotonic if it is monotonic [https://identifiers.org/biomodels.teddy/TEDDY_0000004] and has no equal temporal successive states.</skos:definition>
        <skos:altLabel xml:lang="en">strictly monotone</skos:altLabel>
        <skos:altLabel xml:lang="en">strictly monotonic</skos:altLabel>
        <owl:disjointUnionOf rdf:parseType="Collection">
            <rdf:Description rdf:about="&teddy;TEDDY_0000008"/>
            <rdf:Description rdf:about="&teddy;TEDDY_0000009"/>
        </owl:disjointUnionOf>
    </owl:Class>
    <owl:Axiom>
        <owl:annotatedTarget rdf:datatype="&xsd;anyURI">http://eom.springer.de/M/m064830.htm</owl:annotatedTarget>
        <rdfs:comment xml:lang="en">Weisstein, Eric W. Monotonic Function. From MathWorld--A Wolfram Web Resource.</rdfs:comment>
        <owl:annotatedSource rdf:resource="&teddy;TEDDY_0000007"/>
        <owl:annotatedProperty rdf:resource="&rdfs;seeAlso"/>
    </owl:Axiom>
    


    <!-- http://biomodels.net/teddy/TEDDY#TEDDY_0000008 -->

    <owl:Class rdf:about="&teddy;TEDDY_0000008">
        <rdfs:label xml:lang="en">strictly increasing</rdfs:label>
        <rdfs:subClassOf rdf:resource="&teddy;TEDDY_0000007"/>
        <owl:disjointWith rdf:resource="&teddy;TEDDY_0000009"/>
        <rdfs:seeAlso rdf:datatype="&xsd;anyURI">http://eom.springer.de/M/m064830.htm</rdfs:seeAlso>
        <skos:definition xml:lang="en">A curve is strictly increasing if it is strictly monotonic [https://identifiers.org/biomodels.teddy/TEDDY_0000007] with temporal successive states increasing ordered.</skos:definition>
        <skos:altLabel xml:lang="en">isotonic</skos:altLabel>
    </owl:Class>
    <owl:Axiom>
        <owl:annotatedTarget rdf:datatype="&xsd;anyURI">http://eom.springer.de/M/m064830.htm</owl:annotatedTarget>
        <rdfs:comment xml:lang="en">Weisstein, Eric W. Monotonic Function. From MathWorld--A Wolfram Web Resource.</rdfs:comment>
        <owl:annotatedSource rdf:resource="&teddy;TEDDY_0000008"/>
        <owl:annotatedProperty rdf:resource="&rdfs;seeAlso"/>
    </owl:Axiom>
    


    <!-- http://biomodels.net/teddy/TEDDY#TEDDY_0000009 -->

    <owl:Class rdf:about="&teddy;TEDDY_0000009">
        <rdfs:label xml:lang="en">strictly decreasing</rdfs:label>
        <rdfs:subClassOf rdf:resource="&teddy;TEDDY_0000007"/>
        <rdfs:seeAlso rdf:datatype="&xsd;anyURI">http://eom.springer.de/M/m064830.htm</rdfs:seeAlso>
        <skos:definition xml:lang="en">A curve is strictly decreasing if it is strictly monotonic [https://identifiers.org/biomodels.teddy/TEDDY_0000007] with temporal successive states decreasing ordered.</skos:definition>
        <skos:altLabel xml:lang="en">antitonic</skos:altLabel>
    </owl:Class>
    <owl:Axiom>
        <owl:annotatedTarget rdf:datatype="&xsd;anyURI">http://eom.springer.de/M/m064830.htm</owl:annotatedTarget>
        <rdfs:comment xml:lang="en">Weisstein, Eric W. Monotonic Function. From MathWorld--A Wolfram Web Resource.</rdfs:comment>
        <owl:annotatedSource rdf:resource="&teddy;TEDDY_0000009"/>
        <owl:annotatedProperty rdf:resource="&rdfs;seeAlso"/>
    </owl:Axiom>
    


    <!-- http://biomodels.net/teddy/TEDDY#TEDDY_0000010 -->

    <owl:Class rdf:about="&teddy;TEDDY_0000010">
        <rdfs:label xml:lang="en">single turnaround</rdfs:label>
        <rdfs:subClassOf rdf:resource="&teddy;TEDDY_0000005"/>
        <skos:definition xml:lang="en">A trajectory [https://identifiers.org/biomodels.teddy/TEDDY_0000083] of the system which responds negatively to displacement from equilbrium [https://identifiers.org/biomodels.teddy/TEDDY_0000086]: moving away from equilibrium the trajectory turns around and moves back towards equilibrium.</skos:definition>
    </owl:Class>
    


    <!-- http://biomodels.net/teddy/TEDDY#TEDDY_0000011 -->

    <owl:Class rdf:about="&teddy;TEDDY_0000011">
        <rdfs:label xml:lang="en">steady state ((obsolete))</rdfs:label>
        <rdfs:subClassOf rdf:resource="&teddy;TEDDY_obsolete"/>
        <owl:deprecated rdf:datatype="&xsd;boolean">true</owl:deprecated>
        <skos:definition xml:lang="en">Obsolete: equivalent to TEDDY_0000086 &apos;Fixed Point&apos;.</skos:definition>
    </owl:Class>
    


    <!-- http://biomodels.net/teddy/TEDDY#TEDDY_0000012 -->

    <owl:Class rdf:about="&teddy;TEDDY_0000012">
        <rdfs:label xml:lang="en">rate of change</rdfs:label>
        <rdfs:subClassOf rdf:resource="&teddy;TEDDY_0000023"/>
        <skos:definition xml:lang="en">The rate of growth/decay.</skos:definition>
    </owl:Class>
    


    <!-- http://biomodels.net/teddy/TEDDY#TEDDY_0000013 -->

    <owl:Class rdf:about="&teddy;TEDDY_0000013">
        <rdfs:label xml:lang="en">linear rate of change</rdfs:label>
        <rdfs:subClassOf rdf:resource="&teddy;TEDDY_0000018"/>
        <owl:disjointWith rdf:resource="&teddy;TEDDY_0000017"/>
        <rdfs:seeAlso rdf:datatype="&xsd;anyURI">https://identifiers.org/isbn/1844071448</rdfs:seeAlso>
        <skos:definition xml:lang="en">A quantity changes linearly when its change is a constant amount over a given period of time. </skos:definition>
    </owl:Class>
    <owl:Axiom>
        <owl:annotatedTarget rdf:datatype="&xsd;anyURI">https://identifiers.org/isbn/1844071448</owl:annotatedTarget>
        <rdfs:comment xml:lang="en">D. H. Meadows (2005) The Limits to Growth: The 30-Year Update, Rff Press, revised ed.</rdfs:comment>
        <owl:annotatedSource rdf:resource="&teddy;TEDDY_0000013"/>
        <owl:annotatedProperty rdf:resource="&rdfs;seeAlso"/>
    </owl:Axiom>
    


    <!-- http://biomodels.net/teddy/TEDDY#TEDDY_0000014 -->

    <owl:Class rdf:about="&teddy;TEDDY_0000014">
        <rdfs:label xml:lang="en">exponential rate of change</rdfs:label>
        <rdfs:subClassOf rdf:resource="&teddy;TEDDY_0000012"/>
        <owl:disjointWith rdf:resource="&teddy;TEDDY_0000018"/>
        <rdfs:seeAlso rdf:datatype="&xsd;anyURI">https://identifiers.org/isbn/1844071448</rdfs:seeAlso>
        <skos:definition xml:lang="en">A quantity changes exponentially when its change over a given period of time is proportional to what is already there.</skos:definition>
    </owl:Class>
    <owl:Axiom>
        <owl:annotatedTarget rdf:datatype="&xsd;anyURI">https://identifiers.org/isbn/1844071448</owl:annotatedTarget>
        <rdfs:comment xml:lang="en">D. H. Meadows (2005) The Limits to Growth: The 30-Year Update, Rff Press, revised ed.</rdfs:comment>
        <owl:annotatedSource rdf:resource="&teddy;TEDDY_0000014"/>
        <owl:annotatedProperty rdf:resource="&rdfs;seeAlso"/>
    </owl:Axiom>
    


    <!-- http://biomodels.net/teddy/TEDDY#TEDDY_0000015 -->

    <owl:Class rdf:about="&teddy;TEDDY_0000015">
        <rdfs:label xml:lang="en">curve shape</rdfs:label>
        <rdfs:subClassOf rdf:resource="&teddy;TEDDY_0000023"/>
        <skos:definition xml:lang="en">Characteristic describing the shape of the graph of a function.</skos:definition>
    </owl:Class>
    


    <!-- http://biomodels.net/teddy/TEDDY#TEDDY_0000016 -->

    <owl:Class rdf:about="&teddy;TEDDY_0000016">
        <rdfs:label xml:lang="en">concave shape</rdfs:label>
        <rdfs:subClassOf rdf:resource="&teddy;TEDDY_0000015"/>
        <owl:disjointWith rdf:resource="&teddy;TEDDY_0000032"/>
        <rdfs:seeAlso rdf:datatype="&xsd;anyURI">https://identifiers.org/isbn/0691080690</rdfs:seeAlso>
        <skos:definition xml:lang="en">A shape of a graph of a concave function, i.e. a function whose negative is convex [https://identifiers.org/biomodels.teddy/TEDDY_0000021].</skos:definition>
    </owl:Class>
    <owl:Axiom>
        <owl:annotatedTarget rdf:datatype="&xsd;anyURI">https://identifiers.org/isbn/0691080690</owl:annotatedTarget>
        <rdfs:comment xml:lang="en">R. T. Rockafellar (1970) Convex Analysis (Princeton Mathematical Series), Princeton Univ Pr. (p.23)</rdfs:comment>
        <owl:annotatedSource rdf:resource="&teddy;TEDDY_0000016"/>
        <owl:annotatedProperty rdf:resource="&rdfs;seeAlso"/>
    </owl:Axiom>
    


    <!-- http://biomodels.net/teddy/TEDDY#TEDDY_0000017 -->

    <owl:Class rdf:about="&teddy;TEDDY_0000017">
        <rdfs:label xml:lang="en">zero rate of change</rdfs:label>
        <rdfs:subClassOf rdf:resource="&teddy;TEDDY_0000018"/>
        <rdfs:seeAlso rdf:datatype="&xsd;anyURI">https://identifiers.org/isbn/1844071448</rdfs:seeAlso>
        <skos:definition xml:lang="en">A quantity has a zero rate of change when it neither grows nor declines.</skos:definition>
    </owl:Class>
    <owl:Axiom>
        <owl:annotatedTarget rdf:datatype="&xsd;anyURI">https://identifiers.org/isbn/1844071448</owl:annotatedTarget>
        <rdfs:comment xml:lang="en">D. H. Meadows (2005) The Limits to Growth: The 30-Year Update, Rff Press, revised ed.</rdfs:comment>
        <owl:annotatedSource rdf:resource="&teddy;TEDDY_0000017"/>
        <owl:annotatedProperty rdf:resource="&rdfs;seeAlso"/>
    </owl:Axiom>
    


    <!-- http://biomodels.net/teddy/TEDDY#TEDDY_0000018 -->

    <owl:Class rdf:about="&teddy;TEDDY_0000018">
        <rdfs:label xml:lang="en">polynomial rate of change</rdfs:label>
        <rdfs:subClassOf rdf:resource="&teddy;TEDDY_0000012"/>
        <skos:definition xml:lang="en">A quantity changes polynomially when its change function is bounded above by a polinomial function.</skos:definition>
        <skos:altLabel xml:lang="en">power rate of change</skos:altLabel>
    </owl:Class>
    


    <!-- http://biomodels.net/teddy/TEDDY#TEDDY_0000019 -->

    <owl:Class rdf:about="&teddy;TEDDY_0000019">
        <rdfs:label xml:lang="en">linear increasing</rdfs:label>
        <owl:equivalentClass>
            <owl:Class>
                <owl:intersectionOf rdf:parseType="Collection">
                    <rdf:Description rdf:about="&teddy;TEDDY_0000008"/>
                    <owl:Restriction>
                        <owl:onProperty rdf:resource="&teddy;TR_0004"/>
                        <owl:someValuesFrom rdf:resource="&teddy;TEDDY_0000013"/>
                    </owl:Restriction>
                </owl:intersectionOf>
            </owl:Class>
        </owl:equivalentClass>
        <skos:definition xml:lang="en">A curve is linear increasing if it is is strictly increasing with a linear rate of change.</skos:definition>
    </owl:Class>
    


    <!-- http://biomodels.net/teddy/TEDDY#TEDDY_0000020 -->

    <owl:Class rdf:about="&teddy;TEDDY_0000020">
        <rdfs:label xml:lang="en">linear decreasing</rdfs:label>
        <owl:equivalentClass>
            <owl:Class>
                <owl:intersectionOf rdf:parseType="Collection">
                    <rdf:Description rdf:about="&teddy;TEDDY_0000009"/>
                    <owl:Restriction>
                        <owl:onProperty rdf:resource="&teddy;TR_0004"/>
                        <owl:someValuesFrom rdf:resource="&teddy;TEDDY_0000013"/>
                    </owl:Restriction>
                </owl:intersectionOf>
            </owl:Class>
        </owl:equivalentClass>
        <skos:definition xml:lang="en">A curve is linear decreasing if it is is strictly decreasing with a linear rate of change.</skos:definition>
    </owl:Class>
    


    <!-- http://biomodels.net/teddy/TEDDY#TEDDY_0000021 -->

    <owl:Class rdf:about="&teddy;TEDDY_0000021">
        <rdfs:label xml:lang="en">convex shape</rdfs:label>
        <rdfs:subClassOf rdf:resource="&teddy;TEDDY_0000015"/>
        <owl:disjointWith rdf:resource="&teddy;TEDDY_0000032"/>
        <rdfs:seeAlso rdf:datatype="&xsd;anyURI">https://identifiers.org/isbn/0691080690</rdfs:seeAlso>
        <owl:deprecated xml:lang="en">A shape of a graph of a convex function, i.e. a function whose epigraph (the set of points on or above the graph of the function) is a convex as a subset of R^n. A subset G of a linear space is said to be convex, if it contains the whole segment (closed straight line segment) joining each of its two points.</owl:deprecated>
    </owl:Class>
    <owl:Axiom>
        <owl:annotatedTarget rdf:datatype="&xsd;anyURI">https://identifiers.org/isbn/0691080690</owl:annotatedTarget>
        <rdfs:comment xml:lang="en">R. T. Rockafellar (1970) Convex Analysis (Princeton Mathematical Series), Princeton Univ Pr. (p.10, 23)</rdfs:comment>
        <owl:annotatedSource rdf:resource="&teddy;TEDDY_0000021"/>
        <owl:annotatedProperty rdf:resource="&rdfs;seeAlso"/>
    </owl:Axiom>
    


    <!-- http://biomodels.net/teddy/TEDDY#TEDDY_0000022 -->

    <owl:Class rdf:about="&teddy;TEDDY_0000022">
        <rdfs:label xml:lang="en">straight line shape</rdfs:label>
        <owl:equivalentClass>
            <owl:Class>
                <owl:intersectionOf rdf:parseType="Collection">
                    <rdf:Description rdf:about="&teddy;TEDDY_0000016"/>
                    <rdf:Description rdf:about="&teddy;TEDDY_0000021"/>
                </owl:intersectionOf>
            </owl:Class>
        </owl:equivalentClass>
        <skos:definition xml:lang="en">A shape of a graph of a linear function.</skos:definition>
    </owl:Class>
    


    <!-- http://biomodels.net/teddy/TEDDY#TEDDY_0000023 -->

    <owl:Class rdf:about="&teddy;TEDDY_0000023">
        <rdfs:label xml:lang="en">curve characteristic</rdfs:label>
        <rdfs:subClassOf rdf:resource="&teddy;TEDDY_0000002"/>
        <skos:definition xml:lang="en">A characteristic of the &apos;temporal behaviour&apos; [https://identifiers.org/biomodels.teddy/TEDDY_0000083] curve (projection of the function graph onto a single variable).</skos:definition>
    </owl:Class>
    


    <!-- http://biomodels.net/teddy/TEDDY#TEDDY_0000024 -->

    <owl:Class rdf:about="&teddy;TEDDY_0000024">
        <rdfs:label xml:lang="en">unbounded growth ((obsolete))</rdfs:label>
        <rdfs:subClassOf rdf:resource="&teddy;TEDDY_obsolete"/>
        <owl:deprecated rdf:datatype="&xsd;boolean">true</owl:deprecated>
    </owl:Class>
    


    <!-- http://biomodels.net/teddy/TEDDY#TEDDY_0000025 -->

    <owl:Class rdf:about="&teddy;TEDDY_0000025">
        <rdfs:label xml:lang="en">limit</rdfs:label>
        <rdfs:subClassOf rdf:resource="&teddy;TEDDY_0000023"/>
        <rdfs:seeAlso rdf:datatype="&xsd;anyURI">http://eom.springer.de/L/l058820.htm</rdfs:seeAlso>
        <skos:definition xml:lang="en">One of the fundamental concepts in mathematics, meaning that a variable depending on another variable arbitrary closely approaches some constant as the latter variable changes in a definite manner.</skos:definition>
    </owl:Class>
    <owl:Axiom>
        <owl:annotatedTarget rdf:datatype="&xsd;anyURI">http://eom.springer.de/L/l058820.htm</owl:annotatedTarget>
        <rdfs:comment xml:lang="en">Encyclopaedia of Mathematics, edited by Michiel Hazewinkel, CWI, Amsterdam.</rdfs:comment>
        <owl:annotatedSource rdf:resource="&teddy;TEDDY_0000025"/>
        <owl:annotatedProperty rdf:resource="&rdfs;seeAlso"/>
    </owl:Axiom>
    


    <!-- http://biomodels.net/teddy/TEDDY#TEDDY_0000026 -->

    <owl:Class rdf:about="&teddy;TEDDY_0000026">
        <rdfs:label xml:lang="en">asymptotic limit</rdfs:label>
        <rdfs:subClassOf rdf:resource="&teddy;TEDDY_0000025"/>
        <rdfs:seeAlso rdf:datatype="&xsd;anyURI">http://eom.springer.de/a/a012870.htm</rdfs:seeAlso>
        <skos:definition xml:lang="en">A limit of a function f(x) as x-&gt;x0 over a set E for which x0 is a density point.</skos:definition>
        <skos:altLabel xml:lang="en">approximate limit</skos:altLabel>
    </owl:Class>
    <owl:Axiom>
        <owl:annotatedTarget rdf:datatype="&xsd;anyURI">http://eom.springer.de/a/a012870.htm</owl:annotatedTarget>
        <rdfs:comment xml:lang="en">Encyclopaedia of Mathematics, edited by Michiel Hazewinkel, CWI, Amsterdam.</rdfs:comment>
        <owl:annotatedSource rdf:resource="&teddy;TEDDY_0000026"/>
        <owl:annotatedProperty rdf:resource="&rdfs;seeAlso"/>
    </owl:Axiom>
    


    <!-- http://biomodels.net/teddy/TEDDY#TEDDY_0000027 -->

    <owl:Class rdf:about="&teddy;TEDDY_0000027">
        <rdfs:label xml:lang="en">asymptotic upper limit</rdfs:label>
        <rdfs:subClassOf rdf:resource="&teddy;TEDDY_0000026"/>
        <rdfs:seeAlso rdf:datatype="&xsd;anyURI">http://eom.springer.de/a/a012870.htm</rdfs:seeAlso>
        <skos:definition xml:lang="en">An approximate upper limit of a function f(x) at a point x0 is the lower bound of the set of numbers y (including y=positive infinity) for which x0 is a point of dispersion of the set {x: f(x)&gt;y}.</skos:definition>
        <skos:altLabel xml:lang="en">approximate upper limit</skos:altLabel>
    </owl:Class>
    <owl:Axiom>
        <owl:annotatedTarget rdf:datatype="&xsd;anyURI">http://eom.springer.de/a/a012870.htm</owl:annotatedTarget>
        <rdfs:comment xml:lang="en">Encyclopaedia of Mathematics, edited by Michiel Hazewinkel, CWI, Amsterdam.</rdfs:comment>
        <owl:annotatedSource rdf:resource="&teddy;TEDDY_0000027"/>
        <owl:annotatedProperty rdf:resource="&rdfs;seeAlso"/>
    </owl:Axiom>
    


    <!-- http://biomodels.net/teddy/TEDDY#TEDDY_0000028 -->

    <owl:Class rdf:about="&teddy;TEDDY_0000028">
        <rdfs:label xml:lang="en">asymptotic lower limit</rdfs:label>
        <rdfs:subClassOf rdf:resource="&teddy;TEDDY_0000026"/>
        <rdfs:seeAlso rdf:datatype="&xsd;anyURI">http://eom.springer.de/a/a012870.htm</rdfs:seeAlso>
        <skos:definition xml:lang="en">An approximate lower limit of a function f(x) at a point x0 is the upper bound of the set of numbers y (including y=negative infinity) for which x0 is a point of dispersion of the set {x: f(x)&lt;y}.</skos:definition>
        <skos:altLabel xml:lang="en">approximate lower limit</skos:altLabel>
    </owl:Class>
    <owl:Axiom>
        <owl:annotatedTarget rdf:datatype="&xsd;anyURI">http://eom.springer.de/a/a012870.htm</owl:annotatedTarget>
        <rdfs:comment xml:lang="en">Encyclopaedia of Mathematics, edited by Michiel Hazewinkel, CWI, Amsterdam.</rdfs:comment>
        <owl:annotatedSource rdf:resource="&teddy;TEDDY_0000028"/>
        <owl:annotatedProperty rdf:resource="&rdfs;seeAlso"/>
    </owl:Axiom>
    


    <!-- http://biomodels.net/teddy/TEDDY#TEDDY_0000029 -->

    <owl:Class rdf:about="&teddy;TEDDY_0000029">
        <rdfs:label xml:lang="en">plus infinity limit</rdfs:label>
        <rdfs:subClassOf rdf:resource="&teddy;TEDDY_0000030"/>
        <owl:disjointWith rdf:resource="&teddy;TEDDY_0000031"/>
        <rdfs:seeAlso rdf:datatype="&xsd;anyURI">http://eom.springer.de/I/i050930.htm</rdfs:seeAlso>
        <skos:definition xml:lang="en">A function of x approaches plus infinity if its value becomes and remains larger than any given number as a result of variation of x.</skos:definition>
    </owl:Class>
    <owl:Axiom>
        <owl:annotatedTarget rdf:datatype="&xsd;anyURI">http://eom.springer.de/I/i050930.htm</owl:annotatedTarget>
        <rdfs:comment xml:lang="en">Encyclopaedia of Mathematics, edited by Michiel Hazewinkel, CWI, Amsterdam.</rdfs:comment>
        <owl:annotatedSource rdf:resource="&teddy;TEDDY_0000029"/>
        <owl:annotatedProperty rdf:resource="&rdfs;seeAlso"/>
    </owl:Axiom>
    


    <!-- http://biomodels.net/teddy/TEDDY#TEDDY_0000030 -->

    <owl:Class rdf:about="&teddy;TEDDY_0000030">
        <rdfs:label xml:lang="en">infinite limit</rdfs:label>
        <rdfs:subClassOf rdf:resource="&teddy;TEDDY_0000025"/>
        <rdfs:seeAlso rdf:datatype="&xsd;anyURI">http://eom.springer.de/I/i050930.htm</rdfs:seeAlso>
        <skos:definition xml:lang="en">A function of a variable x has an infinite limit if its absolute value becomes and remains larger than any given number as a result of variation of x.</skos:definition>
    </owl:Class>
    <owl:Axiom>
        <owl:annotatedTarget rdf:datatype="&xsd;anyURI">http://eom.springer.de/I/i050930.htm</owl:annotatedTarget>
        <rdfs:comment xml:lang="en">Encyclopaedia of Mathematics, edited by Michiel Hazewinkel, CWI, Amsterdam.</rdfs:comment>
        <owl:annotatedSource rdf:resource="&teddy;TEDDY_0000030"/>
        <owl:annotatedProperty rdf:resource="&rdfs;seeAlso"/>
    </owl:Axiom>
    


    <!-- http://biomodels.net/teddy/TEDDY#TEDDY_0000031 -->

    <owl:Class rdf:about="&teddy;TEDDY_0000031">
        <rdfs:label xml:lang="en">minus infinity limit</rdfs:label>
        <rdfs:subClassOf rdf:resource="&teddy;TEDDY_0000030"/>
        <rdfs:seeAlso rdf:datatype="&xsd;anyURI">http://eom.springer.de/I/i050930.htm</rdfs:seeAlso>
        <skos:definition xml:lang="en">A function of x approaches minus infinity if its value becomes and remains smaller than any given number as a result of variation of x.</skos:definition>
    </owl:Class>
    <owl:Axiom>
        <owl:annotatedTarget rdf:datatype="&xsd;anyURI">http://eom.springer.de/I/i050930.htm</owl:annotatedTarget>
        <rdfs:comment xml:lang="en">Encyclopaedia of Mathematics, edited by Michiel Hazewinkel, CWI, Amsterdam.</rdfs:comment>
        <owl:annotatedSource rdf:resource="&teddy;TEDDY_0000031"/>
        <owl:annotatedProperty rdf:resource="&rdfs;seeAlso"/>
    </owl:Axiom>
    


    <!-- http://biomodels.net/teddy/TEDDY#TEDDY_0000032 -->

    <owl:Class rdf:about="&teddy;TEDDY_0000032">
        <rdfs:label xml:lang="en">sigmoid shape</rdfs:label>
        <rdfs:subClassOf rdf:resource="&teddy;TEDDY_0000015"/>
        <rdfs:subClassOf>
            <owl:Restriction>
                <owl:onProperty rdf:resource="&ro;has_part"/>
                <owl:someValuesFrom rdf:resource="&teddy;TEDDY_0000021"/>
            </owl:Restriction>
        </rdfs:subClassOf>
        <rdfs:subClassOf>
            <owl:Restriction>
                <owl:onProperty rdf:resource="&ro;has_part"/>
                <owl:someValuesFrom rdf:resource="&teddy;TEDDY_0000016"/>
            </owl:Restriction>
        </rdfs:subClassOf>
        <rdfs:seeAlso rdf:datatype="&xsd;anyURI">https://identifiers.org/isbn/3540605053</rdfs:seeAlso>
        <skos:definition xml:lang="en">A shape of a graph of a sigmoid function, i.e. a real function sc: R-&gt;(0,1) defined by the expression sc(x) = 1/(1 + e^(-cx)). </skos:definition>
    </owl:Class>
    <owl:Axiom>
        <owl:annotatedTarget rdf:datatype="&xsd;anyURI">https://identifiers.org/isbn/3540605053</owl:annotatedTarget>
        <rdfs:comment xml:lang="en">R. Rojas (1996) Neural Networks: A Systematic Introduction, Springer, 1st ed. (p.149)</rdfs:comment>
        <owl:annotatedSource rdf:resource="&teddy;TEDDY_0000032"/>
        <owl:annotatedProperty rdf:resource="&rdfs;seeAlso"/>
    </owl:Axiom>
    


    <!-- http://biomodels.net/teddy/TEDDY#TEDDY_0000033 -->

    <owl:Class rdf:about="&teddy;TEDDY_0000033">
        <rdfs:label xml:lang="en">feedback loop</rdfs:label>
        <rdfs:subClassOf rdf:resource="&teddy;TEDDY_0000003"/>
        <owl:disjointWith rdf:resource="&teddy;TEDDY_0000036"/>
        <rdfs:seeAlso rdf:datatype="&xsd;anyURI">https://identifiers.org/isbn/1584886420</rdfs:seeAlso>
        <skos:definition xml:lang="en">A process whereby some proportion of function of the output signal of a system is passed (fed back) to the input.</skos:definition>
        <skos:altLabel xml:lang="en">feedback</skos:altLabel>
    </owl:Class>
    <owl:Axiom>
        <rdfs:comment rdf:datatype="&xsd;anyURI">Alon U (2006) An Introduction to Systems Biology: Design Principles of Biological Circuits, Chapman and Hall/CRC. (p.266)</rdfs:comment>
        <owl:annotatedTarget rdf:datatype="&xsd;anyURI">https://identifiers.org/isbn/1584886420</owl:annotatedTarget>
        <owl:annotatedSource rdf:resource="&teddy;TEDDY_0000033"/>
        <owl:annotatedProperty rdf:resource="&rdfs;seeAlso"/>
    </owl:Axiom>
    


    <!-- http://biomodels.net/teddy/TEDDY#TEDDY_0000034 -->

    <owl:Class rdf:about="&teddy;TEDDY_0000034">
        <rdfs:label xml:lang="en">negative feedback loop</rdfs:label>
        <rdfs:subClassOf rdf:resource="&teddy;TEDDY_0000033"/>
        <owl:disjointWith rdf:resource="&teddy;TEDDY_0000035"/>
        <rdfs:seeAlso rdf:datatype="&xsd;anyURI">https://identifiers.org/doi/10.1016/j.febslet.2005.02.008</rdfs:seeAlso>
        <skos:definition xml:lang="en">A component or variable of a system is subject to negative feedback when it inhibits its own level of activity.</skos:definition>
        <skos:altLabel xml:lang="en">negative feedback</skos:altLabel>
    </owl:Class>
    <owl:Axiom>
        <owl:annotatedTarget rdf:datatype="&xsd;anyURI">https://identifiers.org/doi/10.1016/j.febslet.2005.02.008</owl:annotatedTarget>
        <rdfs:comment xml:lang="en">Wolkenhauer O, Ullah M, Wellstead P, Cho K-H (2005) The dynamic systems approach to control and regulation of intracellular networks, FEBS Letters, 579 (8): 1846-1853.</rdfs:comment>
        <owl:annotatedSource rdf:resource="&teddy;TEDDY_0000034"/>
        <owl:annotatedProperty rdf:resource="&rdfs;seeAlso"/>
    </owl:Axiom>
    


    <!-- http://biomodels.net/teddy/TEDDY#TEDDY_0000035 -->

    <owl:Class rdf:about="&teddy;TEDDY_0000035">
        <rdfs:label xml:lang="en">positive feedback loop</rdfs:label>
        <rdfs:subClassOf rdf:resource="&teddy;TEDDY_0000033"/>
        <rdfs:seeAlso rdf:datatype="&xsd;anyURI">https://identifiers.org/doi/10.1016/j.febslet.2005.02.008</rdfs:seeAlso>
        <skos:definition xml:lang="en">A component or variable of a system is subject to positive feedback when it increases its own level of activity.</skos:definition>
        <skos:altLabel xml:lang="en">positive feedback</skos:altLabel>
    </owl:Class>
    <owl:Axiom>
        <owl:annotatedTarget rdf:datatype="&xsd;anyURI">https://identifiers.org/doi/10.1016/j.febslet.2005.02.008</owl:annotatedTarget>
        <rdfs:comment xml:lang="en">Wolkenhauer O, Ullah M, Wellstead P, Cho K-H (2005) The dynamic systems approach to control and regulation of intracellular networks, FEBS Letters, 579 (8): 1846-1853.</rdfs:comment>
        <owl:annotatedSource rdf:resource="&teddy;TEDDY_0000035"/>
        <owl:annotatedProperty rdf:resource="&rdfs;seeAlso"/>
    </owl:Axiom>
    


    <!-- http://biomodels.net/teddy/TEDDY#TEDDY_0000036 -->

    <owl:Class rdf:about="&teddy;TEDDY_0000036">
        <rdfs:label xml:lang="en">feed-forward loop</rdfs:label>
        <rdfs:subClassOf rdf:resource="&teddy;TEDDY_0000003"/>
        <skos:definition xml:lang="en">A &apos;three-node feed-forward loop&apos; [https://identifiers.org/biomodels.teddy/TEDDY_0000037] or its topological generalization.</skos:definition>
        <skos:altLabel xml:lang="en">FFL</skos:altLabel>
        <skos:altLabel xml:lang="en">feed-forward</skos:altLabel>
        <skos:altLabel xml:lang="en">feedforward</skos:altLabel>
        <skos:altLabel xml:lang="en">feedforward loop</skos:altLabel>
    </owl:Class>
    


    <!-- http://biomodels.net/teddy/TEDDY#TEDDY_0000037 -->

    <owl:Class rdf:about="&teddy;TEDDY_0000037">
        <rdfs:label xml:lang="en">three-node feed-forward loop</rdfs:label>
        <rdfs:subClassOf rdf:resource="&teddy;TEDDY_0000036"/>
        <owl:disjointWith rdf:resource="&teddy;TEDDY_0000165"/>
        <rdfs:seeAlso rdf:datatype="&xsd;anyURI">https://identifiers.org/isbn/1584886420</rdfs:seeAlso>
        <skos:altLabel xml:lang="en">3-node FFL</skos:altLabel>
        <skos:altLabel xml:lang="en">3-node feed-forward</skos:altLabel>
        <skos:altLabel xml:lang="en">3-node feed-forward loop</skos:altLabel>
        <skos:altLabel xml:lang="en">3-node feedforward</skos:altLabel>
        <skos:altLabel xml:lang="en">3-node feedforward loop</skos:altLabel>
        <skos:definition xml:lang="en">A pattern with three nodes, X, Y, and Z, in which X has a directed edge to Y and Z, and Y has a directed edge to Z. The FFL is a network motif in many biological networks, and can perform a variety of tasks (such as sign-sensitive delay, sign-sensitive acceleration, and pulse generation).</skos:definition>
        <skos:altLabel xml:lang="en">FFL</skos:altLabel>
        <skos:altLabel xml:lang="en">thre-node FFL</skos:altLabel>
        <skos:altLabel xml:lang="en">three-node feedforward loop</skos:altLabel>
    </owl:Class>
    <owl:Axiom>
        <rdfs:comment rdf:datatype="&xsd;anyURI">Alon U (2006) An Introduction to Systems Biology: Design Principles of Biological Circuits, Chapman and Hall/CRC. (p.267)</rdfs:comment>
        <owl:annotatedTarget rdf:datatype="&xsd;anyURI">https://identifiers.org/isbn/1584886420</owl:annotatedTarget>
        <owl:annotatedSource rdf:resource="&teddy;TEDDY_0000037"/>
        <owl:annotatedProperty rdf:resource="&rdfs;seeAlso"/>
    </owl:Axiom>
    <owl:Axiom>
        <owl:annotatedTarget xml:lang="en">FFL</owl:annotatedTarget>
        <rdfs:seeAlso xml:lang="en">https://identifiers.org/isbn/1584886420 (p.41)</rdfs:seeAlso>
        <owl:annotatedSource rdf:resource="&teddy;TEDDY_0000037"/>
        <owl:annotatedProperty rdf:resource="&skos;altLabel"/>
    </owl:Axiom>
    


    <!-- http://biomodels.net/teddy/TEDDY#TEDDY_0000038 -->

    <owl:Class rdf:about="&teddy;TEDDY_0000038">
        <rdfs:label xml:lang="en">coherent three-node feed-forward loop</rdfs:label>
        <rdfs:subClassOf rdf:resource="&teddy;TEDDY_0000037"/>
        <owl:disjointWith rdf:resource="&teddy;TEDDY_0000043"/>
        <rdfs:seeAlso rdf:datatype="&xsd;anyURI">https://identifiers.org/isbn/1584886420</rdfs:seeAlso>
        <skos:definition xml:lang="en">A feed-forward loop [https://identifiers.org/biomodels.teddy/TEDDY_0000037] in which the sign of the direct path from X to Z is the same as the overall sign of the indirect path from X through Y to Z.</skos:definition>
        <skos:altLabel xml:lang="en">coherent 3-node feed-forward loop</skos:altLabel>
        <skos:altLabel xml:lang="en">coherent 3-node feedforward</skos:altLabel>
        <skos:altLabel xml:lang="en">coherent 3-node feedforward loop</skos:altLabel>
        <skos:altLabel xml:lang="en">coherent three-node feedforward loop</skos:altLabel>
    </owl:Class>
    <owl:Axiom>
        <owl:annotatedTarget rdf:datatype="&xsd;anyURI">https://identifiers.org/isbn/1584886420</owl:annotatedTarget>
        <rdfs:comment xml:lang="en">Alon U (2006) An Introduction to Systems Biology: Design Principles of Biological Circuits, Chapman and Hall/CRC. (p.265)</rdfs:comment>
        <owl:annotatedSource rdf:resource="&teddy;TEDDY_0000038"/>
        <owl:annotatedProperty rdf:resource="&rdfs;seeAlso"/>
    </owl:Axiom>
    


    <!-- http://biomodels.net/teddy/TEDDY#TEDDY_0000039 -->

    <owl:Class rdf:about="&teddy;TEDDY_0000039">
        <rdfs:label xml:lang="en">type-1 coherent three-node feed-forward loop</rdfs:label>
        <rdfs:subClassOf rdf:resource="&teddy;TEDDY_0000038"/>
        <rdfs:seeAlso rdf:datatype="&xsd;anyURI">https://identifiers.org/isbn/1584886420</rdfs:seeAlso>
        <skos:definition xml:lang="en">A &apos;coherent three-node feed-forward loop&apos; [https://identifiers.org/biomodels.teddy/TEDDY_0000038] in which all three regulations are positive.</skos:definition>
        <skos:altLabel xml:lang="en">C1-FFL</skos:altLabel>
        <skos:altLabel xml:lang="en">coherent 3-node feedforward type-1</skos:altLabel>
        <skos:altLabel xml:lang="en">type-1 coherent FFL</skos:altLabel>
    </owl:Class>
    <owl:Axiom>
        <owl:annotatedTarget rdf:datatype="&xsd;anyURI">https://identifiers.org/isbn/1584886420</owl:annotatedTarget>
        <rdfs:comment xml:lang="en">Alon U (2006) An Introduction to Systems Biology: Design Principles of Biological Circuits, Chapman and Hall/CRC. (p.47)</rdfs:comment>
        <owl:annotatedSource rdf:resource="&teddy;TEDDY_0000039"/>
        <owl:annotatedProperty rdf:resource="&rdfs;seeAlso"/>
    </owl:Axiom>
    


    <!-- http://biomodels.net/teddy/TEDDY#TEDDY_0000040 -->

    <owl:Class rdf:about="&teddy;TEDDY_0000040">
        <rdfs:label xml:lang="en">type-2 coherent three-node feed-forward loop</rdfs:label>
        <rdfs:subClassOf rdf:resource="&teddy;TEDDY_0000038"/>
        <rdfs:seeAlso rdf:datatype="&xsd;anyURI">https://identifiers.org/isbn/1584886420</rdfs:seeAlso>
        <skos:definition xml:lang="en">A &apos;coherent three-node feed-forward loop&apos; [https://identifiers.org/biomodels.teddy/TEDDY_0000038] in which X represses Z, and also represses an activator of Z.</skos:definition>
        <skos:altLabel xml:lang="en">C2-FFL</skos:altLabel>
        <skos:altLabel xml:lang="en">coherent 3-node feedforward type-2</skos:altLabel>
        <skos:altLabel xml:lang="en">type-2 coherent FFL</skos:altLabel>
    </owl:Class>
    <owl:Axiom>
        <owl:annotatedTarget rdf:datatype="&xsd;anyURI">https://identifiers.org/isbn/1584886420</owl:annotatedTarget>
        <rdfs:comment xml:lang="en">Alon U (2006) An Introduction to Systems Biology: Design Principles of Biological Circuits, Chapman and Hall/CRC. (p.47)</rdfs:comment>
        <owl:annotatedSource rdf:resource="&teddy;TEDDY_0000040"/>
        <owl:annotatedProperty rdf:resource="&rdfs;seeAlso"/>
    </owl:Axiom>
    


    <!-- http://biomodels.net/teddy/TEDDY#TEDDY_0000041 -->

    <owl:Class rdf:about="&teddy;TEDDY_0000041">
        <rdfs:label xml:lang="en">type-3 coherent three-node feed-forward loop</rdfs:label>
        <rdfs:subClassOf rdf:resource="&teddy;TEDDY_0000038"/>
        <rdfs:seeAlso rdf:datatype="&xsd;anyURI">https://identifiers.org/isbn/1584886420</rdfs:seeAlso>
        <skos:definition xml:lang="en">A &apos;coherent three-node feed-forward loop&apos; [https://identifiers.org/biomodels.teddy/TEDDY_0000038] in which X represses Z, and also activates a repressor of Z.</skos:definition>
        <skos:altLabel xml:lang="en">C3-FFL</skos:altLabel>
        <skos:altLabel xml:lang="en">coherent 3-node feedforward type-3</skos:altLabel>
        <skos:altLabel xml:lang="en">type-3 coherent FFL</skos:altLabel>
    </owl:Class>
    <owl:Axiom>
        <owl:annotatedTarget rdf:datatype="&xsd;anyURI">https://identifiers.org/isbn/1584886420</owl:annotatedTarget>
        <rdfs:comment xml:lang="en">Alon U (2006) An Introduction to Systems Biology: Design Principles of Biological Circuits, Chapman and Hall/CRC. (p.47)</rdfs:comment>
        <owl:annotatedSource rdf:resource="&teddy;TEDDY_0000041"/>
        <owl:annotatedProperty rdf:resource="&rdfs;seeAlso"/>
    </owl:Axiom>
    


    <!-- http://biomodels.net/teddy/TEDDY#TEDDY_0000042 -->

    <owl:Class rdf:about="&teddy;TEDDY_0000042">
        <rdfs:label xml:lang="en">type-4 coherent three-node feed-forward loop</rdfs:label>
        <rdfs:subClassOf rdf:resource="&teddy;TEDDY_0000038"/>
        <rdfs:seeAlso rdf:datatype="&xsd;anyURI">https://identifiers.org/isbn/1584886420</rdfs:seeAlso>
        <skos:definition xml:lang="en">A &apos;coherent three-node feed-forward loop&apos; [https://identifiers.org/biomodels.teddy/TEDDY_0000038] in which X activates Z, and also represses a repressor of Z.</skos:definition>
        <skos:altLabel xml:lang="en">C4-FFL</skos:altLabel>
        <skos:altLabel xml:lang="en">coherent 3-node feedforward type-4</skos:altLabel>
        <skos:altLabel xml:lang="en">type-4 coherent FFL</skos:altLabel>
    </owl:Class>
    <owl:Axiom>
        <owl:annotatedTarget rdf:datatype="&xsd;anyURI">https://identifiers.org/isbn/1584886420</owl:annotatedTarget>
        <rdfs:comment xml:lang="en">Alon U (2006) An Introduction to Systems Biology: Design Principles of Biological Circuits, Chapman and Hall/CRC. (p.47)</rdfs:comment>
        <owl:annotatedSource rdf:resource="&teddy;TEDDY_0000042"/>
        <owl:annotatedProperty rdf:resource="&rdfs;seeAlso"/>
    </owl:Axiom>
    


    <!-- http://biomodels.net/teddy/TEDDY#TEDDY_0000043 -->

    <owl:Class rdf:about="&teddy;TEDDY_0000043">
        <rdfs:label xml:lang="en">incoherent three-node feed-forward loop</rdfs:label>
        <rdfs:subClassOf rdf:resource="&teddy;TEDDY_0000037"/>
        <rdfs:seeAlso rdf:datatype="&xsd;anyURI">https://identifiers.org/isbn/1584886420</rdfs:seeAlso>
        <skos:definition xml:lang="en">A feed-forward loop [https://identifiers.org/biomodels.teddy/TEDDY_0000037] in which the sign of the direct path from X to Z is the opposite as the overall sign of the indirect path from X through Y to Z.</skos:definition>
        <skos:altLabel xml:lang="en">incoherent 3-node feed-forward loop</skos:altLabel>
        <skos:altLabel xml:lang="en">incoherent 3-node feedforward</skos:altLabel>
        <skos:altLabel xml:lang="en">incoherent 3-node feedforward loop</skos:altLabel>
        <skos:altLabel xml:lang="en">incoherent three-node feedforward loop</skos:altLabel>
    </owl:Class>
    <owl:Axiom>
        <owl:annotatedTarget rdf:datatype="&xsd;anyURI">https://identifiers.org/isbn/1584886420</owl:annotatedTarget>
        <rdfs:comment xml:lang="en">Alon U (2006) An Introduction to Systems Biology: Design Principles of Biological Circuits, Chapman and Hall/CRC. (p.267)</rdfs:comment>
        <owl:annotatedSource rdf:resource="&teddy;TEDDY_0000043"/>
        <owl:annotatedProperty rdf:resource="&rdfs;seeAlso"/>
    </owl:Axiom>
    


    <!-- http://biomodels.net/teddy/TEDDY#TEDDY_0000044 -->

    <owl:Class rdf:about="&teddy;TEDDY_0000044">
        <rdfs:label xml:lang="en">type-1 incoherent three-node feed-forward loop</rdfs:label>
        <rdfs:subClassOf rdf:resource="&teddy;TEDDY_0000043"/>
        <rdfs:seeAlso rdf:datatype="&xsd;anyURI">https://identifiers.org/isbn/1584886420</rdfs:seeAlso>
        <skos:definition xml:lang="en">An &apos;incoherent three-node feed-forward loop&apos; [https://identifiers.org/biomodels.teddy/TEDDY_0000043] in which X activates Z, and also activates a repressor of Z.</skos:definition>
        <skos:altLabel xml:lang="en">I1-FFL</skos:altLabel>
        <skos:altLabel xml:lang="en">incoherent 3-node feedforward type-1</skos:altLabel>
        <skos:altLabel xml:lang="en">type-1 incoherent FFL</skos:altLabel>
    </owl:Class>
    <owl:Axiom>
        <owl:annotatedTarget rdf:datatype="&xsd;anyURI">https://identifiers.org/isbn/1584886420</owl:annotatedTarget>
        <rdfs:comment xml:lang="en">Alon U (2006) An Introduction to Systems Biology: Design Principles of Biological Circuits, Chapman and Hall/CRC. (p.47)</rdfs:comment>
        <owl:annotatedSource rdf:resource="&teddy;TEDDY_0000044"/>
        <owl:annotatedProperty rdf:resource="&rdfs;seeAlso"/>
    </owl:Axiom>
    


    <!-- http://biomodels.net/teddy/TEDDY#TEDDY_0000045 -->

    <owl:Class rdf:about="&teddy;TEDDY_0000045">
        <rdfs:label xml:lang="en">type-2 incoherent three-node feed-forward loop</rdfs:label>
        <rdfs:subClassOf rdf:resource="&teddy;TEDDY_0000043"/>
        <rdfs:seeAlso rdf:datatype="&xsd;anyURI">https://identifiers.org/isbn/1584886420</rdfs:seeAlso>
        <skos:definition xml:lang="en">An &apos;incoherent three-node feed-forward loop&apos; [https://identifiers.org/biomodels.teddy/TEDDY_0000043] in which X represses Z, and also represses a repressor of Z.</skos:definition>
        <skos:altLabel xml:lang="en">I2-FFL</skos:altLabel>
        <skos:altLabel xml:lang="en">incoherent 3-node feedforward type-2</skos:altLabel>
        <skos:altLabel xml:lang="en">type-2 incoherent FFL</skos:altLabel>
    </owl:Class>
    <owl:Axiom>
        <owl:annotatedTarget rdf:datatype="&xsd;anyURI">https://identifiers.org/isbn/1584886420</owl:annotatedTarget>
        <rdfs:comment xml:lang="en">Alon U (2006) An Introduction to Systems Biology: Design Principles of Biological Circuits, Chapman and Hall/CRC. (p.47)</rdfs:comment>
        <owl:annotatedSource rdf:resource="&teddy;TEDDY_0000045"/>
        <owl:annotatedProperty rdf:resource="&rdfs;seeAlso"/>
    </owl:Axiom>
    


    <!-- http://biomodels.net/teddy/TEDDY#TEDDY_0000046 -->

    <owl:Class rdf:about="&teddy;TEDDY_0000046">
        <rdfs:label xml:lang="en">type-3 incoherent three-node feed-forward loop</rdfs:label>
        <rdfs:subClassOf rdf:resource="&teddy;TEDDY_0000043"/>
        <rdfs:seeAlso rdf:datatype="&xsd;anyURI">https://identifiers.org/isbn/1584886420</rdfs:seeAlso>
        <skos:definition xml:lang="en">An &apos;incoherent three-node feed-forward loop&apos; [https://identifiers.org/biomodels.teddy/TEDDY_0000043] in which X represses Z, and also activates an activator of Z.</skos:definition>
        <skos:altLabel xml:lang="en">I3-FFL</skos:altLabel>
        <skos:altLabel xml:lang="en">incoherent 3-node feedforward type-3</skos:altLabel>
        <skos:altLabel xml:lang="en">type-3 incoherent FFL</skos:altLabel>
    </owl:Class>
    <owl:Axiom>
        <owl:annotatedTarget rdf:datatype="&xsd;anyURI">https://identifiers.org/isbn/1584886420</owl:annotatedTarget>
        <rdfs:comment xml:lang="en">Alon U (2006) An Introduction to Systems Biology: Design Principles of Biological Circuits, Chapman and Hall/CRC. (p.47)</rdfs:comment>
        <owl:annotatedSource rdf:resource="&teddy;TEDDY_0000046"/>
        <owl:annotatedProperty rdf:resource="&rdfs;seeAlso"/>
    </owl:Axiom>
    


    <!-- http://biomodels.net/teddy/TEDDY#TEDDY_0000047 -->

    <owl:Class rdf:about="&teddy;TEDDY_0000047">
        <rdfs:label xml:lang="en">type-4 incoherent three-node feed-forward loop</rdfs:label>
        <rdfs:subClassOf rdf:resource="&teddy;TEDDY_0000043"/>
        <rdfs:seeAlso rdf:datatype="&xsd;anyURI">https://identifiers.org/isbn/1584886420</rdfs:seeAlso>
        <skos:definition xml:lang="en">An &apos;incoherent three-node feed-forward loop&apos; [https://identifiers.org/biomodels.teddy/TEDDY_0000043] in which X activates Z, and also represses an activator of Z.</skos:definition>
        <skos:altLabel xml:lang="en">I4-FFL</skos:altLabel>
        <skos:altLabel xml:lang="en">incoherent 3-node feedforward type-4</skos:altLabel>
        <skos:altLabel xml:lang="en">type-4 incoherent FFL</skos:altLabel>
    </owl:Class>
    <owl:Axiom>
        <owl:annotatedTarget rdf:datatype="&xsd;anyURI">https://identifiers.org/isbn/1584886420</owl:annotatedTarget>
        <rdfs:comment xml:lang="en">Alon U (2006) An Introduction to Systems Biology: Design Principles of Biological Circuits, Chapman and Hall/CRC. (p.47)</rdfs:comment>
        <owl:annotatedSource rdf:resource="&teddy;TEDDY_0000047"/>
        <owl:annotatedProperty rdf:resource="&rdfs;seeAlso"/>
    </owl:Axiom>
    


    <!-- http://biomodels.net/teddy/TEDDY#TEDDY_0000048 -->

    <owl:Class rdf:about="&teddy;TEDDY_0000048">
        <rdfs:label xml:lang="en">orbit ((obsolete))</rdfs:label>
        <rdfs:subClassOf rdf:resource="&teddy;TEDDY_obsolete"/>
        <owl:deprecated rdf:datatype="&xsd;boolean">true</owl:deprecated>
        <skos:definition xml:lang="en">Obsolete: equivalent to TEDDY_0000083 &apos;Temporal Behaviour&apos;.</skos:definition>
    </owl:Class>
    


    <!-- http://biomodels.net/teddy/TEDDY#TEDDY_0000049 -->

    <owl:Class rdf:about="&teddy;TEDDY_0000049">
        <rdfs:label xml:lang="en">fixed point ((obsolete))</rdfs:label>
        <rdfs:subClassOf rdf:resource="&teddy;TEDDY_obsolete"/>
        <owl:deprecated rdf:datatype="&xsd;boolean">true</owl:deprecated>
        <skos:definition xml:lang="en">Obsolete: equivalent to TEDDY_0000086 &apos;Fixed Point&apos;.</skos:definition>
    </owl:Class>
    


    <!-- http://biomodels.net/teddy/TEDDY#TEDDY_0000050 -->

    <owl:Class rdf:about="&teddy;TEDDY_0000050">
        <rdfs:label xml:lang="en">periodic orbit</rdfs:label>
        <owl:equivalentClass>
            <owl:Class>
                <owl:intersectionOf rdf:parseType="Collection">
                    <rdf:Description rdf:about="&teddy;TEDDY_0000083"/>
                    <owl:Restriction>
                        <owl:onProperty rdf:resource="&teddy;TR_0004"/>
                        <owl:someValuesFrom rdf:resource="&teddy;TEDDY_0000067"/>
                    </owl:Restriction>
                </owl:intersectionOf>
            </owl:Class>
        </owl:equivalentClass>
        <rdfs:seeAlso rdf:datatype="&xsd;anyURI">https://identifiers.org/isbn/0387983821</rdfs:seeAlso>
        <skos:definition xml:lang="en">A temporal behaviour [https://identifiers.org/biomodels.teddy/TEDDY_0000083] which repeats every state after a specific period of time.</skos:definition>
        <skos:altLabel xml:lang="en">closed orbit</skos:altLabel>
        <skos:altLabel xml:lang="en">cycle</skos:altLabel>
        <skos:altLabel xml:lang="en">periodic solution</skos:altLabel>
    </owl:Class>
    <owl:Axiom>
        <owl:annotatedTarget rdf:datatype="&xsd;anyURI">https://identifiers.org/isbn/0387983821</owl:annotatedTarget>
        <rdfs:comment xml:lang="en">Kuznetsov YA. (1988) Elements of applied bifurcation theory, Springer, New York. (p.9)</rdfs:comment>
        <owl:annotatedSource rdf:resource="&teddy;TEDDY_0000050"/>
        <owl:annotatedProperty rdf:resource="&rdfs;seeAlso"/>
    </owl:Axiom>
    


    <!-- http://biomodels.net/teddy/TEDDY#TEDDY_0000051 -->

    <owl:Class rdf:about="&teddy;TEDDY_0000051">
        <rdfs:label xml:lang="en">limit cycle</rdfs:label>
        <rdfs:subClassOf rdf:resource="&teddy;TEDDY_0000050"/>
        <rdfs:subClassOf>
            <owl:Class>
                <owl:complementOf>
                    <owl:Restriction>
                        <owl:onProperty rdf:resource="&teddy;TR_0012"/>
                        <owl:someValuesFrom rdf:resource="&teddy;TEDDY_0000050"/>
                    </owl:Restriction>
                </owl:complementOf>
            </owl:Class>
        </rdfs:subClassOf>
        <rdfs:seeAlso rdf:datatype="&xsd;anyURI">https://identifiers.org/isbn/0738204536</rdfs:seeAlso>
        <skos:altLabel xml:lang="de">Grenzzyklus</skos:altLabel>
        <skos:definition xml:lang="en">A closed orbit which is isolated, i.e. neighbouring orbits are not closed.</skos:definition>
        <skos:altLabel xml:lang="en">isolated closed path</skos:altLabel>
    </owl:Class>
    <owl:Axiom>
        <rdfs:seeAlso rdf:datatype="&xsd;anyURI">https://identifiers.org/isbn/3817112823</rdfs:seeAlso>
        <owl:annotatedTarget xml:lang="de">Grenzzyklus</owl:annotatedTarget>
        <owl:annotatedSource rdf:resource="&teddy;TEDDY_0000051"/>
        <owl:annotatedProperty rdf:resource="&skos;altLabel"/>
    </owl:Axiom>
    <owl:Axiom>
        <owl:annotatedTarget rdf:datatype="&xsd;anyURI">https://identifiers.org/isbn/0738204536</owl:annotatedTarget>
        <rdfs:comment xml:lang="en">Strogatz SH. (2000) Nonlinear dynamics and chaos: with applications to physics, biology, chemistry, and engineering, Westview Press, Cambridge, MA. (p.196)</rdfs:comment>
        <owl:annotatedSource rdf:resource="&teddy;TEDDY_0000051"/>
        <owl:annotatedProperty rdf:resource="&rdfs;seeAlso"/>
    </owl:Axiom>
    <owl:Axiom>
        <rdfs:seeAlso rdf:datatype="&xsd;anyURI">https://identifiers.org/isbn/0198565623 (p.30)</rdfs:seeAlso>
        <owl:annotatedTarget xml:lang="en">isolated closed path</owl:annotatedTarget>
        <owl:annotatedSource rdf:resource="&teddy;TEDDY_0000051"/>
        <owl:annotatedProperty rdf:resource="&skos;altLabel"/>
    </owl:Axiom>
    


    <!-- http://biomodels.net/teddy/TEDDY#TEDDY_0000052 -->

    <owl:Class rdf:about="&teddy;TEDDY_0000052">
        <rdfs:label xml:lang="en">parameter dependency ((obsolete))</rdfs:label>
        <rdfs:subClassOf rdf:resource="&teddy;TEDDY_obsolete"/>
        <owl:deprecated rdf:datatype="&xsd;boolean">true</owl:deprecated>
        <skos:definition xml:lang="en">Obsolete: not required anymore.</skos:definition>
    </owl:Class>
    


    <!-- http://biomodels.net/teddy/TEDDY#TEDDY_0000053 -->

    <owl:Class rdf:about="&teddy;TEDDY_0000053">
        <rdfs:label xml:lang="en">bifurcation</rdfs:label>
        <rdfs:subClassOf rdf:resource="&teddy;TEDDY_0000132"/>
        <rdfs:seeAlso rdf:datatype="&xsd;anyURI">https://identifiers.org/isbn/0198565623</rdfs:seeAlso>
        <rdfs:seeAlso rdf:datatype="&xsd;anyURI">http://www.egwald.com/nonlineardynamics/bifurcations.php</rdfs:seeAlso>
        <skos:definition xml:lang="en">A `characteristic` describing a sudden qualitative (topological) change in the orbit structure of a system occuring as a parameter passes through a critical value, called a bifurcation point.</skos:definition>
    </owl:Class>
    <owl:Axiom>
        <owl:annotatedTarget rdf:datatype="&xsd;anyURI">http://www.egwald.com/nonlineardynamics/bifurcations.php</owl:annotatedTarget>
        <rdfs:comment xml:lang="en">Elmer G. Wiens: Egwald Web Services Ltd.</rdfs:comment>
        <owl:annotatedSource rdf:resource="&teddy;TEDDY_0000053"/>
        <owl:annotatedProperty rdf:resource="&rdfs;seeAlso"/>
    </owl:Axiom>
    <owl:Axiom>
        <owl:annotatedTarget rdf:datatype="&xsd;anyURI">https://identifiers.org/isbn/0198565623</owl:annotatedTarget>
        <rdfs:comment xml:lang="en">Jordan DW., Smith P. (1999) Nonlinear ordinary differential equations: an introduction to dynamical systems, Oxford University Press. (p.420)</rdfs:comment>
        <owl:annotatedSource rdf:resource="&teddy;TEDDY_0000053"/>
        <owl:annotatedProperty rdf:resource="&rdfs;seeAlso"/>
    </owl:Axiom>
    


    <!-- http://biomodels.net/teddy/TEDDY#TEDDY_0000054 -->

    <owl:Class rdf:about="&teddy;TEDDY_0000054">
        <rdfs:label xml:lang="en">strange attractor</rdfs:label>
        <rdfs:subClassOf rdf:resource="&teddy;TEDDY_0000094"/>
        <rdfs:subClassOf rdf:resource="&teddy;TEDDY_0000143"/>
        <rdfs:subClassOf>
            <owl:Class>
                <owl:complementOf>
                    <owl:Restriction>
                        <owl:onProperty rdf:resource="&teddy;TR_0004"/>
                        <owl:someValuesFrom rdf:resource="&teddy;TEDDY_0000133"/>
                    </owl:Restriction>
                </owl:complementOf>
            </owl:Class>
        </rdfs:subClassOf>
        <owl:disjointWith rdf:resource="&teddy;TEDDY_0000175"/>
        <rdfs:seeAlso rdf:datatype="&xsd;anyURI">https://identifiers.org/isbn/0738204536</rdfs:seeAlso>
        <rdfs:seeAlso rdf:datatype="&xsd;anyURI">https://identifiers.org/isbn/9810221428</rdfs:seeAlso>
        <skos:definition xml:lang="en">A non-periodic orbit [https://identifiers.org/biomodels.teddy/TEDDY_0000143] which is attracting and exhibits sensitive dependence on initial conditions.</skos:definition>
        <skos:definition xml:lang="en">The attractor [https://identifiers.org/biomodels.teddy/TEDDY_0000094] is strange if trajectories [https://identifiers.org/biomodels.teddy/TEDDY_0000083] on the attractor, being stable according to Poisson [https://identifiers.org/biomodels.teddy/TEDDY_0000149], are unstable according to Lyapunov [not TEDDY_0000113].</skos:definition>
        <skos:altLabel xml:lang="en">chaotic attractor</skos:altLabel>
        <skos:altLabel xml:lang="en">fractal attractor</skos:altLabel>
    </owl:Class>
    <owl:Axiom>
        <owl:annotatedTarget rdf:datatype="&xsd;anyURI">https://identifiers.org/isbn/0738204536</owl:annotatedTarget>
        <rdfs:comment xml:lang="en">Strogatz SH. (2000) Nonlinear dynamics and chaos: with applications to physics, biology, chemistry, and engineering, Westview Press, Cambridge, MA. (p.325)</rdfs:comment>
        <owl:annotatedSource rdf:resource="&teddy;TEDDY_0000054"/>
        <owl:annotatedProperty rdf:resource="&rdfs;seeAlso"/>
    </owl:Axiom>
    <owl:Axiom>
        <owl:annotatedTarget rdf:datatype="&xsd;anyURI">https://identifiers.org/isbn/9810221428</owl:annotatedTarget>
        <rdfs:comment xml:lang="en">V. S. Anishchenko (1995) Dynamical Chaos-Models and Experiments: Appearance Routes and Structure of Chaos in Simple Dynamical Systems (World Scientific Series on Nonlinear Science, Series a, Vol 8). World Scientific Pub Co Inc. (p.10)</rdfs:comment>
        <owl:annotatedSource rdf:resource="&teddy;TEDDY_0000054"/>
        <owl:annotatedProperty rdf:resource="&rdfs;seeAlso"/>
    </owl:Axiom>
    <owl:Axiom>
        <rdfs:seeAlso rdf:datatype="&xsd;anyURI">https://identifiers.org/isbn/0738204536 (p.325)</rdfs:seeAlso>
        <owl:annotatedTarget xml:lang="en">chaotic attractor</owl:annotatedTarget>
        <owl:annotatedSource rdf:resource="&teddy;TEDDY_0000054"/>
        <owl:annotatedProperty rdf:resource="&skos;altLabel"/>
    </owl:Axiom>
    <owl:Axiom>
        <rdfs:seeAlso rdf:datatype="&xsd;anyURI">https://identifiers.org/isbn/0738204536 (p.325)</rdfs:seeAlso>
        <owl:annotatedTarget xml:lang="en">fractal attractor</owl:annotatedTarget>
        <owl:annotatedSource rdf:resource="&teddy;TEDDY_0000054"/>
        <owl:annotatedProperty rdf:resource="&skos;altLabel"/>
    </owl:Axiom>
    


    <!-- http://biomodels.net/teddy/TEDDY#TEDDY_0000055 -->

    <owl:Class rdf:about="&teddy;TEDDY_0000055">
        <rdfs:label xml:lang="en">bursting</rdfs:label>
        <rdfs:subClassOf rdf:resource="&teddy;TEDDY_0000132"/>
        <rdfs:seeAlso rdf:datatype="&xsd;anyURI">https://identifiers.org/isbn/0262090430</rdfs:seeAlso>
        <skos:definition xml:lang="en">A burst is two or more spikes followed by a period of quiescence.</skos:definition>
    </owl:Class>
    <owl:Axiom>
        <owl:annotatedTarget rdf:datatype="&xsd;anyURI">https://identifiers.org/isbn/0262090430</owl:annotatedTarget>
        <rdfs:comment xml:lang="en">Izhikevich EM (2007) Dynamical systems in neuroscience : the geometry of excitability and bursting, MIT Press. (p.325)</rdfs:comment>
        <owl:annotatedSource rdf:resource="&teddy;TEDDY_0000055"/>
        <owl:annotatedProperty rdf:resource="&rdfs;seeAlso"/>
    </owl:Axiom>
    


    <!-- http://biomodels.net/teddy/TEDDY#TEDDY_0000056 -->

    <owl:Class rdf:about="&teddy;TEDDY_0000056">
        <rdfs:label xml:lang="en">switch</rdfs:label>
        <rdfs:subClassOf rdf:resource="&teddy;TEDDY_0000003"/>
        <rdfs:seeAlso rdf:datatype="&xsd;anyURI">https://identifiers.org/doi/10.1371/journal.pcbi.1002085</rdfs:seeAlso>
        <skos:definition xml:lang="en">A signaling network that converts a graded input cue into a binary, all-or-none response is said to exhibit ‘switch-like’ behavior; switching enables the establishment of discrete states which is vital in processes such as cell proliferation and differentiation.</skos:definition>
    </owl:Class>
    <owl:Axiom>
        <owl:annotatedTarget rdf:datatype="&xsd;anyURI">https://identifiers.org/doi/10.1371/journal.pcbi.1002085</owl:annotatedTarget>
        <rdfs:comment xml:lang="en">Shah NA, Sarkar CA (2011) Robust Network Topologies for Generating Switch-Like Cellular Responses, PLoS Comput Biol.; 7(6): e1002085.</rdfs:comment>
        <owl:annotatedSource rdf:resource="&teddy;TEDDY_0000056"/>
        <owl:annotatedProperty rdf:resource="&rdfs;seeAlso"/>
    </owl:Axiom>
    


    <!-- http://biomodels.net/teddy/TEDDY#TEDDY_0000057 -->

    <owl:Class rdf:about="&teddy;TEDDY_0000057">
        <rdfs:label xml:lang="en">stability ((obsolete))</rdfs:label>
        <rdfs:subClassOf rdf:resource="&teddy;TEDDY_obsolete"/>
        <owl:deprecated rdf:datatype="&xsd;boolean">true</owl:deprecated>
        <skos:definition xml:lang="en">Obsolete: not required anymore.</skos:definition>
    </owl:Class>
    


    <!-- http://biomodels.net/teddy/TEDDY#TEDDY_0000058 -->

    <owl:Class rdf:about="&teddy;TEDDY_0000058">
        <rdfs:label xml:lang="en">asymptotic decreasing ((obsolete))</rdfs:label>
        <rdfs:subClassOf rdf:resource="&teddy;TEDDY_obsolete"/>
        <rdfs:seeAlso rdf:datatype="&xsd;anyURI">http://eom.springer.de/A/a013610.htm</rdfs:seeAlso>
        <owl:deprecated rdf:datatype="&xsd;boolean">true</owl:deprecated>
        <skos:definition xml:lang="en">Asymptote of a curve y=f(x) with an infinite branch is a straight line the distance of which from the point (x, f(x)) on the curve tends to zero as the point moves along the branch of the curve to infinity. Decreasing function having for which an asymptote exists is called &apos;asymptotic decreasing&apos;.</skos:definition>
        <rdfs:comment xml:lang="en">use &apos;strictly decreasing&apos; [https://identifiers.org/biomodels.teddy/TEDDY_0000009] and &apos;asymptotic limit&apos; [https://identifiers.org/biomodels.teddy/TEDDY_0000026] terms instead.</rdfs:comment>
    </owl:Class>
    <owl:Axiom>
        <owl:annotatedTarget rdf:datatype="&xsd;anyURI">http://eom.springer.de/A/a013610.htm</owl:annotatedTarget>
        <rdfs:comment xml:lang="en">Encyclopaedia of Mathematics, edited by Michiel Hazewinkel, CWI, Amsterdam.</rdfs:comment>
        <owl:annotatedSource rdf:resource="&teddy;TEDDY_0000058"/>
        <owl:annotatedProperty rdf:resource="&rdfs;seeAlso"/>
    </owl:Axiom>
    


    <!-- http://biomodels.net/teddy/TEDDY#TEDDY_0000059 -->

    <owl:Class rdf:about="&teddy;TEDDY_0000059">
        <rdfs:label xml:lang="en">asymptotic increasing ((obsolete))</rdfs:label>
        <rdfs:subClassOf rdf:resource="&teddy;TEDDY_obsolete"/>
        <rdfs:seeAlso rdf:datatype="&xsd;anyURI">http://eom.springer.de/A/a013610.htm</rdfs:seeAlso>
        <owl:deprecated rdf:datatype="&xsd;boolean">true</owl:deprecated>
        <skos:definition xml:lang="en">Asymptote of a curve y=f(x) with an infinite branch is a straight line the distance of which from the point (x, f(x)) on the curve tends to zero as the point moves along the branch of the curve to infinity. Increasing function having for which an asymptote exists is called &apos;asymptotic increasing&apos;.</skos:definition>
        <rdfs:comment xml:lang="en">use &apos;strictly increasing&apos; [https://identifiers.org/biomodels.teddy/TEDDY_0000008] and &apos;asymptotic limit&apos; [https://identifiers.org/biomodels.teddy/TEDDY_0000026] terms instead.</rdfs:comment>
    </owl:Class>
    <owl:Axiom>
        <owl:annotatedTarget rdf:datatype="&xsd;anyURI">http://eom.springer.de/A/a013610.htm</owl:annotatedTarget>
        <rdfs:comment xml:lang="en">Encyclopaedia of Mathematics, edited by Michiel Hazewinkel, CWI, Amsterdam.</rdfs:comment>
        <owl:annotatedSource rdf:resource="&teddy;TEDDY_0000059"/>
        <owl:annotatedProperty rdf:resource="&rdfs;seeAlso"/>
    </owl:Axiom>
    


    <!-- http://biomodels.net/teddy/TEDDY#TEDDY_0000060 -->

    <owl:Class rdf:about="&teddy;TEDDY_0000060">
        <rdfs:label xml:lang="en">diverging increasing ((obsolete))</rdfs:label>
        <rdfs:subClassOf rdf:resource="&teddy;TEDDY_obsolete"/>
        <owl:deprecated rdf:datatype="&xsd;boolean">true</owl:deprecated>
        <rdfs:comment xml:lang="en">use &apos;strictly increasing&apos; [https://identifiers.org/biomodels.teddy/TEDDY_0000008] and &apos;infinite limit&apos; [https://identifiers.org/biomodels.teddy/TEDDY_0000030] terms instead.</rdfs:comment>
    </owl:Class>
    


    <!-- http://biomodels.net/teddy/TEDDY#TEDDY_0000061 -->

    <owl:Class rdf:about="&teddy;TEDDY_0000061">
        <rdfs:label xml:lang="en">chaotic oscillation</rdfs:label>
        <rdfs:subClassOf rdf:resource="&teddy;TEDDY_0000006"/>
        <skos:definition xml:lang="en">If a particular solution is aperiodic, but bounded for pt-&gt;infinity, then it corresponds to the regime of chaotic oscillation.</skos:definition>
        <rdfs:seeAlso xml:lang="en">https://identifiers.org/isbn/9810221428</rdfs:seeAlso>
        <skos:altLabel xml:lang="en">non-periodic oscillation</skos:altLabel>
    </owl:Class>
    <owl:Axiom>
        <rdfs:comment xml:lang="en">V. S. Anishchenko (1995) Dynamical Chaos-Models and Experiments: Appearance Routes and Structure of Chaos in Simple Dynamical Systems (World Scientific Series on Nonlinear Science, Series a, Vol 8). World Scientific Pub Co Inc. (p.10)</rdfs:comment>
        <owl:annotatedTarget xml:lang="en">https://identifiers.org/isbn/9810221428</owl:annotatedTarget>
        <owl:annotatedSource rdf:resource="&teddy;TEDDY_0000061"/>
        <owl:annotatedProperty rdf:resource="&rdfs;seeAlso"/>
    </owl:Axiom>
    


    <!-- http://biomodels.net/teddy/TEDDY#TEDDY_0000062 -->

    <owl:Class rdf:about="&teddy;TEDDY_0000062">
        <rdfs:label xml:lang="en">sustained oscillation ((obsolete))</rdfs:label>
        <rdfs:subClassOf rdf:resource="&teddy;TEDDY_obsolete"/>
        <owl:deprecated rdf:datatype="&xsd;boolean">true</owl:deprecated>
        <skos:definition xml:lang="en">Obsolete: equivalent to TEDDY_0000051 &apos;Limit Cycle&apos;.</skos:definition>
    </owl:Class>
    


    <!-- http://biomodels.net/teddy/TEDDY#TEDDY_0000063 -->

    <owl:Class rdf:about="&teddy;TEDDY_0000063">
        <rdfs:label xml:lang="en">damped oscillation</rdfs:label>
        <rdfs:subClassOf rdf:resource="&teddy;TEDDY_0000006"/>
        <rdfs:seeAlso rdf:datatype="&xsd;anyURI">https://identifiers.org/isbn/0486655083</rdfs:seeAlso>
        <skos:definition xml:lang="en">Damping is any effect that tends to reduce the amplitude [https://identifiers.org/biomodels.teddy/TEDDY_0000131] of oscillations in an oscillatory system.</skos:definition>
    </owl:Class>
    <owl:Axiom>
        <owl:annotatedTarget rdf:datatype="&xsd;anyURI">https://identifiers.org/isbn/0486655083</owl:annotatedTarget>
        <rdfs:comment xml:lang="en">A. A. Andronov, A. A. Vitt, and S. E. Khaikin (1987) Theory of Oscillators, Dover Publications.</rdfs:comment>
        <owl:annotatedSource rdf:resource="&teddy;TEDDY_0000063"/>
        <owl:annotatedProperty rdf:resource="&rdfs;seeAlso"/>
    </owl:Axiom>
    


    <!-- http://biomodels.net/teddy/TEDDY#TEDDY_0000064 -->

    <owl:Class rdf:about="&teddy;TEDDY_0000064">
        <rdfs:label xml:lang="en">single-periodic oscillation</rdfs:label>
        <rdfs:subClassOf rdf:resource="&teddy;TEDDY_0000066"/>
        <owl:disjointWith rdf:resource="&teddy;TEDDY_0000065"/>
        <rdfs:seeAlso rdf:datatype="&xsd;anyURI">https://identifiers.org/isbn/0198565623</rdfs:seeAlso>
        <skos:definition xml:lang="en">An oscillation [https://identifiers.org/biomodels.teddy/TEDDY_0000006] corresponding to a solution having a one-loop phase path and a period-1 Poincaré map.</skos:definition>
        <skos:altLabel xml:lang="en">SPO</skos:altLabel>
        <skos:altLabel xml:lang="en">single periodic oscillation</skos:altLabel>
    </owl:Class>
    <owl:Axiom>
        <owl:annotatedTarget rdf:datatype="&xsd;anyURI">https://identifiers.org/isbn/0198565623</owl:annotatedTarget>
        <rdfs:comment xml:lang="en">Jordan DW., Smith P. (1999) Nonlinear ordinary differential equations: an introduction to dynamical systems, Oxford University Press. (p.465)</rdfs:comment>
        <owl:annotatedSource rdf:resource="&teddy;TEDDY_0000064"/>
        <owl:annotatedProperty rdf:resource="&rdfs;seeAlso"/>
    </owl:Axiom>
    


    <!-- http://biomodels.net/teddy/TEDDY#TEDDY_0000065 -->

    <owl:Class rdf:about="&teddy;TEDDY_0000065">
        <rdfs:label xml:lang="en">mixed-mode oscillation</rdfs:label>
        <rdfs:subClassOf rdf:resource="&teddy;TEDDY_0000066"/>
        <rdfs:seeAlso rdf:datatype="&xsd;anyURI">https://identifiers.org/doi/10.1063/1.2900015</rdfs:seeAlso>
        <skos:altLabel xml:lang="en">MMO</skos:altLabel>
        <skos:definition xml:lang="en">Mixed-mode oscillations are complex periodic waveforms where each period is comprised of several maxima and minima of different amplitudes [https://identifiers.org/biomodels.teddy/TEDDY_0000131]. </skos:definition>
    </owl:Class>
    <owl:Axiom>
        <rdfs:comment xml:lang="en">I. Erchova and D. J. McGonigle (2008) Rhythms of the brain: an examination of mixed mode oscillation approaches to the analysis of neurophysiological data, Chaos (Woodbury, N.Y.) 18.</rdfs:comment>
        <owl:annotatedTarget xml:lang="en">mixed-mode oscillation</owl:annotatedTarget>
        <owl:annotatedSource rdf:resource="&teddy;TEDDY_0000065"/>
        <owl:annotatedProperty rdf:resource="&rdfs;label"/>
    </owl:Axiom>
    <owl:Axiom>
        <owl:annotatedTarget rdf:datatype="&xsd;anyURI">https://identifiers.org/doi/10.1063/1.2900015</owl:annotatedTarget>
        <rdfs:comment xml:lang="en">I. Erchova &amp; D. J. McGonigle (2008) Rhythms of the brain: an examination of mixed mode oscillation approaches to the analysis of neurophysiological data. Chaos (Woodbury, N.Y.) 18(1).</rdfs:comment>
        <owl:annotatedSource rdf:resource="&teddy;TEDDY_0000065"/>
        <owl:annotatedProperty rdf:resource="&rdfs;seeAlso"/>
    </owl:Axiom>
    


    <!-- http://biomodels.net/teddy/TEDDY#TEDDY_0000066 -->

    <owl:Class rdf:about="&teddy;TEDDY_0000066">
        <rdfs:label xml:lang="en">periodic oscillation</rdfs:label>
        <rdfs:subClassOf rdf:resource="&teddy;TEDDY_0000006"/>
        <rdfs:seeAlso rdf:datatype="&xsd;anyURI">https://identifiers.org/isbn/9810221428</rdfs:seeAlso>
        <skos:definition xml:lang="en">The characteristic of a periodic solution (a solution which is distinguished by the condition x*(t) = x*(t+T), where T is the period [https://identifiers.org/biomodels.teddy/TEDDY_0000067] of solution).</skos:definition>
    </owl:Class>
    <owl:Axiom>
        <owl:annotatedTarget rdf:datatype="&xsd;anyURI">https://identifiers.org/isbn/9810221428</owl:annotatedTarget>
        <rdfs:comment xml:lang="en">V. S. Anishchenko (1995) Dynamical Chaos-Models and Experiments: Appearance Routes and Structure of Chaos in Simple Dynamical Systems (World Scientific Series on Nonlinear Science, Series a, Vol 8). World Scientific Pub Co Inc. (p.6)</rdfs:comment>
        <owl:annotatedSource rdf:resource="&teddy;TEDDY_0000066"/>
        <owl:annotatedProperty rdf:resource="&rdfs;seeAlso"/>
    </owl:Axiom>
    


    <!-- http://biomodels.net/teddy/TEDDY#TEDDY_0000067 -->

    <owl:Class rdf:about="&teddy;TEDDY_0000067">
        <rdfs:label xml:lang="en">period</rdfs:label>
        <rdfs:subClassOf rdf:resource="&teddy;TEDDY_0000178"/>
        <rdfs:seeAlso rdf:datatype="&xsd;anyURI">http://eom.springer.de/p/p072210.htm</rdfs:seeAlso>
        <skos:definition xml:lang="en">For a periodic solution x(t), there is a number T, not equal to 0, such that x(t+T) = x(t) for t ∈ R. All possible such T are called periods of this periodic solution; the continuity of x(t) implies that either x(t) is independent of t or that all possible periods are integral multiples of one of them — the minimal period T0&gt;0. When one speaks of a periodic solution, it is often understood that the second case applies, and T0 is simply termed the period.</skos:definition>
    </owl:Class>
    <owl:Axiom>
        <owl:annotatedTarget rdf:datatype="&xsd;anyURI">http://eom.springer.de/p/p072210.htm</owl:annotatedTarget>
        <rdfs:comment xml:lang="en">Encyclopaedia of Mathematics, edited by Michiel Hazewinkel, CWI, Amsterdam.</rdfs:comment>
        <owl:annotatedSource rdf:resource="&teddy;TEDDY_0000067"/>
        <owl:annotatedProperty rdf:resource="&rdfs;seeAlso"/>
    </owl:Axiom>
    


    <!-- http://biomodels.net/teddy/TEDDY#TEDDY_0000068 -->

    <owl:Class rdf:about="&teddy;TEDDY_0000068">
        <rdfs:label xml:lang="en">regularity ((obsolete))</rdfs:label>
        <rdfs:subClassOf rdf:resource="&teddy;TEDDY_obsolete"/>
        <owl:deprecated rdf:datatype="&xsd;boolean">true</owl:deprecated>
        <skos:definition xml:lang="en">Obsolete: not required anymore.</skos:definition>
    </owl:Class>
    


    <!-- http://biomodels.net/teddy/TEDDY#TEDDY_0000069 -->

    <owl:Class rdf:about="&teddy;TEDDY_0000069">
        <rdfs:label xml:lang="en">local bifurcation</rdfs:label>
        <rdfs:subClassOf rdf:resource="&teddy;TEDDY_0000053"/>
        <rdfs:subClassOf>
            <owl:Restriction>
                <owl:onProperty rdf:resource="&teddy;TR_0017"/>
                <owl:someValuesFrom rdf:resource="&teddy;TEDDY_0000095"/>
            </owl:Restriction>
        </rdfs:subClassOf>
        <owl:disjointWith rdf:resource="&teddy;TEDDY_0000119"/>
        <rdfs:seeAlso rdf:datatype="&xsd;anyURI">http://en.wikipedia.org/wiki/Bifurcation_theory#Local_bifurcations</rdfs:seeAlso>
        <rdfs:seeAlso rdf:datatype="&xsd;anyURI">https://identifiers.org/isbn/0387983821</rdfs:seeAlso>
        <skos:definition xml:lang="en">A `bifurcation` [https://identifiers.org/biomodels.teddy/TEDDY_0000053] in which a stable [https://identifiers.org/biomodels.teddy/TEDDY_0000133] fixed point [https://identifiers.org/biomodels.teddy/TEDDY_0000086] changes to an unstable [not TEDDY_0000133] one or vanishes. It can be detected within any small neighborhood of the fixed point: the real part of the eigenvalue of the linarisation around the fixed point is zero at the bifurcation.</skos:definition>
        <skos:altLabel xml:lang="en">bifurcation from steady state</skos:altLabel>
        <skos:altLabel xml:lang="en">bifurcation of equilibrium</skos:altLabel>
        <skos:altLabel xml:lang="en">bifurcation of equilibrium point</skos:altLabel>
        <skos:altLabel xml:lang="en">bifurcation of fixed point</skos:altLabel>
    </owl:Class>
    <owl:Axiom>
        <owl:annotatedTarget rdf:datatype="&xsd;anyURI">https://identifiers.org/isbn/0387983821</owl:annotatedTarget>
        <rdfs:comment xml:lang="en">Kuznetsov YA. (1988) Elements of applied bifurcation theory, Springer, New York. (p.58)</rdfs:comment>
        <owl:annotatedSource rdf:resource="&teddy;TEDDY_0000069"/>
        <owl:annotatedProperty rdf:resource="&rdfs;seeAlso"/>
    </owl:Axiom>
    <owl:Axiom>
        <rdfs:seeAlso rdf:datatype="&xsd;anyURI">https://identifiers.org/isbn/0387983821 (p.58)</rdfs:seeAlso>
        <owl:annotatedTarget xml:lang="en">bifurcation of fixed point</owl:annotatedTarget>
        <owl:annotatedSource rdf:resource="&teddy;TEDDY_0000069"/>
        <owl:annotatedProperty rdf:resource="&skos;altLabel"/>
    </owl:Axiom>
    <owl:Axiom>
        <rdfs:seeAlso rdf:datatype="&xsd;anyURI">https://identifiers.org/isbn/0387983821 (p.58)</rdfs:seeAlso>
        <owl:annotatedTarget xml:lang="en">bifurcation of equilibrium</owl:annotatedTarget>
        <owl:annotatedSource rdf:resource="&teddy;TEDDY_0000069"/>
        <owl:annotatedProperty rdf:resource="&skos;altLabel"/>
    </owl:Axiom>
    <owl:Axiom>
        <rdfs:seeAlso rdf:datatype="&xsd;anyURI">http://www.scholarpedia.org/article/MATCONT</rdfs:seeAlso>
        <owl:annotatedTarget xml:lang="en">bifurcation from steady state</owl:annotatedTarget>
        <owl:annotatedSource rdf:resource="&teddy;TEDDY_0000069"/>
        <owl:annotatedProperty rdf:resource="&skos;altLabel"/>
    </owl:Axiom>
    


    <!-- http://biomodels.net/teddy/TEDDY#TEDDY_0000070 -->

    <owl:Class rdf:about="&teddy;TEDDY_0000070">
        <rdfs:label xml:lang="en">bifurcation of limit cycle</rdfs:label>
        <rdfs:subClassOf rdf:resource="&teddy;TEDDY_0000147"/>
        <rdfs:seeAlso rdf:datatype="&xsd;anyURI">https://identifiers.org/isbn/0387983821</rdfs:seeAlso>
        <skos:definition xml:lang="en">A global bifurcation [https://identifiers.org/biomodels.teddy/TEDDY_0000147] in which a limit cycle [https://identifiers.org/biomodels.teddy/TEDDY_0000051] (dis)appears or changes its stability [https://identifiers.org/biomodels.teddy/TEDDY_0000113].</skos:definition>
    </owl:Class>
    <owl:Axiom>
        <owl:annotatedTarget rdf:datatype="&xsd;anyURI">https://identifiers.org/isbn/0387983821</owl:annotatedTarget>
        <rdfs:comment xml:lang="en">Kuznetsov YA. (1988) Elements of applied bifurcation theory, Springer, New York. (p.162ff)</rdfs:comment>
        <owl:annotatedSource rdf:resource="&teddy;TEDDY_0000070"/>
        <owl:annotatedProperty rdf:resource="&rdfs;seeAlso"/>
    </owl:Axiom>
    


    <!-- http://biomodels.net/teddy/TEDDY#TEDDY_0000071 -->

    <owl:Class rdf:about="&teddy;TEDDY_0000071">
        <rdfs:label xml:lang="en">saddle-node bifurcation</rdfs:label>
        <rdfs:subClassOf rdf:resource="&teddy;TEDDY_0000123"/>
        <rdfs:subClassOf>
            <owl:Class>
                <owl:unionOf rdf:parseType="Collection">
                    <owl:Class>
                        <owl:intersectionOf rdf:parseType="Collection">
                            <owl:Restriction>
                                <owl:onProperty rdf:resource="&teddy;TR_0017"/>
                                <owl:onClass rdf:resource="&teddy;TEDDY_0000095"/>
                                <owl:qualifiedCardinality rdf:datatype="&xsd;nonNegativeInteger">1</owl:qualifiedCardinality>
                            </owl:Restriction>
                            <owl:Restriction>
                                <owl:onProperty rdf:resource="&teddy;TR_0017"/>
                                <owl:onClass rdf:resource="&teddy;TEDDY_0000129"/>
                                <owl:qualifiedCardinality rdf:datatype="&xsd;nonNegativeInteger">1</owl:qualifiedCardinality>
                            </owl:Restriction>
                        </owl:intersectionOf>
                    </owl:Class>
                    <owl:Class>
                        <owl:intersectionOf rdf:parseType="Collection">
                            <owl:Restriction>
                                <owl:onProperty rdf:resource="&teddy;TR_0018"/>
                                <owl:onClass rdf:resource="&teddy;TEDDY_0000095"/>
                                <owl:qualifiedCardinality rdf:datatype="&xsd;nonNegativeInteger">1</owl:qualifiedCardinality>
                            </owl:Restriction>
                            <owl:Restriction>
                                <owl:onProperty rdf:resource="&teddy;TR_0018"/>
                                <owl:onClass rdf:resource="&teddy;TEDDY_0000129"/>
                                <owl:qualifiedCardinality rdf:datatype="&xsd;nonNegativeInteger">1</owl:qualifiedCardinality>
                            </owl:Restriction>
                        </owl:intersectionOf>
                    </owl:Class>
                </owl:unionOf>
            </owl:Class>
        </rdfs:subClassOf>
        <rdfs:seeAlso rdf:datatype="&xsd;anyURI">https://identifiers.org/isbn/0387983821</rdfs:seeAlso>
        <rdfs:seeAlso rdf:datatype="&xsd;anyURI">https://identifiers.org/isbn/0738204536</rdfs:seeAlso>
        <skos:definition xml:lang="en">A `zero-eigenvalue bifurcation` [https://identifiers.org/biomodels.teddy/TEDDY_0000123] in which a stable [https://identifiers.org/biomodels.teddy/TEDDY_0000133] fixed point [https://identifiers.org/biomodels.teddy/TEDDY_0000086] and an unstable [not TEDDY_0000133] fixed point [https://identifiers.org/biomodels.teddy/TEDDY_0000086] collide and mutually annihilate.</skos:definition>
        <skos:altLabel xml:lang="en">blue sky bifurcation</skos:altLabel>
        <skos:altLabel xml:lang="en">fold bifurcation</skos:altLabel>
        <skos:altLabel xml:lang="en">limit point bifurcation</skos:altLabel>
        <skos:altLabel xml:lang="en">tangent bifurcation</skos:altLabel>
        <skos:altLabel xml:lang="en">turning-point bifurcation</skos:altLabel>
    </owl:Class>
    <owl:Axiom>
        <owl:annotatedTarget rdf:datatype="&xsd;anyURI">https://identifiers.org/isbn/0738204536</owl:annotatedTarget>
        <rdfs:comment xml:lang="en">Strogatz SH. (2000) Nonlinear dynamics and chaos: with applications to physics, biology, chemistry, and engineering, Westview Press, Cambridge, MA. (p.45)</rdfs:comment>
        <owl:annotatedSource rdf:resource="&teddy;TEDDY_0000071"/>
        <owl:annotatedProperty rdf:resource="&rdfs;seeAlso"/>
    </owl:Axiom>
    <owl:Axiom>
        <rdfs:seeAlso rdf:datatype="&xsd;anyURI">http://www.scholarpedia.org/article/Saddle-node_Bifurcation</rdfs:seeAlso>
        <owl:annotatedTarget xml:lang="en">limit point bifurcation</owl:annotatedTarget>
        <owl:annotatedSource rdf:resource="&teddy;TEDDY_0000071"/>
        <owl:annotatedProperty rdf:resource="&skos;altLabel"/>
    </owl:Axiom>
    <owl:Axiom>
        <rdfs:seeAlso rdf:datatype="&xsd;anyURI">https://identifiers.org/isbn/0738204536 (p.47)</rdfs:seeAlso>
        <owl:annotatedTarget xml:lang="en">fold bifurcation</owl:annotatedTarget>
        <owl:annotatedSource rdf:resource="&teddy;TEDDY_0000071"/>
        <owl:annotatedProperty rdf:resource="&skos;altLabel"/>
    </owl:Axiom>
    <owl:Axiom>
        <rdfs:seeAlso rdf:datatype="&xsd;anyURI">https://identifiers.org/isbn/0738204536 (p.47)</rdfs:seeAlso>
        <owl:annotatedTarget xml:lang="en">blue sky bifurcation</owl:annotatedTarget>
        <owl:annotatedSource rdf:resource="&teddy;TEDDY_0000071"/>
        <owl:annotatedProperty rdf:resource="&skos;altLabel"/>
    </owl:Axiom>
    <owl:Axiom>
        <rdfs:seeAlso rdf:datatype="&xsd;anyURI">https://identifiers.org/isbn/0387983821 (p.80)</rdfs:seeAlso>
        <owl:annotatedTarget xml:lang="en">tangent bifurcation</owl:annotatedTarget>
        <owl:annotatedSource rdf:resource="&teddy;TEDDY_0000071"/>
        <owl:annotatedProperty rdf:resource="&skos;altLabel"/>
    </owl:Axiom>
    <owl:Axiom>
        <owl:annotatedTarget rdf:datatype="&xsd;anyURI">https://identifiers.org/isbn/0387983821</owl:annotatedTarget>
        <rdfs:comment xml:lang="en">Kuznetsov YA. (1988) Elements of applied bifurcation theory, Springer, New York. (p.80)</rdfs:comment>
        <owl:annotatedSource rdf:resource="&teddy;TEDDY_0000071"/>
        <owl:annotatedProperty rdf:resource="&rdfs;seeAlso"/>
    </owl:Axiom>
    <owl:Axiom>
        <rdfs:seeAlso rdf:datatype="&xsd;anyURI">https://identifiers.org/isbn/0738204536 (p.47)</rdfs:seeAlso>
        <owl:annotatedTarget xml:lang="en">turning-point bifurcation</owl:annotatedTarget>
        <owl:annotatedSource rdf:resource="&teddy;TEDDY_0000071"/>
        <owl:annotatedProperty rdf:resource="&skos;altLabel"/>
    </owl:Axiom>
    


    <!-- http://biomodels.net/teddy/TEDDY#TEDDY_0000072 -->

    <owl:Class rdf:about="&teddy;TEDDY_0000072">
        <rdfs:label xml:lang="en">Hopf bifurcation</rdfs:label>
        <rdfs:subClassOf rdf:resource="&teddy;TEDDY_0000069"/>
        <rdfs:subClassOf>
            <owl:Class>
                <owl:intersectionOf rdf:parseType="Collection">
                    <owl:Restriction>
                        <owl:onProperty rdf:resource="&teddy;TR_0017"/>
                        <owl:someValuesFrom rdf:resource="&teddy;TEDDY_0000126"/>
                    </owl:Restriction>
                    <owl:Restriction>
                        <owl:onProperty rdf:resource="&teddy;TR_0018"/>
                        <owl:someValuesFrom rdf:resource="&teddy;TEDDY_0000127"/>
                    </owl:Restriction>
                </owl:intersectionOf>
            </owl:Class>
        </rdfs:subClassOf>
        <rdfs:seeAlso rdf:datatype="&xsd;anyURI">https://identifiers.org/isbn/0738204536</rdfs:seeAlso>
        <skos:definition xml:lang="en">A `local bifurcation` [https://identifiers.org/biomodels.teddy/TEDDY_0000069] in which a `stable spiral` [https://identifiers.org/biomodels.teddy/TEDDY_0000126] changes in an `unstable spiral` [https://identifiers.org/biomodels.teddy/TEDDY_0000127].  The linearisation around the fixed point [https://identifiers.org/biomodels.teddy/TEDDY_0000086] has two conjugate  eigenvalues. This eigenvalues cross simultaneously the imaginary axis from left (negative real part) to the right during the bifurcation.</skos:definition>
        <skos:altLabel xml:lang="en">Andronov-Hopf Bifurcation</skos:altLabel>
    </owl:Class>
    <owl:Axiom>
        <rdfs:seeAlso rdf:datatype="&xsd;anyURI">https://identifiers.org/isbn/0387983821 (p.80)</rdfs:seeAlso>
        <owl:annotatedTarget xml:lang="en">Andronov-Hopf Bifurcation</owl:annotatedTarget>
        <owl:annotatedSource rdf:resource="&teddy;TEDDY_0000072"/>
        <owl:annotatedProperty rdf:resource="&skos;altLabel"/>
    </owl:Axiom>
    <owl:Axiom>
        <owl:annotatedTarget rdf:datatype="&xsd;anyURI">https://identifiers.org/isbn/0738204536</owl:annotatedTarget>
        <rdfs:comment xml:lang="en">Strogatz SH. (2000) Nonlinear dynamics and chaos: with applications to physics, biology, chemistry, and engineering, Westview Press, Cambridge, MA. (p.248ff)</rdfs:comment>
        <owl:annotatedSource rdf:resource="&teddy;TEDDY_0000072"/>
        <owl:annotatedProperty rdf:resource="&rdfs;seeAlso"/>
    </owl:Axiom>
    


    <!-- http://biomodels.net/teddy/TEDDY#TEDDY_0000073 -->

    <owl:Class rdf:about="&teddy;TEDDY_0000073">
        <rdfs:label xml:lang="en">subcritical Hopf bifurcation</rdfs:label>
        <rdfs:subClassOf rdf:resource="&teddy;TEDDY_0000072"/>
        <rdfs:subClassOf>
            <owl:Restriction>
                <owl:onProperty rdf:resource="&teddy;TR_0018"/>
                <owl:someValuesFrom rdf:resource="&teddy;TEDDY_0000128"/>
            </owl:Restriction>
        </rdfs:subClassOf>
        <rdfs:seeAlso rdf:datatype="&xsd;anyURI">https://identifiers.org/isbn/0387983821</rdfs:seeAlso>
        <skos:definition xml:lang="en">A `Hopf bifurcation` [https://identifiers.org/biomodels.teddy/TEDDY_0000072] in which an `unstable limit cycle` [https://identifiers.org/biomodels.teddy/TEDDY_0000128] is destroyed.</skos:definition>
        <skos:altLabel xml:lang="en">subc-AH</skos:altLabel>
        <skos:altLabel xml:lang="en">subcritical Andronov-Hopf bifurcation</skos:altLabel>
    </owl:Class>
    <owl:Axiom>
        <rdfs:seeAlso rdf:datatype="&xsd;anyURI">http://www.tbi.univie.ac.at/wiki/index.php/Classification_of_Dynamical_Behaviors</rdfs:seeAlso>
        <owl:annotatedTarget xml:lang="en">subcritical Andronov-Hopf bifurcation</owl:annotatedTarget>
        <owl:annotatedSource rdf:resource="&teddy;TEDDY_0000073"/>
        <owl:annotatedProperty rdf:resource="&skos;altLabel"/>
    </owl:Axiom>
    <owl:Axiom>
        <rdfs:seeAlso rdf:datatype="&xsd;anyURI">http://www.tbi.univie.ac.at/wiki/index.php/Classification_of_Dynamical_Behaviors</rdfs:seeAlso>
        <owl:annotatedTarget xml:lang="en">subc-AH</owl:annotatedTarget>
        <owl:annotatedSource rdf:resource="&teddy;TEDDY_0000073"/>
        <owl:annotatedProperty rdf:resource="&skos;altLabel"/>
    </owl:Axiom>
    <owl:Axiom>
        <owl:annotatedTarget rdf:datatype="&xsd;anyURI">https://identifiers.org/isbn/0387983821</owl:annotatedTarget>
        <rdfs:comment xml:lang="en">Kuznetsov YA. (1988) Elements of applied bifurcation theory, Springer, New York. (p.88)</rdfs:comment>
        <owl:annotatedSource rdf:resource="&teddy;TEDDY_0000073"/>
        <owl:annotatedProperty rdf:resource="&rdfs;seeAlso"/>
    </owl:Axiom>
    


    <!-- http://biomodels.net/teddy/TEDDY#TEDDY_0000074 -->

    <owl:Class rdf:about="&teddy;TEDDY_0000074">
        <rdfs:label xml:lang="en">supercritical Hopf bifurcation</rdfs:label>
        <rdfs:subClassOf rdf:resource="&teddy;TEDDY_0000072"/>
        <rdfs:subClassOf>
            <owl:Restriction>
                <owl:onProperty rdf:resource="&teddy;TR_0017"/>
                <owl:someValuesFrom rdf:resource="&teddy;TEDDY_0000114"/>
            </owl:Restriction>
        </rdfs:subClassOf>
        <rdfs:seeAlso rdf:datatype="&xsd;anyURI">https://identifiers.org/isbn/0738204536</rdfs:seeAlso>
        <skos:definition xml:lang="en">A `Hopf bifurcation` [https://identifiers.org/biomodels.teddy/TEDDY_0000072] in which an `stable limit cycle` [https://identifiers.org/biomodels.teddy/TEDDY_0000114] appears.</skos:definition>
        <skos:altLabel xml:lang="en">supc-AH</skos:altLabel>
        <skos:altLabel xml:lang="en">supercritical Andronov-Hopf bifurcation</skos:altLabel>
    </owl:Class>
    <owl:Axiom>
        <owl:annotatedTarget rdf:datatype="&xsd;anyURI">https://identifiers.org/isbn/0738204536</owl:annotatedTarget>
        <rdfs:comment xml:lang="en">Strogatz SH. (2000) Nonlinear dynamics and chaos: with applications to physics, biology, chemistry, and engineering, Westview Press, Cambridge, MA. (p.249)</rdfs:comment>
        <owl:annotatedSource rdf:resource="&teddy;TEDDY_0000074"/>
        <owl:annotatedProperty rdf:resource="&rdfs;seeAlso"/>
    </owl:Axiom>
    <owl:Axiom>
        <rdfs:seeAlso rdf:datatype="&xsd;anyURI">http://www.tbi.univie.ac.at/wiki/index.php/Classification_of_Dynamical_Behaviors</rdfs:seeAlso>
        <owl:annotatedTarget xml:lang="en">supc-AH</owl:annotatedTarget>
        <owl:annotatedSource rdf:resource="&teddy;TEDDY_0000074"/>
        <owl:annotatedProperty rdf:resource="&skos;altLabel"/>
    </owl:Axiom>
    <owl:Axiom>
        <rdfs:seeAlso rdf:datatype="&xsd;anyURI">http://www.tbi.univie.ac.at/wiki/index.php/Classification_of_Dynamical_Behaviors</rdfs:seeAlso>
        <owl:annotatedTarget xml:lang="en">supercritical Andronov-Hopf bifurcation</owl:annotatedTarget>
        <owl:annotatedSource rdf:resource="&teddy;TEDDY_0000074"/>
        <owl:annotatedProperty rdf:resource="&skos;altLabel"/>
    </owl:Axiom>
    


    <!-- http://biomodels.net/teddy/TEDDY#TEDDY_0000075 -->

    <owl:Class rdf:about="&teddy;TEDDY_0000075">
        <rdfs:label xml:lang="en">saddle-node on invariant circle bifurcation</rdfs:label>
        <rdfs:subClassOf rdf:resource="&teddy;TEDDY_0000069"/>
        <rdfs:subClassOf>
            <owl:Class>
                <owl:unionOf rdf:parseType="Collection">
                    <owl:Restriction>
                        <owl:onProperty rdf:resource="&teddy;TR_0017"/>
                        <owl:someValuesFrom rdf:resource="&teddy;TEDDY_0000051"/>
                    </owl:Restriction>
                    <owl:Restriction>
                        <owl:onProperty rdf:resource="&teddy;TR_0018"/>
                        <owl:someValuesFrom rdf:resource="&teddy;TEDDY_0000051"/>
                    </owl:Restriction>
                </owl:unionOf>
            </owl:Class>
        </rdfs:subClassOf>
        <rdfs:seeAlso rdf:datatype="&xsd;anyURI">https://identifiers.org/isbn/0262090430</rdfs:seeAlso>
        <skos:altLabel xml:lang="en">SNIC</skos:altLabel>
        <skos:altLabel xml:lang="en">SNIC bifurcation</skos:altLabel>
        <skos:altLabel xml:lang="en">SNLC</skos:altLabel>
        <skos:altLabel xml:lang="en">SNLC bifurcation</skos:altLabel>
        <skos:definition xml:lang="en">Saddle-node bifurcation on invariant circle occurs when the center manifold of a saddle-node bifurcation [https://identifiers.org/biomodels.teddy/TEDDY_0000071] forms an invariant circle. Such a bifurcation results in (dis)appearance of a limit cycle [https://identifiers.org/biomodels.teddy/TEDDY_0000051] of an infinite period. </skos:definition>
        <skos:altLabel xml:lang="en">saddle-node on limit cycle bifurcation</skos:altLabel>
    </owl:Class>
    <owl:Axiom>
        <rdfs:seeAlso rdf:datatype="&xsd;anyURI">http://www.scholarpedia.org/article/Saddle-node_bifurcation_on_invariant_circle</rdfs:seeAlso>
        <owl:annotatedTarget xml:lang="en">SNLC bifurcation</owl:annotatedTarget>
        <owl:annotatedSource rdf:resource="&teddy;TEDDY_0000075"/>
        <owl:annotatedProperty rdf:resource="&skos;altLabel"/>
    </owl:Axiom>
    <owl:Axiom>
        <rdfs:seeAlso rdf:datatype="&xsd;anyURI">http://www.scholarpedia.org/article/Saddle-node_bifurcation_on_invariant_circle</rdfs:seeAlso>
        <owl:annotatedTarget xml:lang="en">SNLC</owl:annotatedTarget>
        <owl:annotatedSource rdf:resource="&teddy;TEDDY_0000075"/>
        <owl:annotatedProperty rdf:resource="&skos;altLabel"/>
    </owl:Axiom>
    <owl:Axiom>
        <rdfs:seeAlso rdf:datatype="&xsd;anyURI">http://www.tbi.univie.ac.at/wiki/index.php/Classification_of_Dynamical_Behaviors</rdfs:seeAlso>
        <owl:annotatedTarget xml:lang="en">SNIC</owl:annotatedTarget>
        <owl:annotatedSource rdf:resource="&teddy;TEDDY_0000075"/>
        <owl:annotatedProperty rdf:resource="&skos;altLabel"/>
    </owl:Axiom>
    <owl:Axiom>
        <rdfs:seeAlso rdf:datatype="&xsd;anyURI">http://www.scholarpedia.org/article/Saddle-node_bifurcation_on_invariant_circle</rdfs:seeAlso>
        <owl:annotatedTarget xml:lang="en">SNIC bifurcation</owl:annotatedTarget>
        <owl:annotatedSource rdf:resource="&teddy;TEDDY_0000075"/>
        <owl:annotatedProperty rdf:resource="&skos;altLabel"/>
    </owl:Axiom>
    <owl:Axiom>
        <owl:annotatedTarget rdf:datatype="&xsd;anyURI">https://identifiers.org/isbn/0262090430</owl:annotatedTarget>
        <rdfs:comment xml:lang="en">Izhikevich EM (2007) Dynamical systems in neuroscience : the geometry of excitability and bursting, MIT Press.</rdfs:comment>
        <owl:annotatedSource rdf:resource="&teddy;TEDDY_0000075"/>
        <owl:annotatedProperty rdf:resource="&rdfs;seeAlso"/>
    </owl:Axiom>
    <owl:Axiom>
        <rdfs:seeAlso rdf:datatype="&xsd;anyURI">http://www.scholarpedia.org/article/Saddle-node_bifurcation_on_invariant_circle</rdfs:seeAlso>
        <owl:annotatedTarget xml:lang="en">saddle-node on limit cycle bifurcation</owl:annotatedTarget>
        <owl:annotatedSource rdf:resource="&teddy;TEDDY_0000075"/>
        <owl:annotatedProperty rdf:resource="&skos;altLabel"/>
    </owl:Axiom>
    


    <!-- http://biomodels.net/teddy/TEDDY#TEDDY_0000076 -->

    <owl:Class rdf:about="&teddy;TEDDY_0000076">
        <rdfs:label xml:lang="en">saddle-node bifurcation of limit cycles</rdfs:label>
        <rdfs:subClassOf rdf:resource="&teddy;TEDDY_0000070"/>
        <rdfs:subClassOf>
            <owl:Restriction>
                <owl:onProperty rdf:resource="&teddy;TR_0017"/>
                <owl:onClass rdf:resource="&teddy;TEDDY_0000051"/>
                <owl:qualifiedCardinality rdf:datatype="&xsd;nonNegativeInteger">2</owl:qualifiedCardinality>
            </owl:Restriction>
        </rdfs:subClassOf>
        <rdfs:subClassOf>
            <owl:Restriction>
                <owl:onProperty rdf:resource="&teddy;TR_0018"/>
                <owl:onClass rdf:resource="&teddy;TEDDY_0000051"/>
                <owl:qualifiedCardinality rdf:datatype="&xsd;nonNegativeInteger">0</owl:qualifiedCardinality>
            </owl:Restriction>
        </rdfs:subClassOf>
        <rdfs:seeAlso rdf:datatype="&xsd;anyURI">https://identifiers.org/isbn/0387983821</rdfs:seeAlso>
        <skos:definition xml:lang="en">A &apos;bifurcation of limit cycle&apos; [https://identifiers.org/biomodels.teddy/TEDDY_0000070] in which two limit cycles [https://identifiers.org/biomodels.teddy/TEDDY_0000051] (stable [https://identifiers.org/biomodels.teddy/TEDDY_0000114] and saddle) collide and disappear.</skos:definition>
        <skos:altLabel xml:lang="en">fold bifurcation of limit cycles</skos:altLabel>
    </owl:Class>
    <owl:Axiom>
        <rdfs:seeAlso rdf:datatype="&xsd;anyURI">https://identifiers.org/isbn/0387983821 (p. 163)</rdfs:seeAlso>
        <owl:annotatedTarget xml:lang="en">fold bifurcation of limit cycles</owl:annotatedTarget>
        <owl:annotatedSource rdf:resource="&teddy;TEDDY_0000076"/>
        <owl:annotatedProperty rdf:resource="&skos;altLabel"/>
    </owl:Axiom>
    <owl:Axiom>
        <owl:annotatedTarget rdf:datatype="&xsd;anyURI">https://identifiers.org/isbn/0387983821</owl:annotatedTarget>
        <rdfs:comment xml:lang="en">Kuznetsov YA. (1988) Elements of applied bifurcation theory, Springer, New York. (p.163)</rdfs:comment>
        <owl:annotatedSource rdf:resource="&teddy;TEDDY_0000076"/>
        <owl:annotatedProperty rdf:resource="&rdfs;seeAlso"/>
    </owl:Axiom>
    


    <!-- http://biomodels.net/teddy/TEDDY#TEDDY_0000077 -->

    <owl:Class rdf:about="&teddy;TEDDY_0000077">
        <rdfs:label xml:lang="en">period-doubling bifurcation of limit cycle</rdfs:label>
        <rdfs:subClassOf rdf:resource="&teddy;TEDDY_0000070"/>
        <rdfs:subClassOf>
            <owl:Class>
                <owl:intersectionOf rdf:parseType="Collection">
                    <owl:Class>
                        <owl:unionOf rdf:parseType="Collection">
                            <owl:Class>
                                <owl:intersectionOf rdf:parseType="Collection">
                                    <owl:Restriction>
                                        <owl:onProperty rdf:resource="&teddy;TR_0017"/>
                                        <owl:someValuesFrom rdf:resource="&teddy;TEDDY_0000095"/>
                                    </owl:Restriction>
                                    <owl:Restriction>
                                        <owl:onProperty rdf:resource="&teddy;TR_0018"/>
                                        <owl:someValuesFrom rdf:resource="&teddy;TEDDY_0000129"/>
                                    </owl:Restriction>
                                </owl:intersectionOf>
                            </owl:Class>
                            <owl:Class>
                                <owl:intersectionOf rdf:parseType="Collection">
                                    <owl:Restriction>
                                        <owl:onProperty rdf:resource="&teddy;TR_0017"/>
                                        <owl:someValuesFrom rdf:resource="&teddy;TEDDY_0000129"/>
                                    </owl:Restriction>
                                    <owl:Restriction>
                                        <owl:onProperty rdf:resource="&teddy;TR_0018"/>
                                        <owl:someValuesFrom rdf:resource="&teddy;TEDDY_0000095"/>
                                    </owl:Restriction>
                                </owl:intersectionOf>
                            </owl:Class>
                        </owl:unionOf>
                    </owl:Class>
                    <owl:Restriction>
                        <owl:onProperty rdf:resource="&teddy;TR_0018"/>
                        <owl:someValuesFrom rdf:resource="&teddy;TEDDY_0000050"/>
                    </owl:Restriction>
                </owl:intersectionOf>
            </owl:Class>
        </rdfs:subClassOf>
        <rdfs:seeAlso rdf:datatype="&xsd;anyURI">https://identifiers.org/isbn/0387983821</rdfs:seeAlso>
        <skos:definition xml:lang="en">A &apos;bifurcation of limit cycle&apos; [https://identifiers.org/biomodels.teddy/TEDDY_0000070] in which a &apos;periodic orbit&apos; [https://identifiers.org/biomodels.teddy/TEDDY_0000050] with period-2 Poincaré map appears, while the fixed point changes its stability.</skos:definition>
        <skos:altLabel xml:lang="en">flip bifurcation of limit cycle</skos:altLabel>
    </owl:Class>
    <owl:Axiom>
        <rdfs:seeAlso rdf:datatype="&xsd;anyURI">https://identifiers.org/isbn/0387983821 (p.163)</rdfs:seeAlso>
        <owl:annotatedTarget xml:lang="en">flip bifurcation of limit cycle</owl:annotatedTarget>
        <owl:annotatedSource rdf:resource="&teddy;TEDDY_0000077"/>
        <owl:annotatedProperty rdf:resource="&skos;altLabel"/>
    </owl:Axiom>
    <owl:Axiom>
        <owl:annotatedTarget rdf:datatype="&xsd;anyURI">https://identifiers.org/isbn/0387983821</owl:annotatedTarget>
        <rdfs:comment xml:lang="en">Kuznetsov YA. (1988) Elements of applied bifurcation theory, Springer, New York. (p.163)</rdfs:comment>
        <owl:annotatedSource rdf:resource="&teddy;TEDDY_0000077"/>
        <owl:annotatedProperty rdf:resource="&rdfs;seeAlso"/>
    </owl:Axiom>
    


    <!-- http://biomodels.net/teddy/TEDDY#TEDDY_0000078 -->

    <owl:Class rdf:about="&teddy;TEDDY_0000078">
        <rdfs:label xml:lang="en">Neimark-Sacker bifurcation of limit cycle</rdfs:label>
        <rdfs:subClassOf rdf:resource="&teddy;TEDDY_0000070"/>
        <rdfs:seeAlso rdf:datatype="&xsd;anyURI">https://identifiers.org/isbn/0387983821</rdfs:seeAlso>
        <skos:definition xml:lang="en">A &apos;bifurcation of limit cycle&apos; [https://identifiers.org/biomodels.teddy/TEDDY_0000070] corresponding to the case when the multipliers are complex and simple and lie on the unit circle. The
Poincaré map then has a parameter-dependent, two-dimensional, invariant manifold on which a closed invariant curve generically bifurcates from the fixed point.</skos:definition>
    </owl:Class>
    <owl:Axiom>
        <owl:annotatedTarget rdf:datatype="&xsd;anyURI">https://identifiers.org/isbn/0387983821</owl:annotatedTarget>
        <rdfs:comment xml:lang="en">Kuznetsov YA. (1988) Elements of applied bifurcation theory, Springer, New York. (p.164)</rdfs:comment>
        <owl:annotatedSource rdf:resource="&teddy;TEDDY_0000078"/>
        <owl:annotatedProperty rdf:resource="&rdfs;seeAlso"/>
    </owl:Axiom>
    


    <!-- http://biomodels.net/teddy/TEDDY#TEDDY_0000079 -->

    <owl:Class rdf:about="&teddy;TEDDY_0000079">
        <rdfs:label xml:lang="en">integrator</rdfs:label>
        <rdfs:subClassOf rdf:resource="&teddy;TEDDY_0000003"/>
    </owl:Class>
    


    <!-- http://biomodels.net/teddy/TEDDY#TEDDY_0000080 -->

    <owl:Class rdf:about="&teddy;TEDDY_0000080">
        <rdfs:label xml:lang="en">_obsolete behaviour ((obsolete))</rdfs:label>
        <rdfs:subClassOf rdf:resource="&teddy;TEDDY_obsolete"/>
        <owl:deprecated rdf:datatype="&xsd;boolean">true</owl:deprecated>
        <skos:definition xml:lang="en">Obsolete: only one obsolete branch required.</skos:definition>
    </owl:Class>
    


    <!-- http://biomodels.net/teddy/TEDDY#TEDDY_0000081 -->

    <owl:Class rdf:about="&teddy;TEDDY_0000081">
        <rdfs:label xml:lang="en">_obsolete characteristic ((obsolete))</rdfs:label>
        <rdfs:subClassOf rdf:resource="&teddy;TEDDY_obsolete"/>
        <owl:deprecated rdf:datatype="&xsd;boolean">true</owl:deprecated>
        <skos:definition xml:lang="en">Obsolete: only one obsolete branch required.</skos:definition>
    </owl:Class>
    


    <!-- http://biomodels.net/teddy/TEDDY#TEDDY_0000082 -->

    <owl:Class rdf:about="&teddy;TEDDY_0000082">
        <rdfs:label xml:lang="en">_obsolete functionality ((obsolete))</rdfs:label>
        <rdfs:subClassOf rdf:resource="&teddy;TEDDY_obsolete"/>
        <owl:deprecated rdf:datatype="&xsd;boolean">true</owl:deprecated>
        <skos:definition xml:lang="en">Obsolete: only one obsolete branch required.</skos:definition>
    </owl:Class>
    


    <!-- http://biomodels.net/teddy/TEDDY#TEDDY_0000083 -->

    <owl:Class rdf:about="&teddy;TEDDY_0000083">
        <rdfs:label xml:lang="en">temporal behaviour</rdfs:label>
        <rdfs:subClassOf rdf:resource="&teddy;TEDDY_0000000"/>
        <rdfs:seeAlso rdf:datatype="&xsd;anyURI">https://identifiers.org/isbn/0387983821</rdfs:seeAlso>
        <skos:definition xml:lang="en">A temporal sequence of states following the evolution operator of the dynamical system through a given initial state.</skos:definition>
        <skos:altLabel xml:lang="en">orbit</skos:altLabel>
        <skos:altLabel xml:lang="en">phase curve</skos:altLabel>
        <skos:altLabel xml:lang="en">phase path</skos:altLabel>
        <skos:altLabel xml:lang="en">solution curve</skos:altLabel>
        <skos:altLabel xml:lang="en">trajectory</skos:altLabel>
    </owl:Class>
    <owl:Axiom>
        <rdfs:seeAlso rdf:datatype="&xsd;anyURI">https://identifiers.org/isbn/0387983821 (p.8)</rdfs:seeAlso>
        <owl:annotatedTarget xml:lang="en">trajectory</owl:annotatedTarget>
        <owl:annotatedSource rdf:resource="&teddy;TEDDY_0000083"/>
        <owl:annotatedProperty rdf:resource="&skos;altLabel"/>
    </owl:Axiom>
    <owl:Axiom>
        <rdfs:seeAlso rdf:datatype="&xsd;anyURI">https://identifiers.org/isbn/0198565623 (p.6)</rdfs:seeAlso>
        <owl:annotatedTarget xml:lang="en">phase path</owl:annotatedTarget>
        <owl:annotatedSource rdf:resource="&teddy;TEDDY_0000083"/>
        <owl:annotatedProperty rdf:resource="&skos;altLabel"/>
    </owl:Axiom>
    <owl:Axiom>
        <rdfs:seeAlso rdf:datatype="&xsd;anyURI">https://identifiers.org/isbn/0387983821 (p.8)</rdfs:seeAlso>
        <owl:annotatedTarget xml:lang="en">orbit</owl:annotatedTarget>
        <owl:annotatedSource rdf:resource="&teddy;TEDDY_0000083"/>
        <owl:annotatedProperty rdf:resource="&skos;altLabel"/>
    </owl:Axiom>
    <owl:Axiom>
        <owl:annotatedTarget rdf:datatype="&xsd;anyURI">https://identifiers.org/isbn/0387983821</owl:annotatedTarget>
        <rdfs:comment xml:lang="en">Kuznetsov YA. (1988) Elements of applied bifurcation theory, Springer, New York. (p.8)</rdfs:comment>
        <owl:annotatedSource rdf:resource="&teddy;TEDDY_0000083"/>
        <owl:annotatedProperty rdf:resource="&rdfs;seeAlso"/>
    </owl:Axiom>
    <owl:Axiom>
        <rdfs:seeAlso rdf:datatype="&xsd;anyURI">https://identifiers.org/isbn/0387908196 (p.2)</rdfs:seeAlso>
        <owl:annotatedTarget xml:lang="en">solution curve</owl:annotatedTarget>
        <owl:annotatedSource rdf:resource="&teddy;TEDDY_0000083"/>
        <owl:annotatedProperty rdf:resource="&skos;altLabel"/>
    </owl:Axiom>
    


    <!-- http://biomodels.net/teddy/TEDDY#TEDDY_0000084 -->

    <owl:Class rdf:about="&teddy;TEDDY_0000084">
        <rdfs:label xml:lang="en">parametrical behaviour ((obsolete))</rdfs:label>
        <rdfs:subClassOf rdf:resource="&teddy;TEDDY_obsolete"/>
        <owl:deprecated rdf:datatype="&xsd;boolean">true</owl:deprecated>
        <skos:definition xml:lang="en">Obsolete: not required anymore.</skos:definition>
    </owl:Class>
    


    <!-- http://biomodels.net/teddy/TEDDY#TEDDY_0000085 -->

    <owl:Class rdf:about="&teddy;TEDDY_0000085">
        <rdfs:label xml:lang="en">limit behaviour</rdfs:label>
        <rdfs:subClassOf rdf:resource="&teddy;TEDDY_0000083"/>
        <rdfs:seeAlso rdf:datatype="&xsd;anyURI">https://identifiers.org/isbn/0387983821</rdfs:seeAlso>
        <skos:definition xml:lang="en">A `temporal behaviour` [https://identifiers.org/biomodels.teddy/TEDDY_0000083] with all behaviours starting sufficiently near converge to it as time goes to either positive or negative infinity.</skos:definition>
        <skos:altLabel xml:lang="en">asymptotic state</skos:altLabel>
        <skos:altLabel xml:lang="en">limit set</skos:altLabel>
    </owl:Class>
    <owl:Axiom>
        <owl:annotatedTarget rdf:datatype="&xsd;anyURI">https://identifiers.org/isbn/0387983821</owl:annotatedTarget>
        <rdfs:comment xml:lang="en">Kuznetsov YA. (1988) Elements of applied bifurcation theory, Springer, New York. (p.10)</rdfs:comment>
        <owl:annotatedSource rdf:resource="&teddy;TEDDY_0000085"/>
        <owl:annotatedProperty rdf:resource="&rdfs;seeAlso"/>
    </owl:Axiom>
    


    <!-- http://biomodels.net/teddy/TEDDY#TEDDY_0000086 -->

    <owl:Class rdf:about="&teddy;TEDDY_0000086">
        <rdfs:label xml:lang="en">fixed point</rdfs:label>
        <rdfs:subClassOf rdf:resource="&teddy;TEDDY_0000083"/>
        <rdfs:seeAlso rdf:datatype="&xsd;anyURI">http://mathworld.wolfram.com/FixedPoint.html</rdfs:seeAlso>
        <skos:definition xml:lang="en">A &apos;temporal behaviour&apos; [https://identifiers.org/biomodels.teddy/TEDDY_0000083] which does not change its state.</skos:definition>
        <skos:altLabel xml:lang="en">constant behaviour</skos:altLabel>
        <skos:altLabel xml:lang="en">constant solution</skos:altLabel>
        <skos:altLabel xml:lang="en">critical point</skos:altLabel>
        <skos:altLabel xml:lang="en">equilibrium</skos:altLabel>
        <skos:altLabel xml:lang="en">equilibrium point</skos:altLabel>
        <skos:altLabel xml:lang="en">equilibrium solution</skos:altLabel>
        <skos:altLabel xml:lang="en">rest solution</skos:altLabel>
        <skos:altLabel xml:lang="en">steady state</skos:altLabel>
    </owl:Class>
    <owl:Axiom>
        <owl:annotatedTarget rdf:datatype="&xsd;anyURI">http://mathworld.wolfram.com/FixedPoint.html</owl:annotatedTarget>
        <rdfs:comment xml:lang="en">Weisstein, Eric W. Fixed Point. From MathWorld--A Wolfram Web Resource.</rdfs:comment>
        <owl:annotatedSource rdf:resource="&teddy;TEDDY_0000086"/>
        <owl:annotatedProperty rdf:resource="&rdfs;seeAlso"/>
    </owl:Axiom>
    <owl:Axiom>
        <rdfs:seeAlso rdf:datatype="&xsd;anyURI">https://identifiers.org/isbn/0198565623 (p.4)</rdfs:seeAlso>
        <owl:annotatedTarget xml:lang="en">equilibrium point</owl:annotatedTarget>
        <owl:annotatedSource rdf:resource="&teddy;TEDDY_0000086"/>
        <owl:annotatedProperty rdf:resource="&skos;altLabel"/>
    </owl:Axiom>
    <owl:Axiom>
        <rdfs:seeAlso rdf:datatype="&xsd;anyURI">https://identifiers.org/isbn/0198565623 (p.4)</rdfs:seeAlso>
        <owl:annotatedTarget xml:lang="en">critical point</owl:annotatedTarget>
        <owl:annotatedSource rdf:resource="&teddy;TEDDY_0000086"/>
        <owl:annotatedProperty rdf:resource="&skos;altLabel"/>
    </owl:Axiom>
    


    <!-- http://biomodels.net/teddy/TEDDY#TEDDY_0000087 -->

    <owl:Class rdf:about="&teddy;TEDDY_0000087">
        <rdfs:label xml:lang="en">node</rdfs:label>
        <rdfs:subClassOf rdf:resource="&teddy;TEDDY_0000086"/>
        <rdfs:subClassOf>
            <owl:Restriction>
                <owl:onProperty rdf:resource="&teddy;TR_0004"/>
                <owl:someValuesFrom rdf:resource="&teddy;TEDDY_0000157"/>
            </owl:Restriction>
        </rdfs:subClassOf>
        <rdfs:seeAlso rdf:datatype="&xsd;anyURI">https://identifiers.org/isbn/0738204536</rdfs:seeAlso>
        <skos:definition xml:lang="en">A &apos;fixed point&apos; [https://identifiers.org/biomodels.teddy/TEDDY_0000086] for which the Jacobian matrix has real-valued eigenvalues of the same sign.</skos:definition>
        <skos:altLabel xml:lang="en">fixed point node</skos:altLabel>
    </owl:Class>
    <owl:Axiom>
        <owl:annotatedTarget rdf:datatype="&xsd;anyURI">https://identifiers.org/isbn/0738204536</owl:annotatedTarget>
        <rdfs:comment xml:lang="en">Strogatz SH. (2000) Nonlinear dynamics and chaos: with applications to physics, biology, chemistry, and engineering, Westview Press, Cambridge, MA. (p.137)</rdfs:comment>
        <owl:annotatedSource rdf:resource="&teddy;TEDDY_0000087"/>
        <owl:annotatedProperty rdf:resource="&rdfs;seeAlso"/>
    </owl:Axiom>
    


    <!-- http://biomodels.net/teddy/TEDDY#TEDDY_0000088 -->

    <owl:Class rdf:about="&teddy;TEDDY_0000088">
        <rdfs:label xml:lang="en">center</rdfs:label>
        <rdfs:subClassOf rdf:resource="&teddy;TEDDY_0000086"/>
        <rdfs:subClassOf>
            <owl:Restriction>
                <owl:onProperty rdf:resource="&teddy;TR_0004"/>
                <owl:someValuesFrom rdf:resource="&teddy;TEDDY_0000098"/>
            </owl:Restriction>
        </rdfs:subClassOf>
        <rdfs:subClassOf>
            <owl:Restriction>
                <owl:onProperty rdf:resource="&teddy;TR_0012"/>
                <owl:someValuesFrom rdf:resource="&teddy;TEDDY_0000106"/>
            </owl:Restriction>
        </rdfs:subClassOf>
        <rdfs:subClassOf>
            <owl:Class>
                <owl:complementOf>
                    <owl:Restriction>
                        <owl:onProperty rdf:resource="&teddy;TR_0004"/>
                        <owl:someValuesFrom rdf:resource="&teddy;TEDDY_0000157"/>
                    </owl:Restriction>
                </owl:complementOf>
            </owl:Class>
        </rdfs:subClassOf>
        <rdfs:subClassOf>
            <owl:Class>
                <owl:complementOf>
                    <owl:Restriction>
                        <owl:onProperty rdf:resource="&teddy;TR_0004"/>
                        <owl:someValuesFrom rdf:resource="&teddy;TEDDY_0000097"/>
                    </owl:Restriction>
                </owl:complementOf>
            </owl:Class>
        </rdfs:subClassOf>
        <rdfs:subClassOf>
            <owl:Restriction>
                <owl:onProperty rdf:resource="&teddy;TR_0004"/>
                <owl:someValuesFrom rdf:resource="&teddy;TEDDY_0000150"/>
            </owl:Restriction>
        </rdfs:subClassOf>
        <rdfs:subClassOf>
            <owl:Restriction>
                <owl:onProperty rdf:resource="&teddy;TR_0004"/>
                <owl:someValuesFrom rdf:resource="&teddy;TEDDY_0000149"/>
            </owl:Restriction>
        </rdfs:subClassOf>
        <rdfs:seeAlso rdf:datatype="&xsd;anyURI">https://identifiers.org/isbn/0738204536</rdfs:seeAlso>
        <skos:definition xml:lang="en">A &apos;fixed point&apos; [https://identifiers.org/biomodels.teddy/TEDDY_0000086] for which the Jacobian matrix has purely imaginary complex conjugate eigenvalues. The fixed point is surrounded by a family of cycles in the phase portrait.</skos:definition>
        <skos:altLabel xml:lang="en">centre</skos:altLabel>
        <skos:altLabel xml:lang="en">elliptic fixed point</skos:altLabel>
    </owl:Class>
    <owl:Axiom>
        <owl:annotatedTarget rdf:datatype="&xsd;anyURI">https://identifiers.org/isbn/0738204536</owl:annotatedTarget>
        <rdfs:comment xml:lang="en">Strogatz SH. (2000) Nonlinear dynamics and chaos: with applications to physics, biology, chemistry, and engineering, Westview Press, Cambridge, MA. (pp.134,137)</rdfs:comment>
        <owl:annotatedSource rdf:resource="&teddy;TEDDY_0000088"/>
        <owl:annotatedProperty rdf:resource="&rdfs;seeAlso"/>
    </owl:Axiom>
    


    <!-- http://biomodels.net/teddy/TEDDY#TEDDY_0000089 -->

    <owl:Class rdf:about="&teddy;TEDDY_0000089">
        <rdfs:label xml:lang="en">saddle</rdfs:label>
        <rdfs:subClassOf rdf:resource="&teddy;TEDDY_0000086"/>
        <rdfs:subClassOf>
            <owl:Class>
                <owl:complementOf>
                    <owl:Restriction>
                        <owl:onProperty rdf:resource="&teddy;TR_0004"/>
                        <owl:someValuesFrom rdf:resource="&teddy;TEDDY_0000133"/>
                    </owl:Restriction>
                </owl:complementOf>
            </owl:Class>
        </rdfs:subClassOf>
        <rdfs:subClassOf>
            <owl:Restriction>
                <owl:onProperty rdf:resource="&teddy;TR_0004"/>
                <owl:someValuesFrom rdf:resource="&teddy;TEDDY_0000157"/>
            </owl:Restriction>
        </rdfs:subClassOf>
        <rdfs:subClassOf>
            <owl:Class>
                <owl:complementOf>
                    <owl:Restriction>
                        <owl:onProperty rdf:resource="&teddy;TR_0004"/>
                        <owl:someValuesFrom rdf:resource="&teddy;TEDDY_0000149"/>
                    </owl:Restriction>
                </owl:complementOf>
            </owl:Class>
        </rdfs:subClassOf>
        <rdfs:subClassOf>
            <owl:Restriction>
                <owl:onProperty rdf:resource="&teddy;TR_0004"/>
                <owl:someValuesFrom rdf:resource="&teddy;TEDDY_0000134"/>
            </owl:Restriction>
        </rdfs:subClassOf>
        <rdfs:seeAlso rdf:datatype="&xsd;anyURI">https://identifiers.org/isbn/0738204536</rdfs:seeAlso>
        <skos:definition xml:lang="en">A &apos;fixed point&apos; [https://identifiers.org/biomodels.teddy/TEDDY_0000086] for which the Jacobian matrix has real-valued eigenvalues of opposite signs.</skos:definition>
        <skos:altLabel xml:lang="en">saddle point</skos:altLabel>
    </owl:Class>
    <owl:Axiom>
        <owl:annotatedTarget rdf:datatype="&xsd;anyURI">https://identifiers.org/isbn/0738204536</owl:annotatedTarget>
        <rdfs:comment xml:lang="en">Strogatz SH. (2000) Nonlinear dynamics and chaos: with applications to physics, biology, chemistry, and engineering, Westview Press, Cambridge, MA. (p.137)</rdfs:comment>
        <owl:annotatedSource rdf:resource="&teddy;TEDDY_0000089"/>
        <owl:annotatedProperty rdf:resource="&rdfs;seeAlso"/>
    </owl:Axiom>
    <owl:Axiom>
        <rdfs:seeAlso rdf:datatype="&xsd;anyURI">https://identifiers.org/isbn/0198565623 (p.73)</rdfs:seeAlso>
        <owl:annotatedTarget xml:lang="en">saddle point</owl:annotatedTarget>
        <owl:annotatedSource rdf:resource="&teddy;TEDDY_0000089"/>
        <owl:annotatedProperty rdf:resource="&skos;altLabel"/>
    </owl:Axiom>
    


    <!-- http://biomodels.net/teddy/TEDDY#TEDDY_0000090 -->

    <owl:Class rdf:about="&teddy;TEDDY_0000090">
        <rdfs:label xml:lang="en">star</rdfs:label>
        <rdfs:subClassOf rdf:resource="&teddy;TEDDY_0000086"/>
        <rdfs:seeAlso rdf:datatype="&xsd;anyURI">https://identifiers.org/isbn/0738204536</rdfs:seeAlso>
        <skos:definition xml:lang="en">A &apos;fixed point&apos; [https://identifiers.org/biomodels.teddy/TEDDY_0000086] for which the Jacobian matrix has identical eigenvalues and two independent corresponding eigenvectors. All other trajectories [https://identifiers.org/biomodels.teddy/TEDDY_0000083] of the system lie on straight through the fixed point.</skos:definition>
        <skos:altLabel xml:lang="en">proper node</skos:altLabel>
        <skos:altLabel xml:lang="en">star point</skos:altLabel>
    </owl:Class>
    <owl:Axiom>
        <owl:annotatedTarget rdf:datatype="&xsd;anyURI">https://identifiers.org/isbn/0738204536</owl:annotatedTarget>
        <rdfs:comment xml:lang="en">Strogatz SH. (2000) Nonlinear dynamics and chaos: with applications to physics, biology, chemistry, and engineering, Westview Press, Cambridge, MA. (p.135)</rdfs:comment>
        <owl:annotatedSource rdf:resource="&teddy;TEDDY_0000090"/>
        <owl:annotatedProperty rdf:resource="&rdfs;seeAlso"/>
    </owl:Axiom>
    


    <!-- http://biomodels.net/teddy/TEDDY#TEDDY_0000091 -->

    <owl:Class rdf:about="&teddy;TEDDY_0000091">
        <rdfs:label xml:lang="en">spiral</rdfs:label>
        <rdfs:subClassOf rdf:resource="&teddy;TEDDY_0000086"/>
        <rdfs:subClassOf>
            <owl:Restriction>
                <owl:onProperty rdf:resource="&teddy;TR_0004"/>
                <owl:someValuesFrom rdf:resource="&teddy;TEDDY_0000157"/>
            </owl:Restriction>
        </rdfs:subClassOf>
        <rdfs:seeAlso rdf:datatype="&xsd;anyURI">https://identifiers.org/isbn/0738204536</rdfs:seeAlso>
        <skos:definition xml:lang="en">A &apos;fixed point&apos; [https://identifiers.org/biomodels.teddy/TEDDY_0000086] for which the Jacobian matrix has not purely imaginary complex conjugate eigenvalues. The fixed point is surrounded by spiralling behaviours [https://identifiers.org/biomodels.teddy/TEDDY_0000083].</skos:definition>
        <skos:altLabel xml:lang="en">focus</skos:altLabel>
        <skos:altLabel xml:lang="en">spiral point</skos:altLabel>
    </owl:Class>
    <owl:Axiom>
        <rdfs:seeAlso rdf:datatype="&xsd;anyURI">https://identifiers.org/isbn/0198565623 (p.73)</rdfs:seeAlso>
        <owl:annotatedTarget xml:lang="en">spiral point</owl:annotatedTarget>
        <owl:annotatedSource rdf:resource="&teddy;TEDDY_0000091"/>
        <owl:annotatedProperty rdf:resource="&skos;altLabel"/>
    </owl:Axiom>
    <owl:Axiom>
        <owl:annotatedTarget rdf:datatype="&xsd;anyURI">https://identifiers.org/isbn/0738204536</owl:annotatedTarget>
        <rdfs:comment xml:lang="en">Strogatz SH. (2000) Nonlinear dynamics and chaos: with applications to physics, biology, chemistry, and engineering, Westview Press, Cambridge, MA. (pp.134,137)</rdfs:comment>
        <owl:annotatedSource rdf:resource="&teddy;TEDDY_0000091"/>
        <owl:annotatedProperty rdf:resource="&rdfs;seeAlso"/>
    </owl:Axiom>
    <owl:Axiom>
        <rdfs:seeAlso rdf:datatype="&xsd;anyURI">https://identifiers.org/isbn/0198565623 (p.25)</rdfs:seeAlso>
        <owl:annotatedTarget xml:lang="en">focus</owl:annotatedTarget>
        <owl:annotatedSource rdf:resource="&teddy;TEDDY_0000091"/>
        <owl:annotatedProperty rdf:resource="&skos;altLabel"/>
    </owl:Axiom>
    


    <!-- http://biomodels.net/teddy/TEDDY#TEDDY_0000092 -->

    <owl:Class rdf:about="&teddy;TEDDY_0000092">
        <rdfs:label xml:lang="en">non-isolated fixed point</rdfs:label>
        <rdfs:subClassOf rdf:resource="&teddy;TEDDY_0000086"/>
        <rdfs:subClassOf>
            <owl:Restriction>
                <owl:onProperty rdf:resource="&teddy;TR_0012"/>
                <owl:someValuesFrom rdf:resource="&teddy;TEDDY_0000092"/>
            </owl:Restriction>
        </rdfs:subClassOf>
        <rdfs:seeAlso rdf:datatype="&xsd;anyURI">https://identifiers.org/isbn/0738204536</rdfs:seeAlso>
        <skos:definition xml:lang="en">A &apos;fixed point&apos; [https://identifiers.org/biomodels.teddy/TEDDY_0000086] for which at least one eigenvalue of the Jacobian matrix is zero. If the other eigenvalue is non-zero the system has an entire line of fixed points along one dimension. If both eigenvalues are zero the system has a entire plane of fixed points.</skos:definition>
    </owl:Class>
    <owl:Axiom>
        <owl:annotatedTarget rdf:datatype="&xsd;anyURI">https://identifiers.org/isbn/0738204536</owl:annotatedTarget>
        <rdfs:comment xml:lang="en">Strogatz SH. (2000) Nonlinear dynamics and chaos: with applications to physics, biology, chemistry, and engineering, Westview Press, Cambridge, MA. (pp.128,137)</rdfs:comment>
        <owl:annotatedSource rdf:resource="&teddy;TEDDY_0000092"/>
        <owl:annotatedProperty rdf:resource="&rdfs;seeAlso"/>
    </owl:Axiom>
    


    <!-- http://biomodels.net/teddy/TEDDY#TEDDY_0000093 -->

    <owl:Class rdf:about="&teddy;TEDDY_0000093">
        <rdfs:label xml:lang="en">degenerate node</rdfs:label>
        <rdfs:subClassOf rdf:resource="&teddy;TEDDY_0000086"/>
        <rdfs:seeAlso rdf:datatype="&xsd;anyURI">https://identifiers.org/isbn/0738204536</rdfs:seeAlso>
        <skos:definition xml:lang="en">A &apos;fixed point&apos; [https://identifiers.org/biomodels.teddy/TEDDY_0000086] for which the Jacobian matrix has identical eigenvalues and only one independent eigenvector. All other trajectories [https://identifiers.org/biomodels.teddy/TEDDY_0000083] of the system asymptotically become parallel to the unique eigendirection.</skos:definition>
        <skos:altLabel xml:lang="en">degenerated node</skos:altLabel>
        <skos:altLabel xml:lang="en">improper node</skos:altLabel>
    </owl:Class>
    <owl:Axiom>
        <owl:annotatedTarget rdf:datatype="&xsd;anyURI">https://identifiers.org/isbn/0738204536</owl:annotatedTarget>
        <rdfs:comment xml:lang="en">Strogatz SH. (2000) Nonlinear dynamics and chaos: with applications to physics, biology, chemistry, and engineering, Westview Press, Cambridge, MA. (p.135f)</rdfs:comment>
        <owl:annotatedSource rdf:resource="&teddy;TEDDY_0000093"/>
        <owl:annotatedProperty rdf:resource="&rdfs;seeAlso"/>
    </owl:Axiom>
    


    <!-- http://biomodels.net/teddy/TEDDY#TEDDY_0000094 -->

    <owl:Class rdf:about="&teddy;TEDDY_0000094">
        <rdfs:label xml:lang="en">attractor</rdfs:label>
        <rdfs:subClassOf rdf:resource="&teddy;TEDDY_0000085"/>
        <rdfs:subClassOf>
            <owl:Restriction>
                <owl:onProperty rdf:resource="&teddy;TR_0004"/>
                <owl:someValuesFrom rdf:resource="&teddy;TEDDY_0000149"/>
            </owl:Restriction>
        </rdfs:subClassOf>
        <owl:disjointWith rdf:resource="&teddy;TEDDY_0000102"/>
        <rdfs:seeAlso rdf:datatype="&xsd;anyURI">https://identifiers.org/isbn/0738204536</rdfs:seeAlso>
        <rdfs:seeAlso rdf:datatype="&xsd;anyURI">https://identifiers.org/isbn/9810221428</rdfs:seeAlso>
        <skos:definition xml:lang="en">The limit set which corresponds to the particular type of stable solution and attracts phase trajectories [https://identifiers.org/biomodels.teddy/TEDDY_0000083] from a sertan region of initial conditions is an attractor.</skos:definition>
        <owl:disjointUnionOf rdf:parseType="Collection">
            <rdf:Description rdf:about="&teddy;TEDDY_0000054"/>
            <rdf:Description rdf:about="&teddy;TEDDY_0000175"/>
        </owl:disjointUnionOf>
    </owl:Class>
    <owl:Axiom>
        <owl:annotatedTarget rdf:datatype="&xsd;anyURI">https://identifiers.org/isbn/9810221428</owl:annotatedTarget>
        <rdfs:comment xml:lang="en">V. S. Anishchenko (1995) Dynamical Chaos-Models and Experiments: Appearance Routes and Structure of Chaos in Simple Dynamical Systems (World Scientific Series on Nonlinear Science, Series a, Vol 8). World Scientific Pub Co Inc. (p.10)</rdfs:comment>
        <owl:annotatedSource rdf:resource="&teddy;TEDDY_0000094"/>
        <owl:annotatedProperty rdf:resource="&rdfs;seeAlso"/>
    </owl:Axiom>
    <owl:Axiom>
        <owl:annotatedTarget rdf:datatype="&xsd;anyURI">https://identifiers.org/isbn/0738204536</owl:annotatedTarget>
        <rdfs:comment xml:lang="en">Strogatz SH. (2000) Nonlinear dynamics and chaos: with applications to physics, biology, chemistry, and engineering, Westview Press, Cambridge, MA. (p.324)</rdfs:comment>
        <owl:annotatedSource rdf:resource="&teddy;TEDDY_0000094"/>
        <owl:annotatedProperty rdf:resource="&rdfs;seeAlso"/>
    </owl:Axiom>
    


    <!-- http://biomodels.net/teddy/TEDDY#TEDDY_0000095 -->

    <owl:Class rdf:about="&teddy;TEDDY_0000095">
        <rdfs:label xml:lang="en">Lyapunov stable fixed point</rdfs:label>
        <owl:equivalentClass>
            <owl:Class>
                <owl:intersectionOf rdf:parseType="Collection">
                    <rdf:Description rdf:about="&teddy;TEDDY_0000086"/>
                    <owl:Restriction>
                        <owl:onProperty rdf:resource="&teddy;TR_0004"/>
                        <owl:someValuesFrom rdf:resource="&teddy;TEDDY_0000133"/>
                    </owl:Restriction>
                </owl:intersectionOf>
            </owl:Class>
        </owl:equivalentClass>
        <rdfs:seeAlso rdf:datatype="&xsd;anyURI">https://identifiers.org/isbn/0738204536</rdfs:seeAlso>
        <skos:definition xml:lang="en">A &apos;fixed point&apos; [https://identifiers.org/biomodels.teddy/TEDDY_0000086] which is Liapunov stable [https://identifiers.org/biomodels.teddy/TEDDY_0000133].</skos:definition>
        <skos:altLabel xml:lang="en">Liapunov stable fixed point</skos:altLabel>
    </owl:Class>
    <owl:Axiom>
        <owl:annotatedTarget rdf:datatype="&xsd;anyURI">https://identifiers.org/isbn/0738204536</owl:annotatedTarget>
        <rdfs:comment xml:lang="en">Strogatz SH. (2000) Nonlinear dynamics and chaos: with applications to physics, biology, chemistry, and engineering, Westview Press, Cambridge, MA. (p.129)</rdfs:comment>
        <owl:annotatedSource rdf:resource="&teddy;TEDDY_0000095"/>
        <owl:annotatedProperty rdf:resource="&rdfs;seeAlso"/>
    </owl:Axiom>
    


    <!-- http://biomodels.net/teddy/TEDDY#TEDDY_0000096 -->

    <owl:Class rdf:about="&teddy;TEDDY_0000096">
        <rdfs:label xml:lang="en">unstable ((obsolete))</rdfs:label>
        <rdfs:subClassOf rdf:resource="&teddy;TEDDY_obsolete"/>
        <rdfs:seeAlso rdf:datatype="&xsd;anyURI">https://identifiers.org/isbn/0738204536</rdfs:seeAlso>
        <owl:deprecated rdf:datatype="&xsd;boolean">true</owl:deprecated>
        <skos:definition xml:lang="en">Obsolete: a limit behaviour is unstable if it is neither Liapunov stable nor stable (use repellor instead).</skos:definition>
    </owl:Class>
    <owl:Axiom>
        <owl:annotatedTarget rdf:datatype="&xsd;anyURI">https://identifiers.org/isbn/0738204536</owl:annotatedTarget>
        <rdfs:comment xml:lang="en">Strogatz SH. (2000) Nonlinear dynamics and chaos: with applications to physics, biology, chemistry, and engineering, Westview Press, Cambridge, MA. (p.129)</rdfs:comment>
        <owl:annotatedSource rdf:resource="&teddy;TEDDY_0000096"/>
        <owl:annotatedProperty rdf:resource="&rdfs;seeAlso"/>
    </owl:Axiom>
    


    <!-- http://biomodels.net/teddy/TEDDY#TEDDY_0000097 -->

    <owl:Class rdf:about="&teddy;TEDDY_0000097">
        <rdfs:label xml:lang="en">asymptotic stability</rdfs:label>
        <rdfs:subClassOf rdf:resource="&teddy;TEDDY_0000133"/>
        <owl:disjointWith rdf:resource="&teddy;TEDDY_0000098"/>
        <rdfs:seeAlso rdf:datatype="&xsd;anyURI">https://identifiers.org/isbn/0738204536</rdfs:seeAlso>
        <skos:definition xml:lang="en">A `stable behaviour` which is also a `Liapunov stable behaviour`.</skos:definition>
        <skos:definition xml:lang="en">The solution x*(t), t &gt;= t0 is asymptotically stable, if all sufficiently small disturbances of the initial value lead to the solutions which re-approach the undisturbed solution.</skos:definition>
        <skos:altLabel xml:lang="en">stable behaviour</skos:altLabel>
    </owl:Class>
    <owl:Axiom>
        <owl:annotatedTarget rdf:datatype="&xsd;anyURI">https://identifiers.org/isbn/0738204536</owl:annotatedTarget>
        <rdfs:comment xml:lang="en">Strogatz SH. (2000) Nonlinear dynamics and chaos: with applications to physics, biology, chemistry, and engineering, Westview Press, Cambridge, MA. (p.129)</rdfs:comment>
        <owl:annotatedSource rdf:resource="&teddy;TEDDY_0000097"/>
        <owl:annotatedProperty rdf:resource="&rdfs;seeAlso"/>
    </owl:Axiom>
    <owl:Axiom>
        <rdfs:seeAlso rdf:datatype="&xsd;anyURI">https://identifiers.org/isbn/0738204536, (p.129)</rdfs:seeAlso>
        <owl:annotatedTarget xml:lang="en">stable behaviour</owl:annotatedTarget>
        <owl:annotatedSource rdf:resource="&teddy;TEDDY_0000097"/>
        <owl:annotatedProperty rdf:resource="&skos;altLabel"/>
    </owl:Axiom>
    


    <!-- http://biomodels.net/teddy/TEDDY#TEDDY_0000098 -->

    <owl:Class rdf:about="&teddy;TEDDY_0000098">
        <rdfs:label xml:lang="en">neutral stability</rdfs:label>
        <owl:equivalentClass>
            <owl:Class>
                <owl:intersectionOf rdf:parseType="Collection">
                    <rdf:Description rdf:about="&teddy;TEDDY_0000133"/>
                    <owl:Class>
                        <owl:complementOf rdf:resource="&teddy;TEDDY_0000097"/>
                    </owl:Class>
                </owl:intersectionOf>
            </owl:Class>
        </owl:equivalentClass>
        <rdfs:seeAlso rdf:datatype="&xsd;anyURI">https://identifiers.org/isbn/0738204536</rdfs:seeAlso>
        <skos:definition xml:lang="en">A behaviour [https://identifiers.org/biomodels.teddy/TEDDY_0000083] which is Liapunov stable [https://identifiers.org/biomodels.teddy/TEDDY_0000133] and not attracting [https://identifiers.org/biomodels.teddy/TEDDY_0000097].</skos:definition>
        <skos:altLabel xml:lang="en">asymptotically unstable</skos:altLabel>
    </owl:Class>
    <owl:Axiom>
        <owl:annotatedTarget rdf:datatype="&xsd;anyURI">https://identifiers.org/isbn/0738204536</owl:annotatedTarget>
        <rdfs:comment xml:lang="en">Strogatz SH. (2000) Nonlinear dynamics and chaos: with applications to physics, biology, chemistry, and engineering, Westview Press, Cambridge, MA. (p.129)</rdfs:comment>
        <owl:annotatedSource rdf:resource="&teddy;TEDDY_0000098"/>
        <owl:annotatedProperty rdf:resource="&rdfs;seeAlso"/>
    </owl:Axiom>
    <owl:Axiom>
        <owl:annotatedTarget xml:lang="en">asymptotically unstable</owl:annotatedTarget>
        <rdfs:seeAlso>https://identifiers.org/isbn/0198565623 (p.289)</rdfs:seeAlso>
        <owl:annotatedSource rdf:resource="&teddy;TEDDY_0000098"/>
        <owl:annotatedProperty rdf:resource="&skos;altLabel"/>
    </owl:Axiom>
    


    <!-- http://biomodels.net/teddy/TEDDY#TEDDY_0000099 -->

    <owl:Class rdf:about="&teddy;TEDDY_0000099">
        <rdfs:label xml:lang="en">saddle connection</rdfs:label>
        <owl:equivalentClass>
            <owl:Class>
                <owl:intersectionOf rdf:parseType="Collection">
                    <rdf:Description rdf:about="&teddy;TEDDY_0000143"/>
                    <owl:Class>
                        <owl:complementOf>
                            <owl:Restriction>
                                <owl:onProperty rdf:resource="&teddy;TR_0013"/>
                                <owl:someValuesFrom>
                                    <owl:Class>
                                        <owl:complementOf rdf:resource="&teddy;TEDDY_0000089"/>
                                    </owl:Class>
                                </owl:someValuesFrom>
                            </owl:Restriction>
                        </owl:complementOf>
                    </owl:Class>
                    <owl:Restriction>
                        <owl:onProperty rdf:resource="&teddy;TR_0013"/>
                        <owl:onClass rdf:resource="&teddy;TEDDY_0000089"/>
                        <owl:minQualifiedCardinality rdf:datatype="&xsd;nonNegativeInteger">1</owl:minQualifiedCardinality>
                    </owl:Restriction>
                    <owl:Restriction>
                        <owl:onProperty rdf:resource="&teddy;TR_0013"/>
                        <owl:onClass rdf:resource="&teddy;TEDDY_0000089"/>
                        <owl:maxQualifiedCardinality rdf:datatype="&xsd;nonNegativeInteger">2</owl:maxQualifiedCardinality>
                    </owl:Restriction>
                </owl:intersectionOf>
            </owl:Class>
        </owl:equivalentClass>
        <rdfs:seeAlso rdf:datatype="&xsd;anyURI">https://identifiers.org/isbn/0738204536</rdfs:seeAlso>
        <skos:definition xml:lang="en">A temporal behaviour [https://identifiers.org/biomodels.teddy/TEDDY_0000083] connecting two saddle points [https://identifiers.org/biomodels.teddy/TEDDY_0000089].</skos:definition>
    </owl:Class>
    <owl:Axiom>
        <owl:annotatedTarget rdf:datatype="&xsd;anyURI">https://identifiers.org/isbn/0738204536</owl:annotatedTarget>
        <rdfs:comment xml:lang="en">Strogatz SH. (2000) Nonlinear dynamics and chaos: with applications to physics, biology, chemistry, and engineering, Westview Press, Cambridge, MA. (p.184)</rdfs:comment>
        <owl:annotatedSource rdf:resource="&teddy;TEDDY_0000099"/>
        <owl:annotatedProperty rdf:resource="&rdfs;seeAlso"/>
    </owl:Axiom>
    


    <!-- http://biomodels.net/teddy/TEDDY#TEDDY_0000100 -->

    <owl:Class rdf:about="&teddy;TEDDY_0000100">
        <rdfs:label xml:lang="en">homoclinic saddle connection</rdfs:label>
        <owl:equivalentClass>
            <owl:Class>
                <owl:intersectionOf rdf:parseType="Collection">
                    <rdf:Description rdf:about="&teddy;TEDDY_0000099"/>
                    <owl:Restriction>
                        <owl:onProperty rdf:resource="&teddy;TR_0013"/>
                        <owl:onClass rdf:resource="&teddy;TEDDY_0000089"/>
                        <owl:qualifiedCardinality rdf:datatype="&xsd;nonNegativeInteger">1</owl:qualifiedCardinality>
                    </owl:Restriction>
                </owl:intersectionOf>
            </owl:Class>
        </owl:equivalentClass>
        <owl:disjointWith rdf:resource="&teddy;TEDDY_0000101"/>
        <rdfs:seeAlso rdf:datatype="&xsd;anyURI">https://identifiers.org/isbn/0738204536</rdfs:seeAlso>
        <skos:definition xml:lang="en">A saddle connection [https://identifiers.org/biomodels.teddy/TEDDY_0000099] connecting a saddle point [https://identifiers.org/biomodels.teddy/TEDDY_0000089] to itself.</skos:definition>
        <skos:altLabel xml:lang="en">homoclinic saddle loop</skos:altLabel>
        <skos:altLabel xml:lang="en">saddle loop</skos:altLabel>
    </owl:Class>
    <owl:Axiom>
        <rdfs:seeAlso rdf:datatype="&xsd;anyURI">http://www.egwald.ca/nonlineardynamics/mathappendix.php#limitset</rdfs:seeAlso>
        <owl:annotatedTarget xml:lang="en">saddle loop</owl:annotatedTarget>
        <owl:annotatedSource rdf:resource="&teddy;TEDDY_0000100"/>
        <owl:annotatedProperty rdf:resource="&skos;altLabel"/>
    </owl:Axiom>
    <owl:Axiom>
        <owl:annotatedTarget rdf:datatype="&xsd;anyURI">https://identifiers.org/isbn/0738204536</owl:annotatedTarget>
        <rdfs:comment xml:lang="en">Strogatz SH. (2000) Nonlinear dynamics and chaos: with applications to physics, biology, chemistry, and engineering, Westview Press, Cambridge, MA. (p.161)</rdfs:comment>
        <owl:annotatedSource rdf:resource="&teddy;TEDDY_0000100"/>
        <owl:annotatedProperty rdf:resource="&rdfs;seeAlso"/>
    </owl:Axiom>
    <owl:Axiom>
        <rdfs:seeAlso rdf:datatype="&xsd;anyURI">https://identifiers.org/isbn/3540971416 (p.213)</rdfs:seeAlso>
        <owl:annotatedTarget xml:lang="en">homoclinic saddle loop</owl:annotatedTarget>
        <owl:annotatedSource rdf:resource="&teddy;TEDDY_0000100"/>
        <owl:annotatedProperty rdf:resource="&skos;altLabel"/>
    </owl:Axiom>
    


    <!-- http://biomodels.net/teddy/TEDDY#TEDDY_0000101 -->

    <owl:Class rdf:about="&teddy;TEDDY_0000101">
        <rdfs:label xml:lang="en">heteroclinic saddle connection</rdfs:label>
        <owl:equivalentClass>
            <owl:Class>
                <owl:intersectionOf rdf:parseType="Collection">
                    <rdf:Description rdf:about="&teddy;TEDDY_0000099"/>
                    <owl:Restriction>
                        <owl:onProperty rdf:resource="&teddy;TR_0013"/>
                        <owl:onClass rdf:resource="&teddy;TEDDY_0000089"/>
                        <owl:qualifiedCardinality rdf:datatype="&xsd;nonNegativeInteger">2</owl:qualifiedCardinality>
                    </owl:Restriction>
                </owl:intersectionOf>
            </owl:Class>
        </owl:equivalentClass>
        <rdfs:seeAlso rdf:datatype="&xsd;anyURI">https://identifiers.org/isbn/0738204536</rdfs:seeAlso>
        <skos:definition xml:lang="en">A saddle connection [https://identifiers.org/biomodels.teddy/TEDDY_0000099] connecting two different saddle points [https://identifiers.org/biomodels.teddy/TEDDY_0000089].</skos:definition>
        <skos:altLabel xml:lang="en">heteroclinic saddle trajectory</skos:altLabel>
        <skos:altLabel xml:lang="en">saddle connection</skos:altLabel>
    </owl:Class>
    <owl:Axiom>
        <rdfs:seeAlso rdf:datatype="&xsd;anyURI">https://identifiers.org/isbn/0738204536 (p.166)</rdfs:seeAlso>
        <owl:annotatedTarget xml:lang="en">heteroclinic saddle trajectory</owl:annotatedTarget>
        <owl:annotatedSource rdf:resource="&teddy;TEDDY_0000101"/>
        <owl:annotatedProperty rdf:resource="&skos;altLabel"/>
    </owl:Axiom>
    <owl:Axiom>
        <owl:annotatedTarget rdf:datatype="&xsd;anyURI">https://identifiers.org/isbn/0738204536</owl:annotatedTarget>
        <rdfs:comment xml:lang="en">Strogatz SH. (2000) Nonlinear dynamics and chaos: with applications to physics, biology, chemistry, and engineering, Westview Press, Cambridge, MA. (p.166)</rdfs:comment>
        <owl:annotatedSource rdf:resource="&teddy;TEDDY_0000101"/>
        <owl:annotatedProperty rdf:resource="&rdfs;seeAlso"/>
    </owl:Axiom>
    <owl:Axiom>
        <rdfs:seeAlso rdf:datatype="&xsd;anyURI">https://identifiers.org/isbn/0738204536 (p.166)</rdfs:seeAlso>
        <rdfs:comment xml:lang="en">The term `saddle connection` is used as a synonym for a heteroclinic orbit (https://identifiers.org/isbn/0738204536 (p.166) ). But `saddle connection` is also used for both: homoclinic and heteroclinic orbits (https://identifiers.org/isbn/0387943773 (p.184)).</rdfs:comment>
        <owl:annotatedTarget xml:lang="en">saddle connection</owl:annotatedTarget>
        <owl:annotatedSource rdf:resource="&teddy;TEDDY_0000101"/>
        <owl:annotatedProperty rdf:resource="&skos;altLabel"/>
    </owl:Axiom>
    


    <!-- http://biomodels.net/teddy/TEDDY#TEDDY_0000102 -->

    <owl:Class rdf:about="&teddy;TEDDY_0000102">
        <rdfs:label rdf:datatype="&xsd;anyURI">repeller</rdfs:label>
        <owl:equivalentClass>
            <owl:Restriction>
                <owl:onProperty rdf:resource="&teddy;TR_0015"/>
                <owl:someValuesFrom rdf:resource="&teddy;TEDDY_0000094"/>
            </owl:Restriction>
        </owl:equivalentClass>
        <rdfs:subClassOf rdf:resource="&teddy;TEDDY_0000085"/>
        <rdfs:subClassOf>
            <owl:Class>
                <owl:complementOf>
                    <owl:Restriction>
                        <owl:onProperty rdf:resource="&teddy;TR_0004"/>
                        <owl:someValuesFrom rdf:resource="&teddy;TEDDY_0000133"/>
                    </owl:Restriction>
                </owl:complementOf>
            </owl:Class>
        </rdfs:subClassOf>
        <rdfs:subClassOf>
            <owl:Class>
                <owl:complementOf>
                    <owl:Restriction>
                        <owl:onProperty rdf:resource="&teddy;TR_0004"/>
                        <owl:someValuesFrom rdf:resource="&teddy;TEDDY_0000149"/>
                    </owl:Restriction>
                </owl:complementOf>
            </owl:Class>
        </rdfs:subClassOf>
        <rdfs:seeAlso rdf:datatype="&xsd;anyURI">http://eom.springer.de/R/r081310.htm</rdfs:seeAlso>
        <skos:definition xml:lang="en">A subset of the phase space of the system that is an attractor [https://identifiers.org/biomodels.teddy/TEDDY_0000094] for the reverse [TR_0015] system.</skos:definition>
        <skos:altLabel xml:lang="en">repelling set</skos:altLabel>
        <skos:altLabel xml:lang="en">repellor</skos:altLabel>
    </owl:Class>
    <owl:Axiom>
        <owl:annotatedTarget rdf:datatype="&xsd;anyURI">http://eom.springer.de/R/r081310.htm</owl:annotatedTarget>
        <rdfs:comment xml:lang="en">Encyclopaedia of Mathematics, edited by Michiel Hazewinkel, CWI, Amsterdam.</rdfs:comment>
        <owl:annotatedSource rdf:resource="&teddy;TEDDY_0000102"/>
        <owl:annotatedProperty rdf:resource="&rdfs;seeAlso"/>
    </owl:Axiom>
    <owl:Axiom>
        <rdfs:seeAlso rdf:datatype="&xsd;anyURI">http://eom.springer.de/R/r081310.htm</rdfs:seeAlso>
        <owl:annotatedTarget xml:lang="en">repelling set</owl:annotatedTarget>
        <owl:annotatedSource rdf:resource="&teddy;TEDDY_0000102"/>
        <owl:annotatedProperty rdf:resource="&skos;altLabel"/>
    </owl:Axiom>
    


    <!-- http://biomodels.net/teddy/TEDDY#TEDDY_0000103 -->

    <owl:Class rdf:about="&teddy;TEDDY_0000103">
        <rdfs:label xml:lang="en">stable ((obsolete))</rdfs:label>
        <rdfs:subClassOf rdf:resource="&teddy;TEDDY_obsolete"/>
        <rdfs:seeAlso rdf:datatype="&xsd;anyURI">https://identifiers.org/isbn/0738204536</rdfs:seeAlso>
        <owl:deprecated rdf:datatype="&xsd;boolean">true</owl:deprecated>
        <skos:definition xml:lang="en">Obsolete: a limit behaviour [https://identifiers.org/biomodels.teddy/TEDDY_0000085] is stable if all behaviours starting sufficiently near to it will approach it as time goes to positive infinity (use attractor instead).</skos:definition>
        <skos:altLabel xml:lang="en">attracting</skos:altLabel>
        <rdfs:comment xml:lang="en">rdfs:label follows notation in https://identifiers.org/isbn/3817112823 (p.42).</rdfs:comment>
    </owl:Class>
    <owl:Axiom>
        <owl:annotatedTarget rdf:datatype="&xsd;anyURI">https://identifiers.org/isbn/0738204536</owl:annotatedTarget>
        <rdfs:comment xml:lang="en">Strogatz SH. (2000) Nonlinear dynamics and chaos: with applications to physics, biology, chemistry, and engineering, Westview Press, Cambridge, MA. (p.128)</rdfs:comment>
        <owl:annotatedSource rdf:resource="&teddy;TEDDY_0000103"/>
        <owl:annotatedProperty rdf:resource="&rdfs;seeAlso"/>
    </owl:Axiom>
    


    <!-- http://biomodels.net/teddy/TEDDY#TEDDY_0000104 -->

    <owl:Class rdf:about="&teddy;TEDDY_0000104">
        <rdfs:label xml:lang="en">half-stable fixed point</rdfs:label>
        <owl:equivalentClass>
            <owl:Class>
                <owl:intersectionOf rdf:parseType="Collection">
                    <rdf:Description rdf:about="&teddy;TEDDY_0000086"/>
                    <owl:Restriction>
                        <owl:onProperty rdf:resource="&teddy;TR_0004"/>
                        <owl:someValuesFrom rdf:resource="&teddy;TEDDY_0000134"/>
                    </owl:Restriction>
                </owl:intersectionOf>
            </owl:Class>
        </owl:equivalentClass>
        <rdfs:seeAlso rdf:datatype="&xsd;anyURI">https://identifiers.org/isbn/0738204536</rdfs:seeAlso>
        <skos:definition xml:lang="en">A &apos;fixed point&apos; [https://identifiers.org/biomodels.teddy/TEDDY_0000086] which is half-stable [https://identifiers.org/biomodels.teddy/TEDDY_0000134], i.e. the fixed point is attracting in one direction and unstable in the other direction.</skos:definition>
    </owl:Class>
    <owl:Axiom>
        <owl:annotatedTarget rdf:datatype="&xsd;anyURI">https://identifiers.org/isbn/0738204536</owl:annotatedTarget>
        <rdfs:comment xml:lang="en">Strogatz SH. (2000) Nonlinear dynamics and chaos: with applications to physics, biology, chemistry, and engineering, Westview Press, Cambridge, MA. (p.26)</rdfs:comment>
        <owl:annotatedSource rdf:resource="&teddy;TEDDY_0000104"/>
        <owl:annotatedProperty rdf:resource="&rdfs;seeAlso"/>
    </owl:Axiom>
    


    <!-- http://biomodels.net/teddy/TEDDY#TEDDY_0000105 -->

    <owl:Class rdf:about="&teddy;TEDDY_0000105">
        <rdfs:label xml:lang="en">neutrally stable behaviour ((obsolete))</rdfs:label>
        <rdfs:subClassOf rdf:resource="&teddy;TEDDY_obsolete"/>
        <rdfs:seeAlso rdf:datatype="&xsd;anyURI">https://identifiers.org/isbn/0738204536</rdfs:seeAlso>
        <owl:deprecated rdf:datatype="&xsd;boolean">true</owl:deprecated>
        <skos:altLabel xml:lang="en">Non-Isolated Asymptotic Behaviour</skos:altLabel>
        <skos:definition xml:lang="en">Obsolete: a temporal behaviour which is neither attracting nor unstable (equivalent to &apos;neutrally stable&apos; [https://identifiers.org/biomodels.teddy/TEDDY_0000098]).</skos:definition>
    </owl:Class>
    <owl:Axiom>
        <owl:annotatedTarget rdf:datatype="&xsd;anyURI">https://identifiers.org/isbn/0738204536</owl:annotatedTarget>
        <rdfs:comment xml:lang="en">Strogatz SH. (2000) Nonlinear dynamics and chaos: with applications to physics, biology, chemistry, and engineering, Westview Press, Cambridge, MA. (p.129)</rdfs:comment>
        <owl:annotatedSource rdf:resource="&teddy;TEDDY_0000105"/>
        <owl:annotatedProperty rdf:resource="&rdfs;seeAlso"/>
    </owl:Axiom>
    


    <!-- http://biomodels.net/teddy/TEDDY#TEDDY_0000106 -->

    <owl:Class rdf:about="&teddy;TEDDY_0000106">
        <rdfs:label xml:lang="en">non-isolated cycle</rdfs:label>
        <owl:equivalentClass>
            <owl:Class>
                <owl:intersectionOf rdf:parseType="Collection">
                    <rdf:Description rdf:about="&teddy;TEDDY_0000050"/>
                    <owl:Restriction>
                        <owl:onProperty rdf:resource="&teddy;TR_0004"/>
                        <owl:someValuesFrom rdf:resource="&teddy;TEDDY_0000098"/>
                    </owl:Restriction>
                </owl:intersectionOf>
            </owl:Class>
        </owl:equivalentClass>
        <rdfs:subClassOf>
            <owl:Restriction>
                <owl:onProperty rdf:resource="&teddy;TR_0012"/>
                <owl:someValuesFrom rdf:resource="&teddy;TEDDY_0000106"/>
            </owl:Restriction>
        </rdfs:subClassOf>
        <rdfs:seeAlso rdf:datatype="&xsd;anyURI">https://identifiers.org/isbn/0738204536</rdfs:seeAlso>
        <skos:definition xml:lang="en">A cycle which is surrounded by other cycles.</skos:definition>
        <skos:altLabel xml:lang="en">neutrally stable cycle</skos:altLabel>
    </owl:Class>
    <owl:Axiom>
        <owl:annotatedTarget rdf:datatype="&xsd;anyURI">https://identifiers.org/isbn/0738204536</owl:annotatedTarget>
        <rdfs:comment xml:lang="en">Strogatz SH. (2000) Nonlinear dynamics and chaos: with applications to physics, biology, chemistry, and engineering, Westview Press, Cambridge, MA. (p.196)</rdfs:comment>
        <owl:annotatedSource rdf:resource="&teddy;TEDDY_0000106"/>
        <owl:annotatedProperty rdf:resource="&rdfs;seeAlso"/>
    </owl:Axiom>
    


    <!-- http://biomodels.net/teddy/TEDDY#TEDDY_0000107 -->

    <owl:Class rdf:about="&teddy;TEDDY_0000107">
        <rdfs:label xml:lang="en">temporal behaviour ((obsolete))</rdfs:label>
        <rdfs:subClassOf rdf:resource="&teddy;TEDDY_obsolete"/>
        <owl:deprecated rdf:datatype="&xsd;boolean">true</owl:deprecated>
        <skos:definition xml:lang="en">Obsolete: equivalent to TEDDY_0000083 &apos;Temporal Behaviour&apos;.</skos:definition>
    </owl:Class>
    


    <!-- http://biomodels.net/teddy/TEDDY#TEDDY_0000108 -->

    <owl:Class rdf:about="&teddy;TEDDY_0000108">
        <rdfs:label xml:lang="en">perturbation response</rdfs:label>
        <rdfs:subClassOf rdf:resource="&teddy;TEDDY_0000132"/>
        <skos:definition xml:lang="en">A response to perturbations of the system or its environment.</skos:definition>
    </owl:Class>
    


    <!-- http://biomodels.net/teddy/TEDDY#TEDDY_0000109 -->

    <owl:Class rdf:about="&teddy;TEDDY_0000109">
        <rdfs:label xml:lang="en">monostable perturbation response</rdfs:label>
        <rdfs:subClassOf rdf:resource="&teddy;TEDDY_0000108"/>
        <rdfs:seeAlso rdf:datatype="&xsd;anyURI">https://identifiers.org/doi/10.1371/journal.pone.0021782</rdfs:seeAlso>
        <skos:definition xml:lang="en">A `perturbation response` [https://identifiers.org/biomodels.teddy/TEDDY_0000108] shown by a system with a single attractor [https://identifiers.org/biomodels.teddy/TEDDY_0000094]. For all initial states sufficiently near to the attractor the system tend to this attractor.</skos:definition>
    </owl:Class>
    <owl:Axiom>
        <owl:annotatedTarget rdf:datatype="&xsd;anyURI">https://identifiers.org/doi/10.1371/journal.pone.0021782</owl:annotatedTarget>
        <rdfs:comment xml:lang="en">T. Malashchenko, et al. (2011). `Six types of multistability in a neuronal model based on slow calcium current.&apos;. PloS one 6(7):e21782+.</rdfs:comment>
        <owl:annotatedSource rdf:resource="&teddy;TEDDY_0000109"/>
        <owl:annotatedProperty rdf:resource="&rdfs;seeAlso"/>
    </owl:Axiom>
    


    <!-- http://biomodels.net/teddy/TEDDY#TEDDY_0000110 -->

    <owl:Class rdf:about="&teddy;TEDDY_0000110">
        <rdfs:label xml:lang="en">bistable perturbation response</rdfs:label>
        <rdfs:subClassOf rdf:resource="&teddy;TEDDY_0000108"/>
        <rdfs:seeAlso rdf:datatype="&xsd;anyURI">https://identifiers.org/doi/10.1371/journal.pone.0021782</rdfs:seeAlso>
        <skos:definition xml:lang="en">A `perturbation response` [https://identifiers.org/biomodels.teddy/TEDDY_0000108] shown by a system with two different attractors [https://identifiers.org/biomodels.teddy/TEDDY_0000094]. Depending on the initial state the system tend to the one or the other attractor.</skos:definition>
    </owl:Class>
    <owl:Axiom>
        <owl:annotatedTarget rdf:datatype="&xsd;anyURI">https://identifiers.org/doi/10.1371/journal.pone.0021782</owl:annotatedTarget>
        <rdfs:comment xml:lang="en">T. Malashchenko, et al. (2011). `Six types of multistability in a neuronal model based on slow calcium current.&apos;. PloS one 6(7):e21782+.</rdfs:comment>
        <owl:annotatedSource rdf:resource="&teddy;TEDDY_0000110"/>
        <owl:annotatedProperty rdf:resource="&rdfs;seeAlso"/>
    </owl:Axiom>
    


    <!-- http://biomodels.net/teddy/TEDDY#TEDDY_0000111 -->

    <owl:Class rdf:about="&teddy;TEDDY_0000111">
        <rdfs:label xml:lang="en">multistable perturbation response</rdfs:label>
        <rdfs:subClassOf rdf:resource="&teddy;TEDDY_0000108"/>
        <rdfs:seeAlso rdf:datatype="&xsd;anyURI">https://identifiers.org/doi/10.1371/journal.pone.0021782</rdfs:seeAlso>
        <skos:definition xml:lang="en">A `perturbation response` [https://identifiers.org/biomodels.teddy/TEDDY_0000108] shown by a system with more than two different attractors [https://identifiers.org/biomodels.teddy/TEDDY_0000094]. Depending on the initial state the system tend to one of the attractors.</skos:definition>
    </owl:Class>
    <owl:Axiom>
        <owl:annotatedTarget rdf:datatype="&xsd;anyURI">https://identifiers.org/doi/10.1371/journal.pone.0021782</owl:annotatedTarget>
        <rdfs:comment xml:lang="en">T. Malashchenko, et al. (2011). `Six types of multistability in a neuronal model based on slow calcium current.&apos;. PloS one 6(7):e21782+.</rdfs:comment>
        <owl:annotatedSource rdf:resource="&teddy;TEDDY_0000111"/>
        <owl:annotatedProperty rdf:resource="&rdfs;seeAlso"/>
    </owl:Axiom>
    


    <!-- http://biomodels.net/teddy/TEDDY#TEDDY_0000112 -->

    <owl:Class rdf:about="&teddy;TEDDY_0000112">
        <rdfs:label xml:lang="en">quasi-periodic oscillation</rdfs:label>
        <rdfs:subClassOf rdf:resource="&teddy;TEDDY_0000006"/>
        <rdfs:seeAlso rdf:datatype="&xsd;anyURI">http://eom.springer.de/Q/q076630.htm</rdfs:seeAlso>
        <rdfs:seeAlso rdf:datatype="&xsd;anyURI">https://identifiers.org/isbn/0738204536</rdfs:seeAlso>
        <rdfs:seeAlso rdf:datatype="&xsd;anyURI">http://www.scholarpedia.org/article/Quasiperiodic_oscillations</rdfs:seeAlso>
        <skos:altLabel xml:lang="en">QPO</skos:altLabel>
        <skos:definition xml:lang="en">Quasi-periodic oscillation is an oscillation [https://identifiers.org/biomodels.teddy/TEDDY_0000006] that can be described by a quasiperiodic function, i.e. a function f such that f(t)=F(t,...,t) for some continuous function F(t1,...,tn) of n variables that is periodic with respect to t1,...,tn with periods w1,...,wn, respectively. All the w1,...,wn are required to be strictly positive and their reciprocals p1,...,pn have to be rationally linearly independent.</skos:definition>
        <skos:altLabel xml:lang="en">quasiperiodic oscillation</skos:altLabel>
    </owl:Class>
    <owl:Axiom>
        <owl:annotatedTarget rdf:datatype="&xsd;anyURI">http://www.scholarpedia.org/article/Quasiperiodic_oscillations</owl:annotatedTarget>
        <rdfs:comment xml:lang="en">Anatoly M. Samoilenko (2007) Quasiperiodic oscillations. Scholarpedia, 2(5):1783.</rdfs:comment>
        <owl:annotatedSource rdf:resource="&teddy;TEDDY_0000112"/>
        <owl:annotatedProperty rdf:resource="&rdfs;seeAlso"/>
    </owl:Axiom>
    <owl:Axiom>
        <owl:annotatedTarget rdf:datatype="&xsd;anyURI">http://eom.springer.de/Q/q076630.htm</owl:annotatedTarget>
        <rdfs:comment xml:lang="en">Encyclopaedia of Mathematics, edited by Michiel Hazewinkel, CWI, Amsterdam.</rdfs:comment>
        <owl:annotatedSource rdf:resource="&teddy;TEDDY_0000112"/>
        <owl:annotatedProperty rdf:resource="&rdfs;seeAlso"/>
    </owl:Axiom>
    <owl:Axiom>
        <owl:annotatedTarget rdf:datatype="&xsd;anyURI">https://identifiers.org/isbn/0738204536</owl:annotatedTarget>
        <rdfs:comment xml:lang="en">Strogatz SH. (2000) Nonlinear dynamics and chaos: with applications to physics, biology, chemistry, and engineering, Westview Press, Cambridge, MA. (p.276)</rdfs:comment>
        <owl:annotatedSource rdf:resource="&teddy;TEDDY_0000112"/>
        <owl:annotatedProperty rdf:resource="&rdfs;seeAlso"/>
    </owl:Axiom>
    


    <!-- http://biomodels.net/teddy/TEDDY#TEDDY_0000113 -->

    <owl:Class rdf:about="&teddy;TEDDY_0000113">
        <rdfs:label xml:lang="en">stable fixed point ((obsolete))</rdfs:label>
        <rdfs:subClassOf rdf:resource="&teddy;TEDDY_obsolete"/>
        <rdfs:seeAlso rdf:datatype="&xsd;anyURI">https://identifiers.org/isbn/0738204536</rdfs:seeAlso>
        <owl:deprecated rdf:datatype="&xsd;boolean">true</owl:deprecated>
        <skos:altLabel xml:lang="en">Attractor</skos:altLabel>
        <skos:definition xml:lang="en">Obsolete: a fixed point which is stable.</skos:definition>
        <skos:altLabel xml:lang="en">Sink</skos:altLabel>
    </owl:Class>
    <owl:Axiom>
        <owl:annotatedTarget rdf:datatype="&xsd;anyURI">https://identifiers.org/isbn/0738204536</owl:annotatedTarget>
        <rdfs:comment xml:lang="en">Strogatz SH. (2000) Nonlinear dynamics and chaos: with applications to physics, biology, chemistry, and engineering, Westview Press, Cambridge, MA. (p.17)</rdfs:comment>
        <owl:annotatedSource rdf:resource="&teddy;TEDDY_0000113"/>
        <owl:annotatedProperty rdf:resource="&rdfs;seeAlso"/>
    </owl:Axiom>
    


    <!-- http://biomodels.net/teddy/TEDDY#TEDDY_0000114 -->

    <owl:Class rdf:about="&teddy;TEDDY_0000114">
        <rdfs:label xml:lang="en">stable limit cycle</rdfs:label>
        <rdfs:subClassOf rdf:resource="&teddy;TEDDY_0000051"/>
        <rdfs:subClassOf>
            <owl:Restriction>
                <owl:onProperty rdf:resource="&teddy;TEDDY_0000174"/>
                <owl:someValuesFrom rdf:resource="&teddy;TEDDY_0000034"/>
            </owl:Restriction>
        </rdfs:subClassOf>
        <rdfs:subClassOf>
            <owl:Restriction>
                <owl:onProperty rdf:resource="&teddy;TR_0004"/>
                <owl:someValuesFrom rdf:resource="&teddy;TEDDY_0000149"/>
            </owl:Restriction>
        </rdfs:subClassOf>
        <rdfs:subClassOf>
            <owl:Restriction>
                <owl:onProperty rdf:resource="&teddy;TR_0004"/>
                <owl:someValuesFrom rdf:resource="&teddy;TEDDY_0000097"/>
            </owl:Restriction>
        </rdfs:subClassOf>
        <rdfs:seeAlso rdf:datatype="&xsd;anyURI">https://identifiers.org/isbn/0738204536</rdfs:seeAlso>
        <skos:definition xml:lang="en">If all the neighbouring paths [https://identifiers.org/biomodels.teddy/TEDDY_0000083] approach the limit cycle [https://identifiers.org/biomodels.teddy/TEDDY_0000051] then it is stable.</skos:definition>
    </owl:Class>
    <owl:Axiom>
        <owl:annotatedTarget rdf:datatype="&xsd;anyURI">https://identifiers.org/isbn/0738204536</owl:annotatedTarget>
        <rdfs:comment xml:lang="en">Strogatz SH. (2000) Nonlinear dynamics and chaos: with applications to physics, biology, chemistry, and engineering, Westview Press, Cambridge, MA. (p.196)</rdfs:comment>
        <owl:annotatedSource rdf:resource="&teddy;TEDDY_0000114"/>
        <owl:annotatedProperty rdf:resource="&rdfs;seeAlso"/>
    </owl:Axiom>
    


    <!-- http://biomodels.net/teddy/TEDDY#TEDDY_0000115 -->

    <owl:Class rdf:about="&teddy;TEDDY_0000115">
        <rdfs:label xml:lang="en">neutrally stable fixed point</rdfs:label>
        <owl:equivalentClass>
            <owl:Class>
                <owl:intersectionOf rdf:parseType="Collection">
                    <rdf:Description rdf:about="&teddy;TEDDY_0000086"/>
                    <owl:Restriction>
                        <owl:onProperty rdf:resource="&teddy;TR_0004"/>
                        <owl:someValuesFrom rdf:resource="&teddy;TEDDY_0000098"/>
                    </owl:Restriction>
                </owl:intersectionOf>
            </owl:Class>
        </owl:equivalentClass>
        <rdfs:seeAlso rdf:datatype="&xsd;anyURI">https://identifiers.org/isbn/0738204536</rdfs:seeAlso>
        <skos:definition xml:lang="en">A &apos;fixed point&apos; [https://identifiers.org/biomodels.teddy/TEDDY_0000086] which is neutrally stable [https://identifiers.org/biomodels.teddy/TEDDY_0000098].</skos:definition>
    </owl:Class>
    <owl:Axiom>
        <owl:annotatedTarget rdf:datatype="&xsd;anyURI">https://identifiers.org/isbn/0738204536</owl:annotatedTarget>
        <rdfs:comment xml:lang="en">Strogatz SH. (2000) Nonlinear dynamics and chaos: with applications to physics, biology, chemistry, and engineering, Westview Press, Cambridge, MA. (p.129)</rdfs:comment>
        <owl:annotatedSource rdf:resource="&teddy;TEDDY_0000115"/>
        <owl:annotatedProperty rdf:resource="&rdfs;seeAlso"/>
    </owl:Axiom>
    


    <!-- http://biomodels.net/teddy/TEDDY#TEDDY_0000116 -->

    <owl:Class rdf:about="&teddy;TEDDY_0000116">
        <rdfs:label xml:lang="en">magnitude</rdfs:label>
        <rdfs:subClassOf rdf:resource="&teddy;TEDDY_0000178"/>
        <skos:definition xml:lang="en">A size of an object.</skos:definition>
    </owl:Class>
    


    <!-- http://biomodels.net/teddy/TEDDY#TEDDY_0000117 -->

    <owl:Class rdf:about="&teddy;TEDDY_0000117">
        <rdfs:label xml:lang="en">high magnitude</rdfs:label>
        <rdfs:subClassOf rdf:resource="&teddy;TEDDY_0000116"/>
        <owl:disjointWith rdf:resource="&teddy;TEDDY_0000118"/>
        <skos:definition xml:lang="en">A magnitude that is much higher than the expected one.</skos:definition>
    </owl:Class>
    


    <!-- http://biomodels.net/teddy/TEDDY#TEDDY_0000118 -->

    <owl:Class rdf:about="&teddy;TEDDY_0000118">
        <rdfs:label xml:lang="en">low magnitude</rdfs:label>
        <rdfs:subClassOf rdf:resource="&teddy;TEDDY_0000116"/>
        <skos:definition xml:lang="en">A magnitude that is much lower than the expected one.</skos:definition>
    </owl:Class>
    


    <!-- http://biomodels.net/teddy/TEDDY#TEDDY_0000119 -->

    <owl:Class rdf:about="&teddy;TEDDY_0000119">
        <rdfs:label xml:lang="en">saddle-node homoclinic bifurcation</rdfs:label>
        <rdfs:subClassOf rdf:resource="&teddy;TEDDY_0000147"/>
        <rdfs:subClassOf>
            <owl:Restriction>
                <owl:onProperty rdf:resource="&teddy;TR_0017"/>
                <owl:someValuesFrom rdf:resource="&teddy;TEDDY_0000051"/>
            </owl:Restriction>
        </rdfs:subClassOf>
        <rdfs:subClassOf>
            <owl:Restriction>
                <owl:onProperty rdf:resource="&teddy;TR_0018"/>
                <owl:someValuesFrom rdf:resource="&teddy;TEDDY_0000089"/>
            </owl:Restriction>
        </rdfs:subClassOf>
        <rdfs:seeAlso rdf:datatype="&xsd;anyURI">https://identifiers.org/isbn/0387983821</rdfs:seeAlso>
        <skos:definition xml:lang="en">A global bifurcation [https://identifiers.org/biomodels.teddy/TEDDY_0000147] in which node [https://identifiers.org/biomodels.teddy/TEDDY_0000087] and a saddle [https://identifiers.org/biomodels.teddy/TEDDY_0000089] collide to a saddle [https://identifiers.org/biomodels.teddy/TEDDY_0000089] at the bifurcation point, connected by a homoclinic saddle connection [https://identifiers.org/biomodels.teddy/TEDDY_0000100]. Above the bifurcation point a limit cycle [https://identifiers.org/biomodels.teddy/TEDDY_0000051] appears and the saddle [https://identifiers.org/biomodels.teddy/TEDDY_0000089] vanishes. The period of this cycle tends to infinity as the parameter approaches its bifurcation value.</skos:definition>
        <skos:altLabel xml:lang="en">infinite period bifurcation</skos:altLabel>
    </owl:Class>
    <owl:Axiom>
        <owl:annotatedTarget rdf:datatype="&xsd;anyURI">https://identifiers.org/isbn/0387983821</owl:annotatedTarget>
        <rdfs:comment xml:lang="en">Kuznetsov YA. (1988) Elements of applied bifurcation theory, Springer, New York. (p.59ff)</rdfs:comment>
        <owl:annotatedSource rdf:resource="&teddy;TEDDY_0000119"/>
        <owl:annotatedProperty rdf:resource="&rdfs;seeAlso"/>
    </owl:Axiom>
    <owl:Axiom>
        <rdfs:seeAlso rdf:datatype="&xsd;anyURI">https://identifiers.org/isbn/0738204536 (p.262)</rdfs:seeAlso>
        <owl:annotatedTarget xml:lang="en">infinite period bifurcation</owl:annotatedTarget>
        <owl:annotatedSource rdf:resource="&teddy;TEDDY_0000119"/>
        <owl:annotatedProperty rdf:resource="&skos;altLabel"/>
    </owl:Axiom>
    


    <!-- http://biomodels.net/teddy/TEDDY#TEDDY_0000120 -->

    <owl:Class rdf:about="&teddy;TEDDY_0000120">
        <rdfs:label xml:lang="en">degenerate Hopf bifurcation</rdfs:label>
        <rdfs:subClassOf rdf:resource="&teddy;TEDDY_0000072"/>
        <rdfs:subClassOf>
            <owl:Class>
                <owl:complementOf>
                    <owl:Restriction>
                        <owl:onProperty rdf:resource="&teddy;TR_0018"/>
                        <owl:someValuesFrom rdf:resource="&teddy;TEDDY_0000051"/>
                    </owl:Restriction>
                </owl:complementOf>
            </owl:Class>
        </rdfs:subClassOf>
        <rdfs:subClassOf>
            <owl:Class>
                <owl:complementOf>
                    <owl:Restriction>
                        <owl:onProperty rdf:resource="&teddy;TR_0017"/>
                        <owl:someValuesFrom rdf:resource="&teddy;TEDDY_0000051"/>
                    </owl:Restriction>
                </owl:complementOf>
            </owl:Class>
        </rdfs:subClassOf>
        <rdfs:seeAlso rdf:datatype="&xsd;anyURI">https://identifiers.org/isbn/0738204536</rdfs:seeAlso>
        <skos:definition xml:lang="en">A `Hopf bifurcation` [https://identifiers.org/biomodels.teddy/TEDDY_0000072] in which neigther a limit cycle [https://identifiers.org/biomodels.teddy/TEDDY_0000051] is destroyed nor a limit cycle [https://identifiers.org/biomodels.teddy/TEDDY_0000051] appears. On the bifurcation the fixed point [https://identifiers.org/biomodels.teddy/TEDDY_0000086] is a `center` [https://identifiers.org/biomodels.teddy/TEDDY_0000088].</skos:definition>
    </owl:Class>
    <owl:Axiom>
        <owl:annotatedTarget rdf:datatype="&xsd;anyURI">https://identifiers.org/isbn/0738204536</owl:annotatedTarget>
        <rdfs:comment xml:lang="en">Strogatz SH. (2000) Nonlinear dynamics and chaos: with applications to physics, biology, chemistry, and engineering, Westview Press, Cambridge, MA. (p.253)</rdfs:comment>
        <owl:annotatedSource rdf:resource="&teddy;TEDDY_0000120"/>
        <owl:annotatedProperty rdf:resource="&rdfs;seeAlso"/>
    </owl:Axiom>
    


    <!-- http://biomodels.net/teddy/TEDDY#TEDDY_0000121 -->

    <owl:Class rdf:about="&teddy;TEDDY_0000121">
        <rdfs:label xml:lang="en">transcritical bifurcation</rdfs:label>
        <rdfs:subClassOf rdf:resource="&teddy;TEDDY_0000123"/>
        <rdfs:subClassOf>
            <owl:Class>
                <owl:unionOf rdf:parseType="Collection">
                    <owl:Class>
                        <owl:intersectionOf rdf:parseType="Collection">
                            <owl:Restriction>
                                <owl:onProperty rdf:resource="&teddy;TR_0017"/>
                                <owl:onClass rdf:resource="&teddy;TEDDY_0000095"/>
                                <owl:qualifiedCardinality rdf:datatype="&xsd;nonNegativeInteger">1</owl:qualifiedCardinality>
                            </owl:Restriction>
                            <owl:Restriction>
                                <owl:onProperty rdf:resource="&teddy;TR_0018"/>
                                <owl:onClass rdf:resource="&teddy;TEDDY_0000129"/>
                                <owl:qualifiedCardinality rdf:datatype="&xsd;nonNegativeInteger">1</owl:qualifiedCardinality>
                            </owl:Restriction>
                        </owl:intersectionOf>
                    </owl:Class>
                    <owl:Class>
                        <owl:intersectionOf rdf:parseType="Collection">
                            <owl:Restriction>
                                <owl:onProperty rdf:resource="&teddy;TR_0017"/>
                                <owl:onClass rdf:resource="&teddy;TEDDY_0000129"/>
                                <owl:qualifiedCardinality rdf:datatype="&xsd;nonNegativeInteger">1</owl:qualifiedCardinality>
                            </owl:Restriction>
                            <owl:Restriction>
                                <owl:onProperty rdf:resource="&teddy;TR_0018"/>
                                <owl:onClass rdf:resource="&teddy;TEDDY_0000095"/>
                                <owl:qualifiedCardinality rdf:datatype="&xsd;nonNegativeInteger">1</owl:qualifiedCardinality>
                            </owl:Restriction>
                        </owl:intersectionOf>
                    </owl:Class>
                </owl:unionOf>
            </owl:Class>
        </rdfs:subClassOf>
        <rdfs:seeAlso rdf:datatype="&xsd;anyURI">https://identifiers.org/isbn/0738204536</rdfs:seeAlso>
        <skos:definition xml:lang="en">A `zero-eigenvalue bifurcation` [https://identifiers.org/biomodels.teddy/TEDDY_0000123] in which a stable [https://identifiers.org/biomodels.teddy/TEDDY_0000133] fixed point [https://identifiers.org/biomodels.teddy/TEDDY_0000086] and an unstable [not TEDDY_0000133] fixed point [https://identifiers.org/biomodels.teddy/TEDDY_0000086] coalesce and exchange their stability.</skos:definition>
    </owl:Class>
    <owl:Axiom>
        <owl:annotatedTarget rdf:datatype="&xsd;anyURI">https://identifiers.org/isbn/0738204536</owl:annotatedTarget>
        <rdfs:comment xml:lang="en">Strogatz SH. (2000) Nonlinear dynamics and chaos: with applications to physics, biology, chemistry, and engineering, Westview Press, Cambridge, MA. (p.50f)</rdfs:comment>
        <owl:annotatedSource rdf:resource="&teddy;TEDDY_0000121"/>
        <owl:annotatedProperty rdf:resource="&rdfs;seeAlso"/>
    </owl:Axiom>
    


    <!-- http://biomodels.net/teddy/TEDDY#TEDDY_0000122 -->

    <owl:Class rdf:about="&teddy;TEDDY_0000122">
        <rdfs:label xml:lang="en">pitchfork bifurcation</rdfs:label>
        <rdfs:subClassOf rdf:resource="&teddy;TEDDY_0000123"/>
        <rdfs:subClassOf>
            <owl:Class>
                <owl:unionOf rdf:parseType="Collection">
                    <owl:Restriction>
                        <owl:onProperty rdf:resource="&teddy;TR_0017"/>
                        <owl:onClass rdf:resource="&teddy;TEDDY_0000086"/>
                        <owl:minQualifiedCardinality rdf:datatype="&xsd;nonNegativeInteger">2</owl:minQualifiedCardinality>
                    </owl:Restriction>
                    <owl:Restriction>
                        <owl:onProperty rdf:resource="&teddy;TR_0018"/>
                        <owl:onClass rdf:resource="&teddy;TEDDY_0000086"/>
                        <owl:minQualifiedCardinality rdf:datatype="&xsd;nonNegativeInteger">2</owl:minQualifiedCardinality>
                    </owl:Restriction>
                </owl:unionOf>
            </owl:Class>
        </rdfs:subClassOf>
        <rdfs:seeAlso rdf:datatype="&xsd;anyURI">https://identifiers.org/isbn/0738204536</rdfs:seeAlso>
        <skos:definition xml:lang="en">A `zero-eigenvalue bifurcation` [https://identifiers.org/biomodels.teddy/TEDDY_0000123] in which the fixed point [https://identifiers.org/biomodels.teddy/TEDDY_0000086] is surrounded by two symmetrical fixed points on one side of the bifurcation.</skos:definition>
        <skos:altLabel xml:lang="en">flip bifurcation</skos:altLabel>
    </owl:Class>
    <owl:Axiom>
        <owl:annotatedTarget rdf:datatype="&xsd;anyURI">https://identifiers.org/isbn/0738204536</owl:annotatedTarget>
        <rdfs:comment xml:lang="en">Strogatz SH. (2000) Nonlinear dynamics and chaos: with applications to physics, biology, chemistry, and engineering, Westview Press, Cambridge, MA. (p.55)</rdfs:comment>
        <owl:annotatedSource rdf:resource="&teddy;TEDDY_0000122"/>
        <owl:annotatedProperty rdf:resource="&rdfs;seeAlso"/>
    </owl:Axiom>
    <owl:Axiom>
        <rdfs:comment rdf:datatype="&xsd;anyURI">https://identifiers.org/isbn/0198565623 (p.432)</rdfs:comment>
        <owl:annotatedTarget xml:lang="en">flip bifurcation</owl:annotatedTarget>
        <owl:annotatedSource rdf:resource="&teddy;TEDDY_0000122"/>
        <owl:annotatedProperty rdf:resource="&skos;altLabel"/>
    </owl:Axiom>
    


    <!-- http://biomodels.net/teddy/TEDDY#TEDDY_0000123 -->

    <owl:Class rdf:about="&teddy;TEDDY_0000123">
        <rdfs:label xml:lang="en">zero-eigenvalue bifurcation</rdfs:label>
        <rdfs:subClassOf rdf:resource="&teddy;TEDDY_0000069"/>
        <rdfs:seeAlso rdf:datatype="&xsd;anyURI">https://identifiers.org/isbn/0738204536</rdfs:seeAlso>
        <skos:definition xml:lang="en">A `local bifurcation` [https://identifiers.org/biomodels.teddy/TEDDY_0000069] in which one of the eigenvalue of the linarisation around the fixed point [https://identifiers.org/biomodels.teddy/TEDDY_0000086] is zero at the bifurcation.</skos:definition>
    </owl:Class>
    <owl:Axiom>
        <owl:annotatedTarget rdf:datatype="&xsd;anyURI">https://identifiers.org/isbn/0738204536</owl:annotatedTarget>
        <rdfs:comment xml:lang="en">Strogatz SH. (2000) Nonlinear dynamics and chaos: with applications to physics, biology, chemistry, and engineering, Westview Press, Cambridge, MA. (p.248)</rdfs:comment>
        <owl:annotatedSource rdf:resource="&teddy;TEDDY_0000123"/>
        <owl:annotatedProperty rdf:resource="&rdfs;seeAlso"/>
    </owl:Axiom>
    


    <!-- http://biomodels.net/teddy/TEDDY#TEDDY_0000124 -->

    <owl:Class rdf:about="&teddy;TEDDY_0000124">
        <rdfs:label xml:lang="en">subcritical pitchfork bifurcation</rdfs:label>
        <rdfs:subClassOf rdf:resource="&teddy;TEDDY_0000122"/>
        <rdfs:subClassOf>
            <owl:Class>
                <owl:intersectionOf rdf:parseType="Collection">
                    <owl:Restriction>
                        <owl:onProperty rdf:resource="&teddy;TR_0017"/>
                        <owl:onClass rdf:resource="&teddy;TEDDY_0000095"/>
                        <owl:qualifiedCardinality rdf:datatype="&xsd;nonNegativeInteger">1</owl:qualifiedCardinality>
                    </owl:Restriction>
                    <owl:Restriction>
                        <owl:onProperty rdf:resource="&teddy;TR_0018"/>
                        <owl:onClass rdf:resource="&teddy;TEDDY_0000129"/>
                        <owl:qualifiedCardinality rdf:datatype="&xsd;nonNegativeInteger">1</owl:qualifiedCardinality>
                    </owl:Restriction>
                    <owl:Restriction>
                        <owl:onProperty rdf:resource="&teddy;TR_0018"/>
                        <owl:onClass rdf:resource="&teddy;TEDDY_0000095"/>
                        <owl:qualifiedCardinality rdf:datatype="&xsd;nonNegativeInteger">2</owl:qualifiedCardinality>
                    </owl:Restriction>
                </owl:intersectionOf>
            </owl:Class>
        </rdfs:subClassOf>
        <owl:disjointWith rdf:resource="&teddy;TEDDY_0000125"/>
        <rdfs:seeAlso rdf:datatype="&xsd;anyURI">https://identifiers.org/isbn/0738204536</rdfs:seeAlso>
        <skos:definition xml:lang="en">A `pitchfork bifurcation` [https://identifiers.org/biomodels.teddy/TEDDY_0000122] in which two symmetrical stable [https://identifiers.org/biomodels.teddy/TEDDY_0000133] fixed points [https://identifiers.org/biomodels.teddy/TEDDY_0000086] collide with an unstable [not TEDDY_0000133] fixed point [https://identifiers.org/biomodels.teddy/TEDDY_0000086] and dissapear, while the unstable fixed point transforms into a stable one.</skos:definition>
    </owl:Class>
    <owl:Axiom>
        <owl:annotatedTarget rdf:datatype="&xsd;anyURI">https://identifiers.org/isbn/0738204536</owl:annotatedTarget>
        <rdfs:comment xml:lang="en">Strogatz SH. (2000) Nonlinear dynamics and chaos: with applications to physics, biology, chemistry, and engineering, Westview Press, Cambridge, MA. (p.58f)</rdfs:comment>
        <owl:annotatedSource rdf:resource="&teddy;TEDDY_0000124"/>
        <owl:annotatedProperty rdf:resource="&rdfs;seeAlso"/>
    </owl:Axiom>
    


    <!-- http://biomodels.net/teddy/TEDDY#TEDDY_0000125 -->

    <owl:Class rdf:about="&teddy;TEDDY_0000125">
        <rdfs:label xml:lang="en">supercritical pitchfork bifurcation</rdfs:label>
        <rdfs:subClassOf rdf:resource="&teddy;TEDDY_0000122"/>
        <rdfs:subClassOf>
            <owl:Class>
                <owl:intersectionOf rdf:parseType="Collection">
                    <owl:Restriction>
                        <owl:onProperty rdf:resource="&teddy;TR_0017"/>
                        <owl:onClass rdf:resource="&teddy;TEDDY_0000129"/>
                        <owl:qualifiedCardinality rdf:datatype="&xsd;nonNegativeInteger">1</owl:qualifiedCardinality>
                    </owl:Restriction>
                    <owl:Restriction>
                        <owl:onProperty rdf:resource="&teddy;TR_0017"/>
                        <owl:onClass rdf:resource="&teddy;TEDDY_0000095"/>
                        <owl:qualifiedCardinality rdf:datatype="&xsd;nonNegativeInteger">2</owl:qualifiedCardinality>
                    </owl:Restriction>
                    <owl:Restriction>
                        <owl:onProperty rdf:resource="&teddy;TR_0018"/>
                        <owl:onClass rdf:resource="&teddy;TEDDY_0000095"/>
                        <owl:qualifiedCardinality rdf:datatype="&xsd;nonNegativeInteger">1</owl:qualifiedCardinality>
                    </owl:Restriction>
                </owl:intersectionOf>
            </owl:Class>
        </rdfs:subClassOf>
        <rdfs:seeAlso rdf:datatype="&xsd;anyURI">https://identifiers.org/isbn/0738204536</rdfs:seeAlso>
        <skos:definition xml:lang="en">A `pitchfork bifurcation` [https://identifiers.org/biomodels.teddy/TEDDY_0000122] in which two symmetrical stable [https://identifiers.org/biomodels.teddy/TEDDY_0000133] fixed points [https://identifiers.org/biomodels.teddy/TEDDY_0000086] and an unstable [not TEDDY_0000133] fixed point [https://identifiers.org/biomodels.teddy/TEDDY_0000086] appear from a stable fixed point.</skos:definition>
    </owl:Class>
    <owl:Axiom>
        <owl:annotatedTarget rdf:datatype="&xsd;anyURI">https://identifiers.org/isbn/0738204536</owl:annotatedTarget>
        <rdfs:comment xml:lang="en">Strogatz SH. (2000) Nonlinear dynamics and chaos: with applications to physics, biology, chemistry, and engineering, Westview Press, Cambridge, MA. (p.55f)</rdfs:comment>
        <owl:annotatedSource rdf:resource="&teddy;TEDDY_0000125"/>
        <owl:annotatedProperty rdf:resource="&rdfs;seeAlso"/>
    </owl:Axiom>
    


    <!-- http://biomodels.net/teddy/TEDDY#TEDDY_0000126 -->

    <owl:Class rdf:about="&teddy;TEDDY_0000126">
        <rdfs:label xml:lang="en">stable spiral</rdfs:label>
        <rdfs:subClassOf rdf:resource="&teddy;TEDDY_0000091"/>
        <rdfs:subClassOf>
            <owl:Restriction>
                <owl:onProperty rdf:resource="&teddy;TR_0004"/>
                <owl:someValuesFrom rdf:resource="&teddy;TEDDY_0000149"/>
            </owl:Restriction>
        </rdfs:subClassOf>
        <rdfs:subClassOf>
            <owl:Restriction>
                <owl:onProperty rdf:resource="&teddy;TR_0004"/>
                <owl:someValuesFrom rdf:resource="&teddy;TEDDY_0000150"/>
            </owl:Restriction>
        </rdfs:subClassOf>
        <rdfs:subClassOf>
            <owl:Restriction>
                <owl:onProperty rdf:resource="&teddy;TR_0004"/>
                <owl:someValuesFrom rdf:resource="&teddy;TEDDY_0000097"/>
            </owl:Restriction>
        </rdfs:subClassOf>
        <rdfs:seeAlso rdf:datatype="&xsd;anyURI">https://identifiers.org/isbn/0738204536</rdfs:seeAlso>
        <skos:definition xml:lang="en">A spiral point [https://identifiers.org/biomodels.teddy/TEDDY_0000091] which is stable [https://identifiers.org/biomodels.teddy/TEDDY_0000133], i.e. for which the Jacobian matrix has two negative complex conjugate eigenvalues. The fixed point is surrounded by behaviours [https://identifiers.org/biomodels.teddy/TEDDY_0000083] spiralling downward the fixed point, corresponding to decaying oscillations.</skos:definition>
        <skos:altLabel xml:lang="en">spiral sink</skos:altLabel>
        <skos:altLabel xml:lang="en">stable focus</skos:altLabel>
        <skos:altLabel xml:lang="en">stable spiral point</skos:altLabel>
    </owl:Class>
    <owl:Axiom>
        <rdfs:seeAlso rdf:datatype="&xsd;anyURI">https://identifiers.org/isbn/0198565623 (p.73)</rdfs:seeAlso>
        <owl:annotatedTarget xml:lang="en">stable spiral point</owl:annotatedTarget>
        <owl:annotatedSource rdf:resource="&teddy;TEDDY_0000126"/>
        <owl:annotatedProperty rdf:resource="&skos;altLabel"/>
    </owl:Axiom>
    <owl:Axiom>
        <owl:annotatedTarget rdf:datatype="&xsd;anyURI">https://identifiers.org/isbn/0738204536</owl:annotatedTarget>
        <rdfs:comment xml:lang="en">Strogatz SH. (2000) Nonlinear dynamics and chaos: with applications to physics, biology, chemistry, and engineering, Westview Press, Cambridge, MA. (pp.134,137)</rdfs:comment>
        <owl:annotatedSource rdf:resource="&teddy;TEDDY_0000126"/>
        <owl:annotatedProperty rdf:resource="&rdfs;seeAlso"/>
    </owl:Axiom>
    <owl:Axiom>
        <rdfs:seeAlso rdf:datatype="&xsd;anyURI">https://identifiers.org/isbn/0198565623 (p.25)</rdfs:seeAlso>
        <owl:annotatedTarget xml:lang="en">stable focus</owl:annotatedTarget>
        <owl:annotatedSource rdf:resource="&teddy;TEDDY_0000126"/>
        <owl:annotatedProperty rdf:resource="&skos;altLabel"/>
    </owl:Axiom>
    


    <!-- http://biomodels.net/teddy/TEDDY#TEDDY_0000127 -->

    <owl:Class rdf:about="&teddy;TEDDY_0000127">
        <rdfs:label xml:lang="en">unstable spiral</rdfs:label>
        <owl:equivalentClass>
            <owl:Restriction>
                <owl:onProperty rdf:resource="&teddy;TR_0015"/>
                <owl:someValuesFrom rdf:resource="&teddy;TEDDY_0000126"/>
            </owl:Restriction>
        </owl:equivalentClass>
        <rdfs:subClassOf rdf:resource="&teddy;TEDDY_0000091"/>
        <rdfs:subClassOf>
            <owl:Class>
                <owl:complementOf>
                    <owl:Restriction>
                        <owl:onProperty rdf:resource="&teddy;TR_0004"/>
                        <owl:someValuesFrom rdf:resource="&teddy;TEDDY_0000149"/>
                    </owl:Restriction>
                </owl:complementOf>
            </owl:Class>
        </rdfs:subClassOf>
        <rdfs:subClassOf>
            <owl:Class>
                <owl:complementOf>
                    <owl:Restriction>
                        <owl:onProperty rdf:resource="&teddy;TR_0004"/>
                        <owl:someValuesFrom rdf:resource="&teddy;TEDDY_0000133"/>
                    </owl:Restriction>
                </owl:complementOf>
            </owl:Class>
        </rdfs:subClassOf>
        <rdfs:seeAlso rdf:datatype="&xsd;anyURI">https://identifiers.org/isbn/0738204536</rdfs:seeAlso>
        <skos:definition xml:lang="en">A spiral point [https://identifiers.org/biomodels.teddy/TEDDY_0000091] which is unstable [not TEDDY_0000133], i.e. for which the Jacobian matrix has two positive complex conjugate eigenvalues. The fixed point is surrounded by behaviours [https://identifiers.org/biomodels.teddy/TEDDY_0000083] spiralling upward the fixed point, corresponding to growing oscillations.</skos:definition>
        <skos:altLabel xml:lang="en">spiral source</skos:altLabel>
        <skos:altLabel xml:lang="en">unstable focus</skos:altLabel>
        <skos:altLabel xml:lang="en">unstable spiral point</skos:altLabel>
    </owl:Class>
    <owl:Axiom>
        <owl:annotatedTarget rdf:datatype="&xsd;anyURI">https://identifiers.org/isbn/0738204536</owl:annotatedTarget>
        <rdfs:comment xml:lang="en">Strogatz SH. (2000) Nonlinear dynamics and chaos: with applications to physics, biology, chemistry, and engineering, Westview Press, Cambridge, MA. (pp.134,137)</rdfs:comment>
        <owl:annotatedSource rdf:resource="&teddy;TEDDY_0000127"/>
        <owl:annotatedProperty rdf:resource="&rdfs;seeAlso"/>
    </owl:Axiom>
    <owl:Axiom>
        <rdfs:seeAlso rdf:datatype="&xsd;anyURI">https://identifiers.org/isbn/0198565623 (p.73)</rdfs:seeAlso>
        <owl:annotatedTarget xml:lang="en">unstable spiral point</owl:annotatedTarget>
        <owl:annotatedSource rdf:resource="&teddy;TEDDY_0000127"/>
        <owl:annotatedProperty rdf:resource="&skos;altLabel"/>
    </owl:Axiom>
    <owl:Axiom>
        <rdfs:seeAlso rdf:datatype="&xsd;anyURI">https://identifiers.org/isbn/0198565623 (p.25)</rdfs:seeAlso>
        <owl:annotatedTarget xml:lang="en">unstable focus</owl:annotatedTarget>
        <owl:annotatedSource rdf:resource="&teddy;TEDDY_0000127"/>
        <owl:annotatedProperty rdf:resource="&skos;altLabel"/>
    </owl:Axiom>
    


    <!-- http://biomodels.net/teddy/TEDDY#TEDDY_0000128 -->

    <owl:Class rdf:about="&teddy;TEDDY_0000128">
        <rdfs:label xml:lang="en">unstable limit cycle</rdfs:label>
        <owl:equivalentClass>
            <owl:Restriction>
                <owl:onProperty rdf:resource="&teddy;TR_0015"/>
                <owl:someValuesFrom rdf:resource="&teddy;TEDDY_0000114"/>
            </owl:Restriction>
        </owl:equivalentClass>
        <rdfs:subClassOf rdf:resource="&teddy;TEDDY_0000051"/>
        <rdfs:subClassOf>
            <owl:Class>
                <owl:complementOf>
                    <owl:Restriction>
                        <owl:onProperty rdf:resource="&teddy;TR_0004"/>
                        <owl:someValuesFrom rdf:resource="&teddy;TEDDY_0000149"/>
                    </owl:Restriction>
                </owl:complementOf>
            </owl:Class>
        </rdfs:subClassOf>
        <rdfs:subClassOf>
            <owl:Class>
                <owl:complementOf>
                    <owl:Restriction>
                        <owl:onProperty rdf:resource="&teddy;TR_0004"/>
                        <owl:someValuesFrom rdf:resource="&teddy;TEDDY_0000133"/>
                    </owl:Restriction>
                </owl:complementOf>
            </owl:Class>
        </rdfs:subClassOf>
        <rdfs:seeAlso rdf:datatype="&xsd;anyURI">https://identifiers.org/isbn/0738204536</rdfs:seeAlso>
        <skos:definition xml:lang="en">If all trajectories [https://identifiers.org/biomodels.teddy/TEDDY_0000083] that start near the limit cycle [https://identifiers.org/biomodels.teddy/TEDDY_0000051] (both inside and outside) spiral outward, then the limit cycle is called unstable.</skos:definition>
    </owl:Class>
    <owl:Axiom>
        <owl:annotatedTarget rdf:datatype="&xsd;anyURI">https://identifiers.org/isbn/0738204536</owl:annotatedTarget>
        <rdfs:comment xml:lang="en">Strogatz SH. (2000) Nonlinear dynamics and chaos: with applications to physics, biology, chemistry, and engineering, Westview Press, Cambridge, MA. (p.196)</rdfs:comment>
        <owl:annotatedSource rdf:resource="&teddy;TEDDY_0000128"/>
        <owl:annotatedProperty rdf:resource="&rdfs;seeAlso"/>
    </owl:Axiom>
    


    <!-- http://biomodels.net/teddy/TEDDY#TEDDY_0000129 -->

    <owl:Class rdf:about="&teddy;TEDDY_0000129">
        <rdfs:label xml:lang="en">unstable fixed point</rdfs:label>
        <owl:equivalentClass>
            <owl:Class>
                <owl:intersectionOf rdf:parseType="Collection">
                    <rdf:Description rdf:about="&teddy;TEDDY_0000086"/>
                    <owl:Class>
                        <owl:complementOf rdf:resource="&teddy;TEDDY_0000095"/>
                    </owl:Class>
                </owl:intersectionOf>
            </owl:Class>
        </owl:equivalentClass>
        <rdfs:subClassOf rdf:resource="&teddy;TEDDY_0000086"/>
        <rdfs:seeAlso rdf:datatype="&xsd;anyURI">https://identifiers.org/isbn/0738204536</rdfs:seeAlso>
        <skos:definition xml:lang="en">A fixed point [https://identifiers.org/biomodels.teddy/TEDDY_0000086] which is not Liapunov stable [not TEDDY_0000113].</skos:definition>
    </owl:Class>
    <owl:Axiom>
        <owl:annotatedTarget rdf:datatype="&xsd;anyURI">https://identifiers.org/isbn/0738204536</owl:annotatedTarget>
        <rdfs:comment xml:lang="en">Strogatz SH. (2000) Nonlinear dynamics and chaos: with applications to physics, biology, chemistry, and engineering, Westview Press, Cambridge, MA. (p.17)</rdfs:comment>
        <owl:annotatedSource rdf:resource="&teddy;TEDDY_0000129"/>
        <owl:annotatedProperty rdf:resource="&rdfs;seeAlso"/>
    </owl:Axiom>
    


    <!-- http://biomodels.net/teddy/TEDDY#TEDDY_0000130 -->

    <owl:Class rdf:about="&teddy;TEDDY_0000130">
        <rdfs:label xml:lang="en">inflexion point</rdfs:label>
        <rdfs:subClassOf rdf:resource="&teddy;TEDDY_0000023"/>
        <rdfs:seeAlso rdf:datatype="&xsd;anyURI">http://mathworld.wolfram.com/InflectionPoint.html</rdfs:seeAlso>
        <skos:definition xml:lang="en">An inflection point is a point on a curve at which the sign of the curvature (i.e., the concavity) changes. Inflection points may be stationary points, but are not local maxima or local minima.</skos:definition>
    </owl:Class>
    <owl:Axiom>
        <owl:annotatedTarget rdf:datatype="&xsd;anyURI">http://mathworld.wolfram.com/InflectionPoint.html</owl:annotatedTarget>
        <rdfs:comment xml:lang="en">Weisstein, Eric W. Inflection Point. From MathWorld--A Wolfram Web Resource.</rdfs:comment>
        <owl:annotatedSource rdf:resource="&teddy;TEDDY_0000130"/>
        <owl:annotatedProperty rdf:resource="&rdfs;seeAlso"/>
    </owl:Axiom>
    


    <!-- http://biomodels.net/teddy/TEDDY#TEDDY_0000131 -->

    <owl:Class rdf:about="&teddy;TEDDY_0000131">
        <rdfs:label xml:lang="en">amplitude</rdfs:label>
        <rdfs:subClassOf rdf:resource="&teddy;TEDDY_0000116"/>
        <rdfs:seeAlso rdf:datatype="&xsd;anyURI">http://mathworld.wolfram.com/Amplitude.html</rdfs:seeAlso>
        <skos:definition xml:lang="en">A magnitude of an oscillation.</skos:definition>
    </owl:Class>
    <owl:Axiom>
        <owl:annotatedTarget rdf:datatype="&xsd;anyURI">http://mathworld.wolfram.com/Amplitude.html</owl:annotatedTarget>
        <rdfs:comment xml:lang="en">Weisstein, Eric W. &quot;Amplitude.&quot; From MathWorld--A Wolfram Web Resource.</rdfs:comment>
        <owl:annotatedSource rdf:resource="&teddy;TEDDY_0000131"/>
        <owl:annotatedProperty rdf:resource="&rdfs;seeAlso"/>
    </owl:Axiom>
    


    <!-- http://biomodels.net/teddy/TEDDY#TEDDY_0000132 -->

    <owl:Class rdf:about="&teddy;TEDDY_0000132">
        <rdfs:label xml:lang="en">behaviour diversification</rdfs:label>
        <rdfs:subClassOf rdf:resource="&teddy;TEDDY_0000000"/>
        <skos:definition xml:lang="en">Behaviour diversification describes the way one or several temporal behaviours [https://identifiers.org/biomodels.teddy/TEDDY_0000083] are modified or related upon interaction with information external to the system considered. </skos:definition>
    </owl:Class>
    


    <!-- http://biomodels.net/teddy/TEDDY#TEDDY_0000133 -->

    <owl:Class rdf:about="&teddy;TEDDY_0000133">
        <rdfs:label xml:lang="en">Lyapunov stability</rdfs:label>
        <rdfs:subClassOf rdf:resource="&teddy;TEDDY_0000148"/>
        <owl:disjointWith rdf:resource="&teddy;TEDDY_0000134"/>
        <rdfs:seeAlso rdf:datatype="&xsd;anyURI">https://identifiers.org/isbn/0198565623</rdfs:seeAlso>
        <skos:definition xml:lang="en">A solution x*(t) of the n-dimentional system x ̇=X(x, t) is Liapunov stable, if no matter how small is the permitted deviation, measured by epsilon, there still exists a nonzero tolerance, measured by delta, in the initial conditions when the system is activated, allowing it to run satisfactorily.</skos:definition>
        <skos:altLabel xml:lang="en">Liapunov stability</skos:altLabel>
        <skos:altLabel xml:lang="en">solution stability</skos:altLabel>
    </owl:Class>
    <owl:Axiom>
        <owl:annotatedTarget rdf:datatype="&xsd;anyURI">https://identifiers.org/isbn/0198565623</owl:annotatedTarget>
        <rdfs:comment xml:lang="en">Jordan DW., Smith P. (1999) Nonlinear ordinary differential equations: an introduction to dynamical systems, Oxford University Press. (p.286)</rdfs:comment>
        <owl:annotatedSource rdf:resource="&teddy;TEDDY_0000133"/>
        <owl:annotatedProperty rdf:resource="&rdfs;seeAlso"/>
    </owl:Axiom>
    <owl:Axiom>
        <rdfs:seeAlso rdf:datatype="&xsd;anyURI">https://identifiers.org/isbn/0198565623 (p.286)</rdfs:seeAlso>
        <owl:annotatedTarget xml:lang="en">solution stability</owl:annotatedTarget>
        <owl:annotatedSource rdf:resource="&teddy;TEDDY_0000133"/>
        <owl:annotatedProperty rdf:resource="&skos;altLabel"/>
    </owl:Axiom>
    


    <!-- http://biomodels.net/teddy/TEDDY#TEDDY_0000134 -->

    <owl:Class rdf:about="&teddy;TEDDY_0000134">
        <rdfs:label xml:lang="en">half-stability</rdfs:label>
        <rdfs:subClassOf rdf:resource="&teddy;TEDDY_0000148"/>
        <rdfs:subClassOf>
            <owl:Restriction>
                <owl:onProperty rdf:resource="&ro;has_part"/>
                <owl:someValuesFrom rdf:resource="&teddy;TEDDY_0000097"/>
            </owl:Restriction>
        </rdfs:subClassOf>
        <rdfs:subClassOf>
            <owl:Restriction>
                <owl:onProperty rdf:resource="&ro;has_part"/>
                <owl:someValuesFrom>
                    <owl:Class>
                        <owl:complementOf rdf:resource="&teddy;TEDDY_0000133"/>
                    </owl:Class>
                </owl:someValuesFrom>
            </owl:Restriction>
        </rdfs:subClassOf>
        <owl:disjointWith rdf:resource="&teddy;TEDDY_0000149"/>
        <rdfs:seeAlso rdf:datatype="&xsd;anyURI">https://identifiers.org/isbn/0738204536</rdfs:seeAlso>
        <skos:definition xml:lang="en">An invariant set is called half-stable if there exist a stable and an unstable manifold with respect to the invariant set.</skos:definition>
    </owl:Class>
    <owl:Axiom>
        <owl:annotatedTarget rdf:datatype="&xsd;anyURI">https://identifiers.org/isbn/0738204536</owl:annotatedTarget>
        <rdfs:comment xml:lang="en">Strogatz SH. (2000) Nonlinear dynamics and chaos: with applications to physics, biology, chemistry, and engineering, Westview Press, Cambridge, MA. (p.26,196)</rdfs:comment>
        <owl:annotatedSource rdf:resource="&teddy;TEDDY_0000134"/>
        <owl:annotatedProperty rdf:resource="&rdfs;seeAlso"/>
    </owl:Axiom>
    


    <!-- http://biomodels.net/teddy/TEDDY#TEDDY_0000135 -->

    <owl:Class rdf:about="&teddy;TEDDY_0000135">
        <rdfs:label xml:lang="en">only local stability</rdfs:label>
        <rdfs:subClassOf rdf:resource="&teddy;TEDDY_0000097"/>
        <rdfs:subClassOf>
            <owl:Class>
                <owl:complementOf rdf:resource="&teddy;TEDDY_0000136"/>
            </owl:Class>
        </rdfs:subClassOf>
        <owl:disjointWith rdf:resource="&teddy;TEDDY_0000136"/>
        <rdfs:seeAlso rdf:datatype="&xsd;anyURI">https://identifiers.org/isbn/0738204536</rdfs:seeAlso>
        <skos:definition xml:lang="en">An asymptotically stable [https://identifiers.org/biomodels.teddy/TEDDY_0000097] behaviour [https://identifiers.org/biomodels.teddy/TEDDY_0000083] to which only behaviours starting in a restricted neighbourhood will converge.</skos:definition>
    </owl:Class>
    <owl:Axiom>
        <owl:annotatedTarget rdf:datatype="&xsd;anyURI">https://identifiers.org/isbn/0738204536</owl:annotatedTarget>
        <rdfs:comment xml:lang="en">Strogatz SH. (2000) Nonlinear dynamics and chaos: with applications to physics, biology, chemistry, and engineering, Westview Press, Cambridge, MA. (p.20)</rdfs:comment>
        <owl:annotatedSource rdf:resource="&teddy;TEDDY_0000135"/>
        <owl:annotatedProperty rdf:resource="&rdfs;seeAlso"/>
    </owl:Axiom>
    


    <!-- http://biomodels.net/teddy/TEDDY#TEDDY_0000136 -->

    <owl:Class rdf:about="&teddy;TEDDY_0000136">
        <rdfs:label xml:lang="en">global stability</rdfs:label>
        <rdfs:subClassOf rdf:resource="&teddy;TEDDY_0000097"/>
        <rdfs:subClassOf>
            <owl:Class>
                <owl:complementOf rdf:resource="&teddy;TEDDY_0000135"/>
            </owl:Class>
        </rdfs:subClassOf>
        <rdfs:seeAlso rdf:datatype="&xsd;anyURI">https://identifiers.org/isbn/0738204536</rdfs:seeAlso>
        <skos:definition xml:lang="en">An asymptotically stable [https://identifiers.org/biomodels.teddy/TEDDY_0000097] behaviour [https://identifiers.org/biomodels.teddy/TEDDY_0000083] to which all other behaviours will converge independent of the initial distance.</skos:definition>
    </owl:Class>
    <owl:Axiom>
        <owl:annotatedTarget rdf:datatype="&xsd;anyURI">https://identifiers.org/isbn/0738204536</owl:annotatedTarget>
        <rdfs:comment xml:lang="en">Strogatz SH. (2000) Nonlinear dynamics and chaos: with applications to physics, biology, chemistry, and engineering, Westview Press, Cambridge, MA. (p.20)</rdfs:comment>
        <owl:annotatedSource rdf:resource="&teddy;TEDDY_0000136"/>
        <owl:annotatedProperty rdf:resource="&rdfs;seeAlso"/>
    </owl:Axiom>
    


    <!-- http://biomodels.net/teddy/TEDDY#TEDDY_0000137 -->

    <owl:Class rdf:about="&teddy;TEDDY_0000137">
        <rdfs:label xml:lang="en">stable node</rdfs:label>
        <rdfs:subClassOf rdf:resource="&teddy;TEDDY_0000087"/>
        <rdfs:subClassOf>
            <owl:Restriction>
                <owl:onProperty rdf:resource="&teddy;TR_0004"/>
                <owl:someValuesFrom rdf:resource="&teddy;TEDDY_0000097"/>
            </owl:Restriction>
        </rdfs:subClassOf>
        <rdfs:subClassOf>
            <owl:Restriction>
                <owl:onProperty rdf:resource="&teddy;TR_0004"/>
                <owl:someValuesFrom rdf:resource="&teddy;TEDDY_0000150"/>
            </owl:Restriction>
        </rdfs:subClassOf>
        <rdfs:subClassOf>
            <owl:Restriction>
                <owl:onProperty rdf:resource="&teddy;TR_0004"/>
                <owl:someValuesFrom rdf:resource="&teddy;TEDDY_0000149"/>
            </owl:Restriction>
        </rdfs:subClassOf>
        <rdfs:seeAlso rdf:datatype="&xsd;anyURI">https://identifiers.org/isbn/0738204536</rdfs:seeAlso>
        <skos:definition xml:lang="en">A fixed point node [https://identifiers.org/biomodels.teddy/TEDDY_0000087] which is stable [https://identifiers.org/biomodels.teddy/TEDDY_0000133], i.e. for which the Jacobian matrix has two negative eigenvalues.</skos:definition>
        <skos:altLabel xml:lang="en">nodal sink</skos:altLabel>
    </owl:Class>
    <owl:Axiom>
        <owl:annotatedTarget rdf:datatype="&xsd;anyURI">https://identifiers.org/isbn/0738204536</owl:annotatedTarget>
        <rdfs:comment xml:lang="en">Strogatz SH. (2000) Nonlinear dynamics and chaos: with applications to physics, biology, chemistry, and engineering, Westview Press, Cambridge, MA. (p.137)</rdfs:comment>
        <owl:annotatedSource rdf:resource="&teddy;TEDDY_0000137"/>
        <owl:annotatedProperty rdf:resource="&rdfs;seeAlso"/>
    </owl:Axiom>
    


    <!-- http://biomodels.net/teddy/TEDDY#TEDDY_0000138 -->

    <owl:Class rdf:about="&teddy;TEDDY_0000138">
        <rdfs:label xml:lang="en">unstable node</rdfs:label>
        <owl:equivalentClass>
            <owl:Restriction>
                <owl:onProperty rdf:resource="&teddy;TR_0015"/>
                <owl:someValuesFrom rdf:resource="&teddy;TEDDY_0000137"/>
            </owl:Restriction>
        </owl:equivalentClass>
        <rdfs:subClassOf rdf:resource="&teddy;TEDDY_0000087"/>
        <rdfs:subClassOf>
            <owl:Class>
                <owl:complementOf>
                    <owl:Restriction>
                        <owl:onProperty rdf:resource="&teddy;TR_0004"/>
                        <owl:someValuesFrom rdf:resource="&teddy;TEDDY_0000133"/>
                    </owl:Restriction>
                </owl:complementOf>
            </owl:Class>
        </rdfs:subClassOf>
        <rdfs:subClassOf>
            <owl:Class>
                <owl:complementOf>
                    <owl:Restriction>
                        <owl:onProperty rdf:resource="&teddy;TR_0004"/>
                        <owl:someValuesFrom rdf:resource="&teddy;TEDDY_0000149"/>
                    </owl:Restriction>
                </owl:complementOf>
            </owl:Class>
        </rdfs:subClassOf>
        <rdfs:seeAlso rdf:datatype="&xsd;anyURI">https://identifiers.org/isbn/0738204536</rdfs:seeAlso>
        <skos:definition xml:lang="en">A fixed point node [https://identifiers.org/biomodels.teddy/TEDDY_0000087] which is unstable [not TEDDY_0000133], i.e. for which the Jacobian matrix has two positive eigenvalues.</skos:definition>
        <skos:altLabel xml:lang="en">nodal source</skos:altLabel>
    </owl:Class>
    <owl:Axiom>
        <owl:annotatedTarget rdf:datatype="&xsd;anyURI">https://identifiers.org/isbn/0738204536</owl:annotatedTarget>
        <rdfs:comment xml:lang="en">Strogatz SH. (2000) Nonlinear dynamics and chaos: with applications to physics, biology, chemistry, and engineering, Westview Press, Cambridge, MA. (p.137)</rdfs:comment>
        <owl:annotatedSource rdf:resource="&teddy;TEDDY_0000138"/>
        <owl:annotatedProperty rdf:resource="&rdfs;seeAlso"/>
    </owl:Axiom>
    


    <!-- http://biomodels.net/teddy/TEDDY#TEDDY_0000139 -->

    <owl:Class rdf:about="&teddy;TEDDY_0000139">
        <rdfs:label xml:lang="en">stable star</rdfs:label>
        <rdfs:subClassOf rdf:resource="&teddy;TEDDY_0000090"/>
        <rdfs:subClassOf>
            <owl:Restriction>
                <owl:onProperty rdf:resource="&teddy;TR_0004"/>
                <owl:someValuesFrom rdf:resource="&teddy;TEDDY_0000097"/>
            </owl:Restriction>
        </rdfs:subClassOf>
        <rdfs:seeAlso rdf:datatype="&xsd;anyURI">https://identifiers.org/isbn/0738204536</rdfs:seeAlso>
        <skos:definition xml:lang="en">A star [https://identifiers.org/biomodels.teddy/TEDDY_0000090] which is stable [https://identifiers.org/biomodels.teddy/TEDDY_0000133], i.e. for which the Jacobian matrix has two identical negative eigenvalues. All other trajectories [https://identifiers.org/biomodels.teddy/TEDDY_0000083] of the system are straight lines towards the fixed point.</skos:definition>
        <skos:altLabel xml:lang="en">stable proper node</skos:altLabel>
    </owl:Class>
    <owl:Axiom>
        <owl:annotatedTarget rdf:datatype="&xsd;anyURI">https://identifiers.org/isbn/0738204536</owl:annotatedTarget>
        <rdfs:comment xml:lang="en">Strogatz SH. (2000) Nonlinear dynamics and chaos: with applications to physics, biology, chemistry, and engineering, Westview Press, Cambridge, MA. (p.137)</rdfs:comment>
        <owl:annotatedSource rdf:resource="&teddy;TEDDY_0000139"/>
        <owl:annotatedProperty rdf:resource="&rdfs;seeAlso"/>
    </owl:Axiom>
    


    <!-- http://biomodels.net/teddy/TEDDY#TEDDY_0000140 -->

    <owl:Class rdf:about="&teddy;TEDDY_0000140">
        <rdfs:label xml:lang="en">unstable star</rdfs:label>
        <owl:equivalentClass>
            <owl:Restriction>
                <owl:onProperty rdf:resource="&teddy;TR_0015"/>
                <owl:someValuesFrom rdf:resource="&teddy;TEDDY_0000139"/>
            </owl:Restriction>
        </owl:equivalentClass>
        <rdfs:subClassOf rdf:resource="&teddy;TEDDY_0000090"/>
        <rdfs:subClassOf>
            <owl:Class>
                <owl:complementOf>
                    <owl:Restriction>
                        <owl:onProperty rdf:resource="&teddy;TR_0004"/>
                        <owl:someValuesFrom rdf:resource="&teddy;TEDDY_0000133"/>
                    </owl:Restriction>
                </owl:complementOf>
            </owl:Class>
        </rdfs:subClassOf>
        <rdfs:seeAlso rdf:datatype="&xsd;anyURI">https://identifiers.org/isbn/0738204536</rdfs:seeAlso>
        <skos:definition xml:lang="en">A star [https://identifiers.org/biomodels.teddy/TEDDY_0000090] which is unstable [not TEDDY_0000133], i.e. for which the Jacobian matrix has two identical positive eigenvalues. All other trajectories [https://identifiers.org/biomodels.teddy/TEDDY_0000083] of the system are straight lines away the fixed point.</skos:definition>
        <skos:altLabel xml:lang="en">unstable proper node</skos:altLabel>
    </owl:Class>
    <owl:Axiom>
        <owl:annotatedTarget rdf:datatype="&xsd;anyURI">https://identifiers.org/isbn/0738204536</owl:annotatedTarget>
        <rdfs:comment xml:lang="en">Strogatz SH. (2000) Nonlinear dynamics and chaos: with applications to physics, biology, chemistry, and engineering, Westview Press, Cambridge, MA. (p.137)</rdfs:comment>
        <owl:annotatedSource rdf:resource="&teddy;TEDDY_0000140"/>
        <owl:annotatedProperty rdf:resource="&rdfs;seeAlso"/>
    </owl:Axiom>
    


    <!-- http://biomodels.net/teddy/TEDDY#TEDDY_0000141 -->

    <owl:Class rdf:about="&teddy;TEDDY_0000141">
        <rdfs:label xml:lang="en">stable degenerate node</rdfs:label>
        <rdfs:subClassOf rdf:resource="&teddy;TEDDY_0000093"/>
        <rdfs:subClassOf>
            <owl:Restriction>
                <owl:onProperty rdf:resource="&teddy;TR_0004"/>
                <owl:someValuesFrom rdf:resource="&teddy;TEDDY_0000149"/>
            </owl:Restriction>
        </rdfs:subClassOf>
        <rdfs:subClassOf>
            <owl:Restriction>
                <owl:onProperty rdf:resource="&teddy;TR_0004"/>
                <owl:someValuesFrom rdf:resource="&teddy;TEDDY_0000133"/>
            </owl:Restriction>
        </rdfs:subClassOf>
        <rdfs:seeAlso rdf:datatype="&xsd;anyURI">https://identifiers.org/isbn/0738204536</rdfs:seeAlso>
        <skos:definition xml:lang="en">A degenerated node [https://identifiers.org/biomodels.teddy/TEDDY_0000093] which is stable [https://identifiers.org/biomodels.teddy/TEDDY_0000133], i.e. for which the Jacobian matrix has two identical negative eigenvalues.</skos:definition>
        <skos:altLabel xml:lang="en">degenerate stable node</skos:altLabel>
        <skos:altLabel xml:lang="en">stable degenerated node</skos:altLabel>
        <skos:altLabel xml:lang="en">stable improper node</skos:altLabel>
    </owl:Class>
    <owl:Axiom>
        <rdfs:seeAlso rdf:datatype="&xsd;anyURI">https://identifiers.org/isbn/0198565623 (p.73)</rdfs:seeAlso>
        <owl:annotatedTarget xml:lang="en">degenerate stable node</owl:annotatedTarget>
        <owl:annotatedSource rdf:resource="&teddy;TEDDY_0000141"/>
        <owl:annotatedProperty rdf:resource="&skos;altLabel"/>
    </owl:Axiom>
    <owl:Axiom>
        <owl:annotatedTarget rdf:datatype="&xsd;anyURI">https://identifiers.org/isbn/0738204536</owl:annotatedTarget>
        <rdfs:comment xml:lang="en">Strogatz SH. (2000) Nonlinear dynamics and chaos: with applications to physics, biology, chemistry, and engineering, Westview Press, Cambridge, MA. (p.137)</rdfs:comment>
        <owl:annotatedSource rdf:resource="&teddy;TEDDY_0000141"/>
        <owl:annotatedProperty rdf:resource="&rdfs;seeAlso"/>
    </owl:Axiom>
    


    <!-- http://biomodels.net/teddy/TEDDY#TEDDY_0000142 -->

    <owl:Class rdf:about="&teddy;TEDDY_0000142">
        <rdfs:label xml:lang="en">unstable degenerate node</rdfs:label>
        <owl:equivalentClass>
            <owl:Restriction>
                <owl:onProperty rdf:resource="&teddy;TR_0015"/>
                <owl:someValuesFrom rdf:resource="&teddy;TEDDY_0000141"/>
            </owl:Restriction>
        </owl:equivalentClass>
        <rdfs:subClassOf rdf:resource="&teddy;TEDDY_0000093"/>
        <rdfs:subClassOf>
            <owl:Class>
                <owl:complementOf>
                    <owl:Restriction>
                        <owl:onProperty rdf:resource="&teddy;TR_0004"/>
                        <owl:someValuesFrom rdf:resource="&teddy;TEDDY_0000133"/>
                    </owl:Restriction>
                </owl:complementOf>
            </owl:Class>
        </rdfs:subClassOf>
        <rdfs:subClassOf>
            <owl:Class>
                <owl:complementOf>
                    <owl:Restriction>
                        <owl:onProperty rdf:resource="&teddy;TR_0004"/>
                        <owl:someValuesFrom rdf:resource="&teddy;TEDDY_0000149"/>
                    </owl:Restriction>
                </owl:complementOf>
            </owl:Class>
        </rdfs:subClassOf>
        <rdfs:seeAlso rdf:datatype="&xsd;anyURI">https://identifiers.org/isbn/0738204536</rdfs:seeAlso>
        <skos:definition xml:lang="en">A degenerated node [https://identifiers.org/biomodels.teddy/TEDDY_0000093] which is unstable [not TEDDY_0000133], i.e. for which the Jacobian matrix has two identical positive eigenvalues.</skos:definition>
        <skos:altLabel xml:lang="en">degenerate unstable point</skos:altLabel>
        <skos:altLabel xml:lang="en">unstable degenerated node</skos:altLabel>
        <skos:altLabel xml:lang="en">unstable improper node</skos:altLabel>
    </owl:Class>
    <owl:Axiom>
        <owl:annotatedTarget rdf:datatype="&xsd;anyURI">https://identifiers.org/isbn/0738204536</owl:annotatedTarget>
        <rdfs:comment xml:lang="en">Strogatz SH. (2000) Nonlinear dynamics and chaos: with applications to physics, biology, chemistry, and engineering, Westview Press, Cambridge, MA. (p.137)</rdfs:comment>
        <owl:annotatedSource rdf:resource="&teddy;TEDDY_0000142"/>
        <owl:annotatedProperty rdf:resource="&rdfs;seeAlso"/>
    </owl:Axiom>
    <owl:Axiom>
        <rdfs:seeAlso rdf:datatype="&xsd;anyURI">https://identifiers.org/isbn/0198565623 (p.73)</rdfs:seeAlso>
        <owl:annotatedTarget xml:lang="en">degenerate unstable point</owl:annotatedTarget>
        <owl:annotatedSource rdf:resource="&teddy;TEDDY_0000142"/>
        <owl:annotatedProperty rdf:resource="&skos;altLabel"/>
    </owl:Axiom>
    


    <!-- http://biomodels.net/teddy/TEDDY#TEDDY_0000143 -->

    <owl:Class rdf:about="&teddy;TEDDY_0000143">
        <rdfs:label xml:lang="en">non-periodic orbit</rdfs:label>
        <rdfs:subClassOf rdf:resource="&teddy;TEDDY_0000083"/>
        <rdfs:seeAlso rdf:datatype="&xsd;anyURI">https://identifiers.org/isbn/9781402014031</rdfs:seeAlso>
        <skos:definition xml:lang="en">A &apos;temporal behaviour&apos; [https://identifiers.org/biomodels.teddy/TEDDY_0000083] which never repeats its state.</skos:definition>
    </owl:Class>
    <owl:Axiom>
        <owl:annotatedTarget rdf:datatype="&xsd;anyURI">https://identifiers.org/isbn/9781402014031</owl:annotatedTarget>
        <rdfs:comment xml:lang="en">Coley AA. (2003) Dynamical systems and cosmology, Kluwer Academic Publishers, Dordrecht. (p.10)</rdfs:comment>
        <owl:annotatedSource rdf:resource="&teddy;TEDDY_0000143"/>
        <owl:annotatedProperty rdf:resource="&rdfs;seeAlso"/>
    </owl:Axiom>
    


    <!-- http://biomodels.net/teddy/TEDDY#TEDDY_0000144 -->

    <owl:Class rdf:about="&teddy;TEDDY_0000144">
        <rdfs:label xml:lang="en">monotonicity characteristic</rdfs:label>
        <rdfs:subClassOf rdf:resource="&teddy;TEDDY_0000023"/>
        <skos:definition xml:lang="en">A characteristic describing the order of the successive states of a curve.</skos:definition>
    </owl:Class>
    


    <!-- http://biomodels.net/teddy/TEDDY#TEDDY_0000145 -->

    <owl:Class rdf:about="&teddy;TEDDY_0000145">
        <rdfs:label xml:lang="en">half-stable limit cycle</rdfs:label>
        <rdfs:subClassOf rdf:resource="&teddy;TEDDY_0000051"/>
        <rdfs:subClassOf>
            <owl:Restriction>
                <owl:onProperty rdf:resource="&teddy;TR_0004"/>
                <owl:someValuesFrom rdf:resource="&teddy;TEDDY_0000134"/>
            </owl:Restriction>
        </rdfs:subClassOf>
        <rdfs:seeAlso rdf:datatype="&xsd;anyURI">https://identifiers.org/isbn/0738204536</rdfs:seeAlso>
        <skos:definition xml:lang="en">If trajectories [https://identifiers.org/biomodels.teddy/TEDDY_0000083] on one side of the limit cycle [https://identifiers.org/biomodels.teddy/TEDDY_0000051] spiral inward and on the other side spiral outward, it is called semistable.</skos:definition>
        <skos:altLabel xml:lang="en">semi-stable limit cycle</skos:altLabel>
        <skos:altLabel xml:lang="en">semistable limit cycle</skos:altLabel>
    </owl:Class>
    <owl:Axiom>
        <owl:annotatedTarget rdf:datatype="&xsd;anyURI">https://identifiers.org/isbn/0738204536</owl:annotatedTarget>
        <rdfs:comment xml:lang="en">Strogatz SH. (2000) Nonlinear dynamics and chaos: with applications to physics, biology, chemistry, and engineering, Westview Press, Cambridge, MA. (p.196)</rdfs:comment>
        <owl:annotatedSource rdf:resource="&teddy;TEDDY_0000145"/>
        <owl:annotatedProperty rdf:resource="&rdfs;seeAlso"/>
    </owl:Axiom>
    <owl:Axiom>
        <rdfs:comment rdf:datatype="&xsd;anyURI">https://identifiers.org/isbn/0198565623 (p.114)</rdfs:comment>
        <owl:annotatedTarget xml:lang="en">semi-stable limit cycle</owl:annotatedTarget>
        <owl:annotatedSource rdf:resource="&teddy;TEDDY_0000145"/>
        <owl:annotatedProperty rdf:resource="&skos;altLabel"/>
    </owl:Axiom>
    


    <!-- http://biomodels.net/teddy/TEDDY#TEDDY_0000146 -->

    <owl:Class rdf:about="&teddy;TEDDY_0000146">
        <rdfs:label xml:lang="en">asymptotic behaviour</rdfs:label>
        <rdfs:subClassOf>
            <owl:Class>
                <owl:intersectionOf rdf:parseType="Collection">
                    <rdf:Description rdf:about="&teddy;TEDDY_0000143"/>
                    <owl:Restriction>
                        <owl:onProperty rdf:resource="&teddy;TR_0013"/>
                        <owl:someValuesFrom rdf:resource="&teddy;TEDDY_0000085"/>
                    </owl:Restriction>
                </owl:intersectionOf>
            </owl:Class>
        </rdfs:subClassOf>
        <skos:definition xml:lang="en">A `temporal behaviour` [https://identifiers.org/biomodels.teddy/TEDDY_0000083] which converges to some `limit behaviour` [https://identifiers.org/biomodels.teddy/TEDDY_0000085].</skos:definition>
    </owl:Class>
    


    <!-- http://biomodels.net/teddy/TEDDY#TEDDY_0000147 -->

    <owl:Class rdf:about="&teddy;TEDDY_0000147">
        <rdfs:label xml:lang="en">global bifurcation</rdfs:label>
        <rdfs:subClassOf rdf:resource="&teddy;TEDDY_0000053"/>
        <rdfs:seeAlso rdf:datatype="&xsd;anyURI">https://identifiers.org/isbn/0387983821</rdfs:seeAlso>
        <skos:definition xml:lang="en">A bifurcation [https://identifiers.org/biomodels.teddy/TEDDY_0000053] in which at least two limit cycles [https://identifiers.org/biomodels.teddy/TEDDY_0000051] or fixed points TEDDY_0000086 are involved. It can not be detected within a small neighborhood of a fixed point.</skos:definition>
    </owl:Class>
    <owl:Axiom>
        <owl:annotatedTarget rdf:datatype="&xsd;anyURI">https://identifiers.org/isbn/0387983821</owl:annotatedTarget>
        <rdfs:comment xml:lang="en">Kuznetsov YA. (1988) Elements of applied bifurcation theory, Springer, New York. (p.59)</rdfs:comment>
        <owl:annotatedSource rdf:resource="&teddy;TEDDY_0000147"/>
        <owl:annotatedProperty rdf:resource="&rdfs;seeAlso"/>
    </owl:Axiom>
    


    <!-- http://biomodels.net/teddy/TEDDY#TEDDY_0000148 -->

    <owl:Class rdf:about="&teddy;TEDDY_0000148">
        <rdfs:label xml:lang="en">stability characteristic</rdfs:label>
        <rdfs:subClassOf rdf:resource="&teddy;TEDDY_0000002"/>
        <skos:definition xml:lang="en">A characteristic describing stability of a &apos;temporal behaviour&apos; [https://identifiers.org/biomodels.teddy/TEDDY_0000083], i.e. how far from each other solutions with close initial states become as time passes.</skos:definition>
    </owl:Class>
    


    <!-- http://biomodels.net/teddy/TEDDY#TEDDY_0000149 -->

    <owl:Class rdf:about="&teddy;TEDDY_0000149">
        <rdfs:label xml:lang="en">Poincaré stability</rdfs:label>
        <rdfs:subClassOf rdf:resource="&teddy;TEDDY_0000148"/>
        <rdfs:seeAlso rdf:datatype="&xsd;anyURI">https://identifiers.org/isbn/0198565623</rdfs:seeAlso>
        <skos:altLabel xml:lang="en">Poisson stability</skos:altLabel>
        <skos:definition xml:lang="en">The solution x*(t), t &gt;= t0 is Poincaré stable, if all sufficiently small disturbances of the initial value a* lead to half-paths remaining for all later time at a small distance from the half-path H* with initial point a*.</skos:definition>
        <skos:altLabel xml:lang="en">orbitally stable behaviour</skos:altLabel>
    </owl:Class>
    <owl:Axiom>
        <rdfs:seeAlso rdf:datatype="&xsd;anyURI">https://identifiers.org/isbn/0198565623 (p.278)</rdfs:seeAlso>
        <owl:annotatedTarget xml:lang="en">orbitally stable behaviour</owl:annotatedTarget>
        <owl:annotatedSource rdf:resource="&teddy;TEDDY_0000149"/>
        <owl:annotatedProperty rdf:resource="&skos;altLabel"/>
    </owl:Axiom>
    <owl:Axiom>
        <owl:annotatedTarget rdf:datatype="&xsd;anyURI">https://identifiers.org/isbn/0198565623</owl:annotatedTarget>
        <rdfs:comment xml:lang="en">Jordan DW., Smith P. (1999) Nonlinear ordinary differential equations: an introduction to dynamical systems, Oxford University Press. (p.278)</rdfs:comment>
        <owl:annotatedSource rdf:resource="&teddy;TEDDY_0000149"/>
        <owl:annotatedProperty rdf:resource="&rdfs;seeAlso"/>
    </owl:Axiom>
    <owl:Axiom>
        <rdfs:seeAlso rdf:datatype="&xsd;anyURI">https://identifiers.org/isbn/0821803670</rdfs:seeAlso>
        <owl:annotatedTarget xml:lang="en">Poisson stability</owl:annotatedTarget>
        <owl:annotatedSource rdf:resource="&teddy;TEDDY_0000149"/>
        <owl:annotatedProperty rdf:resource="&skos;altLabel"/>
    </owl:Axiom>
    


    <!-- http://biomodels.net/teddy/TEDDY#TEDDY_0000150 -->

    <owl:Class rdf:about="&teddy;TEDDY_0000150">
        <rdfs:label xml:lang="en">uniform stability</rdfs:label>
        <rdfs:subClassOf rdf:resource="&teddy;TEDDY_0000133"/>
        <rdfs:seeAlso rdf:datatype="&xsd;anyURI">https://identifiers.org/isbn/0198565623</rdfs:seeAlso>
        <skos:definition xml:lang="en">A Liapunov stable [https://identifiers.org/biomodels.teddy/TEDDY_0000133] solution [https://identifiers.org/biomodels.teddy/TEDDY_0000083] is uniformly stable if its sensitivity to disturbance does not increase indefinitely with time.</skos:definition>
    </owl:Class>
    <owl:Axiom>
        <owl:annotatedTarget rdf:datatype="&xsd;anyURI">https://identifiers.org/isbn/0198565623</owl:annotatedTarget>
        <rdfs:comment xml:lang="en">Jordan DW., Smith P. (1999) Nonlinear ordinary differential equations: an introduction to dynamical systems, Oxford University Press. (p.288)</rdfs:comment>
        <owl:annotatedSource rdf:resource="&teddy;TEDDY_0000150"/>
        <owl:annotatedProperty rdf:resource="&rdfs;seeAlso"/>
    </owl:Axiom>
    


    <!-- http://biomodels.net/teddy/TEDDY#TEDDY_0000151 -->

    <owl:Class rdf:about="&teddy;TEDDY_0000151">
        <rdfs:label xml:lang="en">heteroclinic orbit</rdfs:label>
        <owl:equivalentClass>
            <owl:Class>
                <owl:intersectionOf rdf:parseType="Collection">
                    <rdf:Description rdf:about="&teddy;TEDDY_0000143"/>
                    <owl:Restriction>
                        <owl:onProperty rdf:resource="&teddy;TR_0013"/>
                        <owl:onClass>
                            <owl:Class>
                                <owl:unionOf rdf:parseType="Collection">
                                    <rdf:Description rdf:about="&teddy;TEDDY_0000050"/>
                                    <rdf:Description rdf:about="&teddy;TEDDY_0000086"/>
                                </owl:unionOf>
                            </owl:Class>
                        </owl:onClass>
                        <owl:qualifiedCardinality rdf:datatype="&xsd;nonNegativeInteger">2</owl:qualifiedCardinality>
                    </owl:Restriction>
                </owl:intersectionOf>
            </owl:Class>
        </owl:equivalentClass>
        <owl:disjointWith rdf:resource="&teddy;TEDDY_0000152"/>
        <rdfs:seeAlso rdf:datatype="&xsd;anyURI">https://identifiers.org/isbn/0198565623</rdfs:seeAlso>
        <skos:definition xml:lang="en">A heteroclinic orbit is a trajectory [https://identifiers.org/biomodels.teddy/TEDDY_0000083] of a dynamical system that tends to two different invariant sets as time approaches positive and negative infinities.</skos:definition>
        <skos:altLabel xml:lang="en">heteroclinic path</skos:altLabel>
    </owl:Class>
    <owl:Axiom>
        <owl:annotatedTarget rdf:datatype="&xsd;anyURI">https://identifiers.org/isbn/0198565623</owl:annotatedTarget>
        <rdfs:comment xml:lang="en">Jordan DW., Smith P. (1999) Nonlinear ordinary differential equations: an introduction to dynamical systems, Oxford University Press. (pp.114-115)</rdfs:comment>
        <owl:annotatedSource rdf:resource="&teddy;TEDDY_0000151"/>
        <owl:annotatedProperty rdf:resource="&rdfs;seeAlso"/>
    </owl:Axiom>
    <owl:Axiom>
        <rdfs:seeAlso rdf:datatype="&xsd;anyURI">https://identifiers.org/isbn/0198565623 (pp.114-115)</rdfs:seeAlso>
        <owl:annotatedTarget xml:lang="en">heteroclinic path</owl:annotatedTarget>
        <owl:annotatedSource rdf:resource="&teddy;TEDDY_0000151"/>
        <owl:annotatedProperty rdf:resource="&skos;altLabel"/>
    </owl:Axiom>
    


    <!-- http://biomodels.net/teddy/TEDDY#TEDDY_0000152 -->

    <owl:Class rdf:about="&teddy;TEDDY_0000152">
        <rdfs:label xml:lang="en">homoclinic orbit</rdfs:label>
        <owl:equivalentClass>
            <owl:Class>
                <owl:intersectionOf rdf:parseType="Collection">
                    <rdf:Description rdf:about="&teddy;TEDDY_0000143"/>
                    <owl:Restriction>
                        <owl:onProperty rdf:resource="&teddy;TR_0013"/>
                        <owl:onClass>
                            <owl:Class>
                                <owl:unionOf rdf:parseType="Collection">
                                    <rdf:Description rdf:about="&teddy;TEDDY_0000050"/>
                                    <rdf:Description rdf:about="&teddy;TEDDY_0000086"/>
                                </owl:unionOf>
                            </owl:Class>
                        </owl:onClass>
                        <owl:qualifiedCardinality rdf:datatype="&xsd;nonNegativeInteger">1</owl:qualifiedCardinality>
                    </owl:Restriction>
                </owl:intersectionOf>
            </owl:Class>
        </owl:equivalentClass>
        <rdfs:seeAlso rdf:datatype="&xsd;anyURI">https://identifiers.org/isbn/0198565623</rdfs:seeAlso>
        <skos:definition xml:lang="en">A homoclinic orbit is a trajectory [https://identifiers.org/biomodels.teddy/TEDDY_0000083] of a dynamical system that tends to the same invariant set as time approaches positive and negative infinities.</skos:definition>
        <skos:altLabel xml:lang="en">homoclinic path</skos:altLabel>
    </owl:Class>
    <owl:Axiom>
        <rdfs:seeAlso rdf:datatype="&xsd;anyURI">https://identifiers.org/isbn/0198565623 (pp.114-115)</rdfs:seeAlso>
        <owl:annotatedTarget xml:lang="en">homoclinic path</owl:annotatedTarget>
        <owl:annotatedSource rdf:resource="&teddy;TEDDY_0000152"/>
        <owl:annotatedProperty rdf:resource="&skos;altLabel"/>
    </owl:Axiom>
    <owl:Axiom>
        <owl:annotatedTarget rdf:datatype="&xsd;anyURI">https://identifiers.org/isbn/0198565623</owl:annotatedTarget>
        <rdfs:comment xml:lang="en">Jordan DW., Smith P. (1999) Nonlinear ordinary differential equations: an introduction to dynamical systems, Oxford University Press. (pp.114-115)</rdfs:comment>
        <owl:annotatedSource rdf:resource="&teddy;TEDDY_0000152"/>
        <owl:annotatedProperty rdf:resource="&rdfs;seeAlso"/>
    </owl:Axiom>
    


    <!-- http://biomodels.net/teddy/TEDDY#TEDDY_0000153 -->

    <owl:Class rdf:about="&teddy;TEDDY_0000153">
        <rdfs:label xml:lang="en">heteroclinic bifurcation</rdfs:label>
        <rdfs:subClassOf rdf:resource="&teddy;TEDDY_0000147"/>
        <rdfs:seeAlso rdf:datatype="&xsd;anyURI">https://identifiers.org/isbn/0387983821</rdfs:seeAlso>
        <skos:definition xml:lang="en">A global bifurcation [https://identifiers.org/biomodels.teddy/TEDDY_0000147] in which two saddles [https://identifiers.org/biomodels.teddy/TEDDY_0000089] are only connected at the bifurcation point by a heteroclinic saddle connection [https://identifiers.org/biomodels.teddy/TEDDY_0000101]. This saddle connection does not exist below and above the bifurcation.</skos:definition>
    </owl:Class>
    <owl:Axiom>
        <owl:annotatedTarget rdf:datatype="&xsd;anyURI">https://identifiers.org/isbn/0387983821</owl:annotatedTarget>
        <rdfs:comment xml:lang="en">Kuznetsov YA. (1988) Elements of applied bifurcation theory, Springer, New York. (p.59)</rdfs:comment>
        <owl:annotatedSource rdf:resource="&teddy;TEDDY_0000153"/>
        <owl:annotatedProperty rdf:resource="&rdfs;seeAlso"/>
    </owl:Axiom>
    


    <!-- http://biomodels.net/teddy/TEDDY#TEDDY_0000154 -->

    <owl:Class rdf:about="&teddy;TEDDY_0000154">
        <rdfs:label xml:lang="en">homoclinic bifurcation</rdfs:label>
        <rdfs:subClassOf rdf:resource="&teddy;TEDDY_0000147"/>
        <rdfs:seeAlso rdf:datatype="&xsd;anyURI">https://identifiers.org/isbn/0387983821</rdfs:seeAlso>
        <skos:definition xml:lang="en">A global bifurcation [https://identifiers.org/biomodels.teddy/TEDDY_0000147] in which a homoclinic saddle connection [https://identifiers.org/biomodels.teddy/TEDDY_0000100] only exists at the bifurcation point. There exists a Limit Cycle [https://identifiers.org/biomodels.teddy/TEDDY_0000051] either below or above the bifurcation.</skos:definition>
        <skos:altLabel xml:lang="en">saddle-loop bifurcation</skos:altLabel>
    </owl:Class>
    <owl:Axiom>
        <rdfs:comment rdf:datatype="&xsd;anyURI">Kuznetsov YA. (1988) Elements of applied bifurcation theory, Springer, New York. (p.200ff)</rdfs:comment>
        <owl:annotatedTarget rdf:datatype="&xsd;anyURI">https://identifiers.org/isbn/0387983821</owl:annotatedTarget>
        <owl:annotatedSource rdf:resource="&teddy;TEDDY_0000154"/>
        <owl:annotatedProperty rdf:resource="&rdfs;seeAlso"/>
    </owl:Axiom>
    <owl:Axiom>
        <rdfs:seeAlso rdf:datatype="&xsd;anyURI">https://identifiers.org/isbn/0738204536 (p.263)</rdfs:seeAlso>
        <owl:annotatedTarget xml:lang="en">saddle-loop bifurcation</owl:annotatedTarget>
        <owl:annotatedSource rdf:resource="&teddy;TEDDY_0000154"/>
        <owl:annotatedProperty rdf:resource="&skos;altLabel"/>
    </owl:Axiom>
    


    <!-- http://biomodels.net/teddy/TEDDY#TEDDY_0000157 -->

    <owl:Class rdf:about="&teddy;TEDDY_0000157">
        <rdfs:label xml:lang="en">hyperbolicity</rdfs:label>
        <rdfs:subClassOf rdf:resource="&teddy;TEDDY_0000148"/>
        <rdfs:seeAlso rdf:datatype="&xsd;anyURI">https://identifiers.org/isbn/0198565623</rdfs:seeAlso>
        <rdfs:seeAlso rdf:datatype="&xsd;anyURI">https://identifiers.org/isbn/0387983821</rdfs:seeAlso>
        <skos:definition xml:lang="en">A fixed point [https://identifiers.org/biomodels.teddy/TEDDY_0000086] is said to be hyperbolic if all eigenvalues of the Jacobian matrix have non-zero real parts. A limit cycle [https://identifiers.org/biomodels.teddy/TEDDY_0000051] is called hyperbolic if the fixed point of the Poincare ́map is hyperbolic.</skos:definition>
    </owl:Class>
    <owl:Axiom>
        <owl:annotatedTarget rdf:datatype="&xsd;anyURI">https://identifiers.org/isbn/0198565623</owl:annotatedTarget>
        <rdfs:comment xml:lang="en">Jordan DW., Smith P. (1999) Nonlinear ordinary differential equations: an introduction to dynamical systems, Oxford University Press. (p.74)</rdfs:comment>
        <owl:annotatedSource rdf:resource="&teddy;TEDDY_0000157"/>
        <owl:annotatedProperty rdf:resource="&rdfs;seeAlso"/>
    </owl:Axiom>
    <owl:Axiom>
        <owl:annotatedTarget rdf:datatype="&xsd;anyURI">https://identifiers.org/isbn/0387983821</owl:annotatedTarget>
        <rdfs:comment xml:lang="en">Kuznetsov YA. (1988) Elements of applied bifurcation theory, Springer, New York. (p.55)</rdfs:comment>
        <owl:annotatedSource rdf:resource="&teddy;TEDDY_0000157"/>
        <owl:annotatedProperty rdf:resource="&rdfs;seeAlso"/>
    </owl:Axiom>
    


    <!-- http://biomodels.net/teddy/TEDDY#TEDDY_0000162 -->

    <owl:Class rdf:about="&teddy;TEDDY_0000162">
        <rdfs:label xml:lang="en">two-node positive feedback loop</rdfs:label>
        <rdfs:subClassOf rdf:resource="&teddy;TEDDY_0000035"/>
        <rdfs:seeAlso rdf:datatype="&xsd;anyURI">https://identifiers.org/isbn/1584886420</rdfs:seeAlso>
        <skos:altLabel xml:lang="en">2-node positive feedback</skos:altLabel>
        <skos:altLabel xml:lang="en">2-node positive feedback loop</skos:altLabel>
        <skos:definition xml:lang="en">A network motif in which two transcription factors regulate each other with the regulation signs of the two interactions leading to a positive feedback loop.</skos:definition>
        <skos:altLabel xml:lang="en">two-node positive feedback</skos:altLabel>
    </owl:Class>
    <owl:Axiom>
        <owl:annotatedTarget rdf:datatype="&xsd;anyURI">https://identifiers.org/isbn/1584886420</owl:annotatedTarget>
        <rdfs:comment xml:lang="en">Alon U (2006) An Introduction to Systems Biology: Design Principles of Biological Circuits, Chapman and Hall/CRC. (p.99)</rdfs:comment>
        <owl:annotatedSource rdf:resource="&teddy;TEDDY_0000162"/>
        <owl:annotatedProperty rdf:resource="&rdfs;seeAlso"/>
    </owl:Axiom>
    


    <!-- http://biomodels.net/teddy/TEDDY#TEDDY_0000163 -->

    <owl:Class rdf:about="&teddy;TEDDY_0000163">
        <rdfs:label xml:lang="en">double-positive feedback loop</rdfs:label>
        <rdfs:subClassOf rdf:resource="&teddy;TEDDY_0000162"/>
        <owl:disjointWith rdf:resource="&teddy;TEDDY_0000164"/>
        <rdfs:seeAlso rdf:datatype="&xsd;anyURI">https://identifiers.org/isbn/1584886420</rdfs:seeAlso>
        <skos:definition xml:lang="en">A positive feedback loop made of two positive interactions, so that the two transcription factors activate each other.</skos:definition>
        <skos:altLabel xml:lang="en">double-positive feedback</skos:altLabel>
    </owl:Class>
    <owl:Axiom>
        <owl:annotatedTarget rdf:datatype="&xsd;anyURI">https://identifiers.org/isbn/1584886420</owl:annotatedTarget>
        <rdfs:comment xml:lang="en">Alon U (2006) An Introduction to Systems Biology: Design Principles of Biological Circuits, Chapman and Hall/CRC. (p.99)</rdfs:comment>
        <owl:annotatedSource rdf:resource="&teddy;TEDDY_0000163"/>
        <owl:annotatedProperty rdf:resource="&rdfs;seeAlso"/>
    </owl:Axiom>
    


    <!-- http://biomodels.net/teddy/TEDDY#TEDDY_0000164 -->

    <owl:Class rdf:about="&teddy;TEDDY_0000164">
        <rdfs:label xml:lang="en">double-negative feedback loop</rdfs:label>
        <rdfs:subClassOf rdf:resource="&teddy;TEDDY_0000162"/>
        <rdfs:seeAlso rdf:datatype="&xsd;anyURI">https://identifiers.org/isbn/1584886420</rdfs:seeAlso>
        <skos:definition xml:lang="en">A positive feedback loop made of two negative interactions, so that the two transcription factors repress each other.</skos:definition>
        <skos:altLabel xml:lang="en">double-negative feedback</skos:altLabel>
    </owl:Class>
    <owl:Axiom>
        <owl:annotatedTarget rdf:datatype="&xsd;anyURI">https://identifiers.org/isbn/1584886420</owl:annotatedTarget>
        <rdfs:comment xml:lang="en">Alon U (2006) An Introduction to Systems Biology: Design Principles of Biological Circuits, Chapman and Hall/CRC. (p.99)</rdfs:comment>
        <owl:annotatedSource rdf:resource="&teddy;TEDDY_0000164"/>
        <owl:annotatedProperty rdf:resource="&rdfs;seeAlso"/>
    </owl:Axiom>
    


    <!-- http://biomodels.net/teddy/TEDDY#TEDDY_0000165 -->

    <owl:Class rdf:about="&teddy;TEDDY_0000165">
        <rdfs:label xml:lang="en">multi-output feed-forward loop</rdfs:label>
        <rdfs:subClassOf rdf:resource="&teddy;TEDDY_0000036"/>
        <rdfs:seeAlso rdf:datatype="&xsd;anyURI">https://identifiers.org/isbn/1584886420</rdfs:seeAlso>
        <skos:definition xml:lang="en">A simple topological generalization of the &apos;three-node feed-forward loop&apos; [https://identifiers.org/biomodels.teddy/TEDDY_0000037] based on multiplication of the output node.</skos:definition>
        <skos:altLabel xml:lang="en">multi-output FFL</skos:altLabel>
    </owl:Class>
    <owl:Axiom>
        <owl:annotatedTarget rdf:datatype="&xsd;anyURI">https://identifiers.org/isbn/1584886420</owl:annotatedTarget>
        <rdfs:comment xml:lang="en">Alon U (2006) An Introduction to Systems Biology: Design Principles of Biological Circuits, Chapman and Hall/CRC. (p.83)</rdfs:comment>
        <owl:annotatedSource rdf:resource="&teddy;TEDDY_0000165"/>
        <owl:annotatedProperty rdf:resource="&rdfs;seeAlso"/>
    </owl:Axiom>
    


    <!-- http://biomodels.net/teddy/TEDDY#TEDDY_0000166 -->

    <owl:Class rdf:about="&teddy;TEDDY_0000166">
        <rdfs:label xml:lang="en">toggle switch</rdfs:label>
        <rdfs:subClassOf rdf:resource="&teddy;TEDDY_0000056"/>
        <rdfs:seeAlso rdf:datatype="&xsd;anyURI">https://identifiers.org/pubmed/10659857</rdfs:seeAlso>
        <skos:definition xml:lang="en">A two-node double-negative loop.</skos:definition>
    </owl:Class>
    <owl:Axiom>
        <owl:annotatedTarget rdf:datatype="&xsd;anyURI">https://identifiers.org/pubmed/10659857</owl:annotatedTarget>
        <rdfs:comment xml:lang="en">Gardner TS, Cantor CR, Collins JJ (2000) Construction of a genetic toggle switch in Escherichia coli, Nature; 403(6767):339-42.</rdfs:comment>
        <owl:annotatedSource rdf:resource="&teddy;TEDDY_0000166"/>
        <owl:annotatedProperty rdf:resource="&rdfs;seeAlso"/>
    </owl:Axiom>
    


    <!-- http://biomodels.net/teddy/TEDDY#TEDDY_0000167 -->

    <owl:Class rdf:about="&teddy;TEDDY_0000167">
        <rdfs:label xml:lang="en">structural stability</rdfs:label>
        <rdfs:subClassOf rdf:resource="&teddy;TEDDY_0000148"/>
        <rdfs:seeAlso rdf:datatype="&xsd;anyURI">https://identifiers.org/isbn/0387983821</rdfs:seeAlso>
        <skos:definition xml:lang="en">A system x ̇=f(x), x ∈ Rn (1), defined in a region D ⊂ Rn is called structurally stable in a region D0 ⊂ D if for any sufficiently C1-close in D system x ̇=g(x), x ∈ Rn (2), there are regions U, V ⊂ D, D0 ⊂ U such that (1) is topologically equivalent in U to (2) in V.</skos:definition>
        <skos:altLabel xml:lang="en">Andronov&apos;s structural stability</skos:altLabel>
    </owl:Class>
    <owl:Axiom>
        <owl:annotatedTarget rdf:datatype="&xsd;anyURI">https://identifiers.org/isbn/0387983821</owl:annotatedTarget>
        <rdfs:comment xml:lang="en">Kuznetsov YA. (1988) Elements of applied bifurcation theory, Springer, New York. (p.71)</rdfs:comment>
        <owl:annotatedSource rdf:resource="&teddy;TEDDY_0000167"/>
        <owl:annotatedProperty rdf:resource="&rdfs;seeAlso"/>
    </owl:Axiom>
    


    <!-- http://biomodels.net/teddy/TEDDY#TEDDY_0000175 -->

    <owl:Class rdf:about="&teddy;TEDDY_0000175">
        <rdfs:label xml:lang="en">regular attractor</rdfs:label>
        <rdfs:subClassOf rdf:resource="&teddy;TEDDY_0000094"/>
        <rdfs:subClassOf>
            <owl:Restriction>
                <owl:onProperty rdf:resource="&teddy;TR_0004"/>
                <owl:someValuesFrom rdf:resource="&teddy;TEDDY_0000097"/>
            </owl:Restriction>
        </rdfs:subClassOf>
        <rdfs:seeAlso rdf:datatype="&xsd;anyURI">https://identifiers.org/isbn/9810221428</rdfs:seeAlso>
        <skos:definition xml:lang="en">The attractor [https://identifiers.org/biomodels.teddy/TEDDY_0000094] is regular or simple if the phase trajectories [https://identifiers.org/biomodels.teddy/TEDDY_0000083] on the attractor are stable according both to Lyapunov [https://identifiers.org/biomodels.teddy/TEDDY_0000113] and to Poisson [https://identifiers.org/biomodels.teddy/TEDDY_0000149].</skos:definition>
        <skos:altLabel xml:lang="en">simple attractor</skos:altLabel>
    </owl:Class>
    <owl:Axiom>
        <owl:annotatedTarget rdf:datatype="&xsd;anyURI">https://identifiers.org/isbn/9810221428</owl:annotatedTarget>
        <rdfs:comment xml:lang="en">V. S. Anishchenko (1995) Dynamical Chaos-Models and Experiments: Appearance Routes and Structure of Chaos in Simple Dynamical Systems (World Scientific Series on Nonlinear Science, Series a, Vol 8). World Scientific Pub Co Inc. (p.10)</rdfs:comment>
        <owl:annotatedSource rdf:resource="&teddy;TEDDY_0000175"/>
        <owl:annotatedProperty rdf:resource="&rdfs;seeAlso"/>
    </owl:Axiom>
    


    <!-- http://biomodels.net/teddy/TEDDY#TEDDY_0000177 -->

    <owl:Class rdf:about="&teddy;TEDDY_0000177">
        <rdfs:label xml:lang="en">blue sky catastrophe</rdfs:label>
        <rdfs:subClassOf rdf:resource="&teddy;TEDDY_0000070"/>
        <skos:definition xml:lang="en">A &apos;bifurcation of limit cycle&apos; [https://identifiers.org/biomodels.teddy/TEDDY_0000070] in which a limit cycle collides with a non-hyperbolic cycle.</skos:definition>
    </owl:Class>
    


    <!-- http://biomodels.net/teddy/TEDDY#TEDDY_0000178 -->

    <owl:Class rdf:about="&teddy;TEDDY_0000178">
        <rdfs:label xml:lang="en">curve quantitative characteristic</rdfs:label>
        <rdfs:subClassOf rdf:resource="&teddy;TEDDY_0000023"/>
        <skos:definition xml:lang="en">A quantitative characteristic of the graph of a function.</skos:definition>
    </owl:Class>
    


    <!-- http://biomodels.net/teddy/TEDDY#TEDDY_0000179 -->

    <owl:Class rdf:about="&teddy;TEDDY_0000179">
        <rdfs:label xml:lang="en">excitability</rdfs:label>
        <rdfs:subClassOf rdf:resource="&teddy;TEDDY_0000108"/>
        <rdfs:seeAlso rdf:datatype="&xsd;anyURI">https://identifiers.org/doi/10.1142/S0218127400000840</rdfs:seeAlso>
        <rdfs:seeAlso rdf:datatype="&xsd;anyURI">https://identifiers.org/pubmed/16333295</rdfs:seeAlso>
        <skos:definition xml:lang="en">According to the intuitive definition of excitability, small perturbations near the equilibrium can cause large excursions for the solution before it returns to the equilibrium.</skos:definition>
    </owl:Class>
    <owl:Axiom>
        <owl:annotatedTarget rdf:datatype="&xsd;anyURI">https://identifiers.org/pubmed/16333295</owl:annotatedTarget>
        <rdfs:comment xml:lang="en">Tyson JJ.: Modeling the cell division cycle: cdc2 and cyclin
interactions. Proc Natl Acad Sci U S A. 1991 Aug 15;88(16):7328-32.</rdfs:comment>
        <owl:annotatedSource rdf:resource="&teddy;TEDDY_0000179"/>
        <owl:annotatedProperty rdf:resource="&rdfs;seeAlso"/>
    </owl:Axiom>
    <owl:Axiom>
        <owl:annotatedTarget rdf:datatype="&xsd;anyURI">https://identifiers.org/doi/10.1142/S0218127400000840</owl:annotatedTarget>
        <rdfs:comment xml:lang="en">Eugene M. Izhikevich: Neural Excitability, Spiking and Bursting. Int. J. Bifurcation Chaos, 10, 1171 (2000).</rdfs:comment>
        <owl:annotatedSource rdf:resource="&teddy;TEDDY_0000179"/>
        <owl:annotatedProperty rdf:resource="&rdfs;seeAlso"/>
    </owl:Axiom>
    


    <!-- http://biomodels.net/teddy/TEDDY#TEDDY_obsolete -->

    <owl:Class rdf:about="&teddy;TEDDY_obsolete">
        <rdfs:label xml:lang="en">_obsolete</rdfs:label>
        <rdfs:subClassOf rdf:resource="&teddy;TEDDY_0000000"/>
        <owl:deprecated rdf:datatype="&xsd;boolean">true</owl:deprecated>
    </owl:Class>
    


    <!-- http://www.w3.org/2002/07/owl#Thing -->

    <owl:Class rdf:about="&owl;Thing"/>
    


    <!-- 
    ///////////////////////////////////////////////////////////////////////////////////////
    //
    // General axioms
    //
    ///////////////////////////////////////////////////////////////////////////////////////
     -->

    <rdf:Description>
        <rdf:type rdf:resource="&owl;AllDisjointClasses"/>
        <owl:members rdf:parseType="Collection">
            <rdf:Description rdf:about="&teddy;TEDDY_0000073"/>
            <rdf:Description rdf:about="&teddy;TEDDY_0000074"/>
            <rdf:Description rdf:about="&teddy;TEDDY_0000120"/>
        </owl:members>
    </rdf:Description>
    <rdf:Description>
        <rdf:type rdf:resource="&owl;AllDisjointClasses"/>
        <owl:members rdf:parseType="Collection">
            <rdf:Description rdf:about="&teddy;TEDDY_0000109"/>
            <rdf:Description rdf:about="&teddy;TEDDY_0000110"/>
            <rdf:Description rdf:about="&teddy;TEDDY_0000111"/>
        </owl:members>
    </rdf:Description>
    <owl:Restriction>
        <rdfs:subClassOf>
            <owl:Restriction>
                <owl:onProperty rdf:resource="&teddy;TEDDY_0000176"/>
                <owl:someValuesFrom rdf:resource="&teddy;TEDDY_0000109"/>
            </owl:Restriction>
        </rdfs:subClassOf>
        <owl:onProperty rdf:resource="&ro;has_part"/>
        <owl:onClass rdf:resource="&teddy;TEDDY_0000094"/>
        <owl:qualifiedCardinality rdf:datatype="&xsd;nonNegativeInteger">1</owl:qualifiedCardinality>
    </owl:Restriction>
    <owl:Restriction>
        <rdfs:subClassOf>
            <owl:Restriction>
                <owl:onProperty rdf:resource="&teddy;TEDDY_0000176"/>
                <owl:someValuesFrom rdf:resource="&teddy;TEDDY_0000110"/>
            </owl:Restriction>
        </rdfs:subClassOf>
        <owl:onProperty rdf:resource="&ro;has_part"/>
        <owl:onClass rdf:resource="&teddy;TEDDY_0000094"/>
        <owl:qualifiedCardinality rdf:datatype="&xsd;nonNegativeInteger">2</owl:qualifiedCardinality>
    </owl:Restriction>
    <rdf:Description>
        <rdf:type rdf:resource="&owl;AllDisjointClasses"/>
        <owl:members rdf:parseType="Collection">
            <rdf:Description rdf:about="&teddy;TEDDY_0000087"/>
            <rdf:Description rdf:about="&teddy;TEDDY_0000088"/>
            <rdf:Description rdf:about="&teddy;TEDDY_0000089"/>
            <rdf:Description rdf:about="&teddy;TEDDY_0000090"/>
            <rdf:Description rdf:about="&teddy;TEDDY_0000091"/>
            <rdf:Description rdf:about="&teddy;TEDDY_0000093"/>
        </owl:members>
    </rdf:Description>
    <rdf:Description>
        <rdf:type rdf:resource="&owl;AllDisjointClasses"/>
        <owl:members rdf:parseType="Collection">
            <rdf:Description rdf:about="&teddy;TEDDY_0000002"/>
            <rdf:Description rdf:about="&teddy;TEDDY_0000003"/>
            <rdf:Description rdf:about="&teddy;TEDDY_0000083"/>
            <rdf:Description rdf:about="&teddy;TEDDY_0000132"/>
            <rdf:Description rdf:about="&teddy;TEDDY_obsolete"/>
        </owl:members>
    </rdf:Description>
    <owl:Class>
        <rdfs:subClassOf>
            <owl:Class>
                <owl:intersectionOf rdf:parseType="Collection">
                    <rdf:Description rdf:about="&teddy;TEDDY_0000083"/>
                    <owl:Restriction>
                        <owl:onProperty rdf:resource="&teddy;TR_0004"/>
                        <owl:someValuesFrom rdf:resource="&teddy;TEDDY_0000066"/>
                    </owl:Restriction>
                </owl:intersectionOf>
            </owl:Class>
        </rdfs:subClassOf>
        <owl:intersectionOf rdf:parseType="Collection">
            <rdf:Description rdf:about="&teddy;TEDDY_0000083"/>
            <owl:Restriction>
                <owl:onProperty rdf:resource="&teddy;TR_0004"/>
                <owl:someValuesFrom rdf:resource="&teddy;TEDDY_0000067"/>
            </owl:Restriction>
        </owl:intersectionOf>
    </owl:Class>
    <rdf:Description>
        <rdf:type rdf:resource="&owl;AllDisjointClasses"/>
        <owl:members rdf:parseType="Collection">
            <rdf:Description rdf:about="&teddy;TEDDY_0000133"/>
            <rdf:Description rdf:about="&teddy;TEDDY_0000134"/>
            <rdf:Description rdf:about="&teddy;TEDDY_0000149"/>
            <rdf:Description rdf:about="&teddy;TEDDY_0000157"/>
            <rdf:Description rdf:about="&teddy;TEDDY_0000167"/>
        </owl:members>
    </rdf:Description>
    <rdf:Description>
        <rdf:type rdf:resource="&owl;AllDisjointClasses"/>
        <owl:members rdf:parseType="Collection">
            <rdf:Description rdf:about="&teddy;TEDDY_0000044"/>
            <rdf:Description rdf:about="&teddy;TEDDY_0000045"/>
            <rdf:Description rdf:about="&teddy;TEDDY_0000046"/>
            <rdf:Description rdf:about="&teddy;TEDDY_0000047"/>
        </owl:members>
    </rdf:Description>
    <owl:Class>
        <rdfs:subClassOf rdf:resource="&teddy;TEDDY_0000175"/>
        <owl:intersectionOf rdf:parseType="Collection">
            <rdf:Description rdf:about="&teddy;TEDDY_0000086"/>
            <owl:Restriction>
                <owl:onProperty rdf:resource="&teddy;TR_0004"/>
                <owl:someValuesFrom rdf:resource="&teddy;TEDDY_0000097"/>
            </owl:Restriction>
        </owl:intersectionOf>
    </owl:Class>
    <owl:Axiom>
        <rdfs:seeAlso rdf:datatype="&xsd;anyURI">https://identifiers.org/isbn/9810221428 (p.10)</rdfs:seeAlso>
        <owl:annotatedTarget rdf:resource="&teddy;TEDDY_0000175"/>
        <owl:annotatedProperty rdf:resource="&rdfs;subClassOf"/>
        <owl:annotatedSource>
            <owl:Class>
                <rdfs:subClassOf rdf:resource="&teddy;TEDDY_0000175"/>
                <owl:intersectionOf rdf:parseType="Collection">
                    <rdf:Description rdf:about="&teddy;TEDDY_0000083"/>
                    <owl:Restriction>
                        <owl:onProperty rdf:resource="&teddy;TR_0004"/>
                        <owl:someValuesFrom rdf:resource="&teddy;TEDDY_0000066"/>
                    </owl:Restriction>
                    <owl:Restriction>
                        <owl:onProperty rdf:resource="&teddy;TR_0004"/>
                        <owl:someValuesFrom rdf:resource="&teddy;TEDDY_0000097"/>
                    </owl:Restriction>
                </owl:intersectionOf>
            </owl:Class>
        </owl:annotatedSource>
    </owl:Axiom>
    <rdf:Description>
        <rdf:type rdf:resource="&owl;AllDisjointClasses"/>
        <owl:members rdf:parseType="Collection">
            <rdf:Description rdf:about="&teddy;TEDDY_0000053"/>
            <rdf:Description rdf:about="&teddy;TEDDY_0000055"/>
            <rdf:Description rdf:about="&teddy;TEDDY_0000108"/>
        </owl:members>
    </rdf:Description>
    <rdf:Description>
        <rdf:type rdf:resource="&owl;AllDisjointClasses"/>
        <owl:members rdf:parseType="Collection">
            <rdf:Description rdf:about="&teddy;TEDDY_0000071"/>
            <rdf:Description rdf:about="&teddy;TEDDY_0000121"/>
            <rdf:Description rdf:about="&teddy;TEDDY_0000122"/>
        </owl:members>
    </rdf:Description>
    <rdf:Description>
        <rdf:type rdf:resource="&owl;AllDisjointClasses"/>
        <owl:members rdf:parseType="Collection">
            <rdf:Description rdf:about="&teddy;TEDDY_0000114"/>
            <rdf:Description rdf:about="&teddy;TEDDY_0000128"/>
            <rdf:Description rdf:about="&teddy;TEDDY_0000145"/>
        </owl:members>
    </rdf:Description>
    <owl:Class>
        <rdfs:subClassOf rdf:resource="&teddy;TEDDY_0000175"/>
        <owl:intersectionOf rdf:parseType="Collection">
            <rdf:Description rdf:about="&teddy;TEDDY_0000051"/>
            <owl:Restriction>
                <owl:onProperty rdf:resource="&teddy;TR_0004"/>
                <owl:someValuesFrom rdf:resource="&teddy;TEDDY_0000097"/>
            </owl:Restriction>
        </owl:intersectionOf>
    </owl:Class>
    <owl:Class>
        <rdfs:subClassOf rdf:resource="&teddy;TEDDY_0000022"/>
        <owl:intersectionOf rdf:parseType="Collection">
            <rdf:Description rdf:about="&teddy;TEDDY_0000016"/>
            <rdf:Description rdf:about="&teddy;TEDDY_0000021"/>
        </owl:intersectionOf>
    </owl:Class>
    <rdf:Description>
        <rdf:type rdf:resource="&owl;AllDisjointClasses"/>
        <owl:members rdf:parseType="Collection">
            <rdf:Description rdf:about="&teddy;TEDDY_0000076"/>
            <rdf:Description rdf:about="&teddy;TEDDY_0000077"/>
            <rdf:Description rdf:about="&teddy;TEDDY_0000078"/>
            <rdf:Description rdf:about="&teddy;TEDDY_0000177"/>
        </owl:members>
    </rdf:Description>
    <rdf:Description>
        <rdf:type rdf:resource="&owl;AllDisjointClasses"/>
        <owl:members rdf:parseType="Collection">
            <rdf:Description rdf:about="&teddy;TEDDY_0000012"/>
            <rdf:Description rdf:about="&teddy;TEDDY_0000015"/>
            <rdf:Description rdf:about="&teddy;TEDDY_0000025"/>
            <rdf:Description rdf:about="&teddy;TEDDY_0000130"/>
            <rdf:Description rdf:about="&teddy;TEDDY_0000144"/>
            <rdf:Description rdf:about="&teddy;TEDDY_0000178"/>
        </owl:members>
    </rdf:Description>
    <owl:Class>
        <rdfs:subClassOf>
            <owl:Class>
                <owl:intersectionOf rdf:parseType="Collection">
                    <rdf:Description rdf:about="&teddy;TEDDY_0000083"/>
                    <owl:Restriction>
                        <owl:onProperty rdf:resource="&teddy;TR_0004"/>
                        <owl:someValuesFrom rdf:resource="&teddy;TEDDY_0000130"/>
                    </owl:Restriction>
                </owl:intersectionOf>
            </owl:Class>
        </rdfs:subClassOf>
        <owl:intersectionOf rdf:parseType="Collection">
            <rdf:Description rdf:about="&teddy;TEDDY_0000083"/>
            <owl:Restriction>
                <owl:onProperty rdf:resource="&teddy;TR_0004"/>
                <owl:someValuesFrom rdf:resource="&teddy;TEDDY_0000032"/>
            </owl:Restriction>
        </owl:intersectionOf>
    </owl:Class>
    <rdf:Description>
        <rdf:type rdf:resource="&owl;AllDisjointClasses"/>
        <owl:members rdf:parseType="Collection">
            <rdf:Description rdf:about="&teddy;TEDDY_0000039"/>
            <rdf:Description rdf:about="&teddy;TEDDY_0000040"/>
            <rdf:Description rdf:about="&teddy;TEDDY_0000041"/>
            <rdf:Description rdf:about="&teddy;TEDDY_0000042"/>
        </owl:members>
    </rdf:Description>
    <rdf:Description>
        <rdf:type rdf:resource="&owl;AllDisjointClasses"/>
        <owl:members rdf:parseType="Collection">
            <rdf:Description rdf:about="&teddy;TEDDY_0000134"/>
            <rdf:Description rdf:about="&teddy;TEDDY_0000149"/>
            <rdf:Description rdf:about="&teddy;TEDDY_0000167"/>
        </owl:members>
    </rdf:Description>
    <rdf:Description>
        <rdf:type rdf:resource="&owl;AllDisjointClasses"/>
        <owl:members rdf:parseType="Collection">
            <rdf:Description rdf:about="&teddy;TEDDY_0000072"/>
            <rdf:Description rdf:about="&teddy;TEDDY_0000075"/>
            <rdf:Description rdf:about="&teddy;TEDDY_0000123"/>
        </owl:members>
    </rdf:Description>
    <owl:Axiom>
        <rdfs:seeAlso rdf:datatype="&xsd;anyURI">https://identifiers.org/isbn/9810221428 (p.10)</rdfs:seeAlso>
        <owl:annotatedProperty rdf:resource="&rdfs;subClassOf"/>
        <owl:annotatedSource>
            <owl:Class>
                <rdfs:subClassOf>
                    <owl:Class>
                        <owl:intersectionOf rdf:parseType="Collection">
                            <rdf:Description rdf:about="&teddy;TEDDY_0000083"/>
                            <owl:Restriction>
                                <owl:onProperty rdf:resource="&teddy;TR_0004"/>
                                <owl:someValuesFrom rdf:resource="&teddy;TEDDY_0000066"/>
                            </owl:Restriction>
                        </owl:intersectionOf>
                    </owl:Class>
                </rdfs:subClassOf>
                <owl:intersectionOf rdf:parseType="Collection">
                    <rdf:Description rdf:about="&teddy;TEDDY_0000083"/>
                    <owl:Restriction>
                        <owl:onProperty rdf:resource="&teddy;TR_0004"/>
                        <owl:someValuesFrom rdf:resource="&teddy;TEDDY_0000006"/>
                    </owl:Restriction>
                    <owl:Restriction>
                        <owl:onProperty rdf:resource="&teddy;TR_0004"/>
                        <owl:someValuesFrom rdf:resource="&teddy;TEDDY_0000067"/>
                    </owl:Restriction>
                </owl:intersectionOf>
            </owl:Class>
        </owl:annotatedSource>
        <owl:annotatedTarget>
            <owl:Class>
                <owl:intersectionOf rdf:parseType="Collection">
                    <rdf:Description rdf:about="&teddy;TEDDY_0000083"/>
                    <owl:Restriction>
                        <owl:onProperty rdf:resource="&teddy;TR_0004"/>
                        <owl:someValuesFrom rdf:resource="&teddy;TEDDY_0000066"/>
                    </owl:Restriction>
                </owl:intersectionOf>
            </owl:Class>
        </owl:annotatedTarget>
    </owl:Axiom>
    <rdf:Description>
        <rdf:type rdf:resource="&owl;AllDisjointClasses"/>
        <owl:members rdf:parseType="Collection">
            <rdf:Description rdf:about="&teddy;TEDDY_0000133"/>
            <rdf:Description rdf:about="&teddy;TEDDY_0000134"/>
            <rdf:Description rdf:about="&teddy;TEDDY_0000167"/>
        </owl:members>
    </rdf:Description>
    <owl:Restriction>
        <rdfs:subClassOf>
            <owl:Restriction>
                <owl:onProperty rdf:resource="&teddy;TEDDY_0000176"/>
                <owl:someValuesFrom rdf:resource="&teddy;TEDDY_0000111"/>
            </owl:Restriction>
        </rdfs:subClassOf>
        <owl:onProperty rdf:resource="&ro;has_part"/>
        <owl:onClass rdf:resource="&teddy;TEDDY_0000094"/>
        <owl:minQualifiedCardinality rdf:datatype="&xsd;nonNegativeInteger">3</owl:minQualifiedCardinality>
    </owl:Restriction>
    <owl:Restriction>
        <rdfs:subClassOf>
            <owl:Restriction>
                <owl:onProperty rdf:resource="&ro;has_part"/>
                <owl:someValuesFrom>
                    <owl:Restriction>
                        <owl:onProperty rdf:resource="&teddy;TEDDY_0000174"/>
                        <owl:someValuesFrom rdf:resource="&teddy;TEDDY_0000035"/>
                    </owl:Restriction>
                </owl:someValuesFrom>
            </owl:Restriction>
        </rdfs:subClassOf>
        <owl:onProperty rdf:resource="&teddy;TEDDY_0000176"/>
        <owl:someValuesFrom rdf:resource="&teddy;TEDDY_0000110"/>
    </owl:Restriction>
    <rdf:Description>
        <rdf:type rdf:resource="&owl;AllDisjointClasses"/>
        <owl:members rdf:parseType="Collection">
            <rdf:Description rdf:about="&teddy;TEDDY_0000061"/>
            <rdf:Description rdf:about="&teddy;TEDDY_0000063"/>
            <rdf:Description rdf:about="&teddy;TEDDY_0000066"/>
            <rdf:Description rdf:about="&teddy;TEDDY_0000112"/>
        </owl:members>
    </rdf:Description>
    <owl:Axiom>
        <rdfs:seeAlso rdf:datatype="&xsd;anyURI">https://identifiers.org/isbn/0387983821 (p.196)</rdfs:seeAlso>
        <owl:annotatedProperty rdf:resource="&rdfs;subClassOf"/>
        <owl:annotatedTarget>
            <owl:Class>
                <owl:complementOf>
                    <owl:Restriction>
                        <owl:onProperty rdf:resource="&teddy;TR_0004"/>
                        <owl:someValuesFrom rdf:resource="&teddy;TEDDY_0000167"/>
                    </owl:Restriction>
                </owl:complementOf>
            </owl:Class>
        </owl:annotatedTarget>
        <owl:annotatedSource>
            <owl:Class>
                <rdfs:subClassOf>
                    <owl:Class>
                        <owl:complementOf>
                            <owl:Restriction>
                                <owl:onProperty rdf:resource="&teddy;TR_0004"/>
                                <owl:someValuesFrom rdf:resource="&teddy;TEDDY_0000167"/>
                            </owl:Restriction>
                        </owl:complementOf>
                    </owl:Class>
                </rdfs:subClassOf>
                <owl:intersectionOf rdf:parseType="Collection">
                    <rdf:Description rdf:about="&teddy;TEDDY_0000152"/>
                    <owl:Restriction>
                        <owl:onProperty rdf:resource="&teddy;TR_0013"/>
                        <owl:someValuesFrom>
                            <owl:Class>
                                <owl:intersectionOf rdf:parseType="Collection">
                                    <rdf:Description rdf:about="&teddy;TEDDY_0000086"/>
                                    <owl:Restriction>
                                        <owl:onProperty rdf:resource="&teddy;TR_0004"/>
                                        <owl:someValuesFrom rdf:resource="&teddy;TEDDY_0000157"/>
                                    </owl:Restriction>
                                </owl:intersectionOf>
                            </owl:Class>
                        </owl:someValuesFrom>
                    </owl:Restriction>
                </owl:intersectionOf>
            </owl:Class>
        </owl:annotatedSource>
    </owl:Axiom>
    <owl:Class>
        <rdfs:subClassOf rdf:resource="&teddy;TEDDY_0000175"/>
        <owl:intersectionOf rdf:parseType="Collection">
            <rdf:Description rdf:about="&teddy;TEDDY_0000083"/>
            <owl:Restriction>
                <owl:onProperty rdf:resource="&teddy;TR_0004"/>
                <owl:someValuesFrom rdf:resource="&teddy;TEDDY_0000097"/>
            </owl:Restriction>
            <owl:Restriction>
                <owl:onProperty rdf:resource="&teddy;TR_0004"/>
                <owl:someValuesFrom rdf:resource="&teddy;TEDDY_0000112"/>
            </owl:Restriction>
        </owl:intersectionOf>
    </owl:Class>
    <rdf:Description>
        <rdf:type rdf:resource="&owl;AllDisjointClasses"/>
        <owl:members rdf:parseType="Collection">
            <rdf:Description rdf:about="&teddy;TEDDY_0000002"/>
            <rdf:Description rdf:about="&teddy;TEDDY_0000003"/>
            <rdf:Description rdf:about="&teddy;TEDDY_0000083"/>
            <rdf:Description rdf:about="&teddy;TEDDY_0000132"/>
        </owl:members>
    </rdf:Description>
    <owl:Class>
        <rdfs:subClassOf>
            <owl:Class>
                <owl:intersectionOf rdf:parseType="Collection">
                    <rdf:Description rdf:about="&teddy;TEDDY_0000083"/>
                    <owl:Restriction>
                        <owl:onProperty rdf:resource="&teddy;TR_0004"/>
                        <owl:someValuesFrom rdf:resource="&teddy;TEDDY_0000067"/>
                    </owl:Restriction>
                </owl:intersectionOf>
            </owl:Class>
        </rdfs:subClassOf>
        <owl:intersectionOf rdf:parseType="Collection">
            <rdf:Description rdf:about="&teddy;TEDDY_0000083"/>
            <owl:Restriction>
                <owl:onProperty rdf:resource="&teddy;TR_0004"/>
                <owl:someValuesFrom rdf:resource="&teddy;TEDDY_0000066"/>
            </owl:Restriction>
        </owl:intersectionOf>
    </owl:Class>
    <rdf:Description>
        <rdf:type rdf:resource="&owl;AllDisjointClasses"/>
        <owl:members rdf:parseType="Collection">
            <rdf:Description rdf:about="&teddy;TEDDY_0000050"/>
            <rdf:Description rdf:about="&teddy;TEDDY_0000086"/>
            <rdf:Description rdf:about="&teddy;TEDDY_0000143"/>
        </owl:members>
    </rdf:Description>
</rdf:RDF>



<!-- Generated by the OWL API (version 3.4.2) http://owlapi.sourceforge.net -->

